format-version: 1.2
data-version: 1
date: 29:01:2018 01:11
auto-generated-by: OntoBrowser Export Service

[Term]
id: terms:085493
name: terms_C85493

[Term]
id: terms:0102356
name: Accumulation Ratio AUCTAU
def: "The area under the curve (AUCTAU) at steady state divided by the area under the curve (AUCTAU) over the initial dosing interval."[]
is_a: terms:085493 ! terms_C85493

[Term]
id: terms:0102357
name: Accumulation Ratio Cmax
def: "The maximum concentration at steady state divided by the maximum concentration during the initial dosing interval."[]
is_a: terms:085493 ! terms_C85493

[Term]
id: terms:0102358
name: Accumulation Ratio Cmin
def: "The minimum concentration at steady state divided by the minimum concentration during the initial dosing interval."[]
is_a: terms:085493 ! terms_C85493

[Term]
id: terms:0102359
name: Amt Rec from T1 to T2
def: "The cumulative amount recovered from the specimen type specified in PPSPEC over the interval from T1 to T2."[]
is_a: terms:085493 ! terms_C85493

[Term]
id: terms:0102360
name: Amt Rec from T1 to T2 Norm by BMI
def: "The cumulative amount recovered from the specimen type specified in PPSPEC over the interval from T1 to T2 divided by body mass index."[]
is_a: terms:085493 ! terms_C85493

[Term]
id: terms:0102361
name: Amt Rec from T1 to T2 Norm by SA
def: "The cumulative amount recovered from the specimen type specified in PPSPEC over the interval from T1 to T2 divided by surface area."[]
is_a: terms:085493 ! terms_C85493

[Term]
id: terms:0102362
name: Amt Rec from T1 to T2 Norm by WT
def: "The cumulative amount recovered from the specimen type specified in PPSPEC over the interval from T1 to T2 divided by weight."[]
is_a: terms:085493 ! terms_C85493

[Term]
id: terms:0102363
name: Amt Rec Over Dosing Interval
def: "The cumulative amount recovered from the specimen type specified in PPSPEC between doses (TAU)."[]
is_a: terms:085493 ! terms_C85493

[Term]
id: terms:0102364
name: Amt Rec Over Dosing Interval Norm by BMI
def: "The cumulative amount recovered from the specimen type specified in PPSPEC between doses (TAU) divided by body mass index."[]
is_a: terms:085493 ! terms_C85493

[Term]
id: terms:0102365
name: Amt Rec Over Dosing Interval Norm by SA
def: "The cumulative amount recovered from the specimen type specified in PPSPEC between doses (TAU) divided by surface area."[]
is_a: terms:085493 ! terms_C85493

[Term]
id: terms:0102366
name: Amt Rec Over Dosing Interval Norm by WT
def: "The cumulative amount recovered from the specimen type specified in PPSPEC between doses (TAU) divided by weight."[]
is_a: terms:085493 ! terms_C85493

[Term]
id: terms:0102367
name: Conc by BMI
def: "The concentration divided by body mass index."[]
is_a: terms:085493 ! terms_C85493

[Term]
id: terms:0102368
name: Conc by Dose
def: "The concentration divided by dose."[]
is_a: terms:085493 ! terms_C85493

[Term]
id: terms:0102369
name: Conc by SA
def: "The concentration divided by surface area."[]
is_a: terms:085493 ! terms_C85493

[Term]
id: terms:0102370
name: Conc by WT
def: "The concentration divided by weight."[]
is_a: terms:085493 ! terms_C85493

[Term]
id: terms:0102371
name: Vol Dist Initial
def: "The initial volume of distribution for a substance administered by bolus intravascular dosing."[]
is_a: terms:085493 ! terms_C85493

[Term]
id: terms:0102372
name: Vol Dist Initial Norm by BMI
def: "The initial volume of distribution for a substance administered by bolus intravascular dosing divided by the body mass index."[]
is_a: terms:085493 ! terms_C85493

[Term]
id: terms:0102373
name: Vol Dist Initial Norm by Dose
def: "The initial volume of distribution for a substance administered by bolus intravascular dosing divided by the dose."[]
is_a: terms:085493 ! terms_C85493

[Term]
id: terms:0102374
name: Vol Dist Initial Norm by SA
def: "The initial volume of distribution for a substance administered by bolus intravascular dosing divided by the surface area."[]
is_a: terms:085493 ! terms_C85493

[Term]
id: terms:0102375
name: Vol Dist Initial Norm by WT
def: "The initial volume of distribution for a substance administered by bolus intravascular dosing divided by the weight."[]
is_a: terms:085493 ! terms_C85493

[Term]
id: terms:0102376
name: Nonrenal CL
def: "The total clearance of a substance from the blood less the renal clearance."[]
is_a: terms:085493 ! terms_C85493

[Term]
id: terms:0102377
name: Vol Dist Steady State Obs Norm by BMI
def: "The volume of distribution at steady state based on the observed CLST for a substance administered by intravascular dosing divided by the body mass index."[]
is_a: terms:085493 ! terms_C85493

[Term]
id: terms:0102378
name: Vol Dist Steady State Obs Norm by Dose
def: "The volume of distribution at steady state based on the observed CLST for a substance administered by intravascular dosing divided by the dose."[]
is_a: terms:085493 ! terms_C85493

[Term]
id: terms:0102379
name: Vol Dist Steady State Obs Norm by SA
def: "The volume of distribution at steady state based on the observed CLST for a substance administered by intravascular dosing divided by the surface area."[]
is_a: terms:085493 ! terms_C85493

[Term]
id: terms:0102380
name: Vol Dist Steady State Obs Norm by WT
def: "The volume of distribution at steady state based on the observed CLST for a substance administered by intravascular dosing divided by the weight."[]
is_a: terms:085493 ! terms_C85493

[Term]
id: terms:0102381
name: Peak Trough Ratio
def: "The maximum concentration during a dosing interval divided by the concentration at the end of the dosing interval."[]
is_a: terms:085493 ! terms_C85493

[Term]
id: terms:0102382
name: Pct Rec from T1 to T2
def: "The percentage of the administered dose that is recovered from the specimen type specified in PPSPEC, over the interval between T1 and T2."[]
is_a: terms:085493 ! terms_C85493

[Term]
id: terms:0102383
name: Pct Rec from T1 to T2 Norm by BMI
def: "The percentage of the administered dose that is recovered from the specimen type specified in PPSPEC, over the interval between T1 and T2 divided by body mass index."[]
is_a: terms:085493 ! terms_C85493

[Term]
id: terms:0102384
name: Pct Rec from T1 to T2 Norm by SA
def: "The percentage of the administered dose that is recovered from the specimen type specified in PPSPEC, over the interval between T1 and T2 divided by surface area."[]
is_a: terms:085493 ! terms_C85493

[Term]
id: terms:0102385
name: Pct Rec from T1 to T2 Norm by WT
def: "The percentage of the administered dose that is recovered from the specimen type specified in PPSPEC, over the interval between T1 and T2 divided by weight."[]
is_a: terms:085493 ! terms_C85493

[Term]
id: terms:0102386
name: Pct Rec Over Dosing Interval
def: "The percentage of the administered dose that is recovered from the specimen type specified in PPSPEC, between doses (TAU)."[]
is_a: terms:085493 ! terms_C85493

[Term]
id: terms:0102387
name: Pct Rec Over Dosing Interval Norm by BMI
def: "The percentage of the administered dose that is recovered from the specimen type specified in PPSPEC, between doses (TAU) divided by the body mass index."[]
is_a: terms:085493 ! terms_C85493

[Term]
id: terms:0102388
name: Pct Rec Over Dosing Interval Norm by SA
def: "The percentage of the administered dose that is recovered from the specimen type specified in PPSPEC, between doses (TAU) divided by surface area."[]
is_a: terms:085493 ! terms_C85493

[Term]
id: terms:0102389
name: Pct Rec Over Dosing Interval Norm by WT
def: "The percentage of the administered dose that is recovered from the specimen type specified in PPSPEC, between doses (TAU) divided by weight."[]
is_a: terms:085493 ! terms_C85493

[Term]
id: terms:0102390
name: Vol Dist Steady State Pred Norm by BMI
def: "The volume of distribution at steady state based on the predicted CLST for a substance administered by intravascular dosing divided by the body mass index."[]
is_a: terms:085493 ! terms_C85493

[Term]
id: terms:0102391
name: Vol Dist Steady State Pred Norm by Dose
def: "The volume of distribution at steady state based on the predicted CLST for a substance administered by intravascular dosing divided by the dose."[]
is_a: terms:085493 ! terms_C85493

[Term]
id: terms:0102392
name: Vol Dist Steady State Pred Norm by SA
def: "The volume of distribution at steady state based on the predicted CLST for a substance administered by intravascular dosing divided by the surface area."[]
is_a: terms:085493 ! terms_C85493

[Term]
id: terms:0102393
name: Vol Dist Steady State Pred Norm by WT
def: "The volume of distribution at steady state based on the predicted CLST for a substance administered by intravascular dosing divided by the weight."[]
is_a: terms:085493 ! terms_C85493

[Term]
id: terms:0102394
name: Conc Trough
def: "Concentration at end of dosing interval."[]
is_a: terms:085493 ! terms_C85493

[Term]
id: terms:0102395
name: Conc Trough by BMI
def: "The trough concentration divided by body mass index."[]
is_a: terms:085493 ! terms_C85493

[Term]
id: terms:0102396
name: Conc Trough by Dose
def: "The trough concentration divided by dose."[]
is_a: terms:085493 ! terms_C85493

[Term]
id: terms:0102397
name: Conc Trough by SA
def: "The trough concentration divided by surface area."[]
is_a: terms:085493 ! terms_C85493

[Term]
id: terms:0102398
name: Conc Trough by WT
def: "The trough concentration divided by weight."[]
is_a: terms:085493 ! terms_C85493

[Term]
id: terms:0102426
name: Accumulation Ratio Ctrough
def: "The trough concentration at steady state divided by the trough concentration during the initial dosing interval."[]
is_a: terms:085493 ! terms_C85493

[Term]
id: terms:0102683
name: Vz Obs Norm by Dose
def: "The volume of distribution associated with the terminal slope following intravascular administration, calculated using the observed value of the last non-zero concentration, divided by the dose."[]
is_a: terms:085493 ! terms_C85493

[Term]
id: terms:0102696
name: Vz Pred Norm by Dose
def: "The volume of distribution associated with the terminal slope following intravascular administration, calculated using the predicted value of the last non-zero concentration, divided by the dose."[]
is_a: terms:085493 ! terms_C85493

[Term]
id: terms:0102729
name: Vz Obs by F Norm by Dose
def: "The volume of distribution associated with the terminal slope following extravascular administration divided by the fraction of dose absorbed, calculated using the observed value of the last non-zero concentration, divided by the dose."[]
is_a: terms:085493 ! terms_C85493

[Term]
id: terms:0102730
name: Vz Pred by F Norm by Dose
def: "The volume of distribution associated with the terminal slope following extravascular administration divided by the fraction of dose absorbed, calculated using the predicted value of the last non-zero concentration, divided by the dose."[]
is_a: terms:085493 ! terms_C85493

[Term]
id: terms:0105449
name: Excret Rate from T1 to T2
def: "The excretion rate over the interval from T1 to T2, determined for the specimen type specified in PPSPEC."[]
is_a: terms:085493 ! terms_C85493

[Term]
id: terms:0105450
name: Excret Rate from T1 to T2 Norm by BMI
def: "The excretion rate over the interval from T1 to T2 divided by the body mass index, determined for the specimen type specified in PPSPEC."[]
is_a: terms:085493 ! terms_C85493

[Term]
id: terms:0105451
name: Excret Rate from T1 to T2 Norm by Dose
def: "The excretion rate over the interval from T1 to T2 divided by the dose, determined for the specimen type specified in PPSPEC."[]
is_a: terms:085493 ! terms_C85493

[Term]
id: terms:0105452
name: Excret Rate from T1 to T2 Norm by SA
def: "The excretion rate over the interval from T1 to T2 divided by the surface area, determined for the specimen type specified in PPSPEC."[]
is_a: terms:085493 ! terms_C85493

[Term]
id: terms:0105453
name: Excret Rate from T1 to T2 Norm by WT
def: "The excretion rate over the interval from T1 to T2 divided by the weight, determined for the specimen type specified in PPSPEC."[]
is_a: terms:085493 ! terms_C85493

[Term]
id: terms:0105454
name: Nonrenal CL Norm by BMI
def: "The total clearance of a substance from the blood minus the renal clearance divided by the body mass index."[]
is_a: terms:085493 ! terms_C85493

[Term]
id: terms:0105455
name: Nonrenal CL Norm by Dose
def: "The total clearance of a substance from the blood minus the renal clearance divided by the dose."[]
is_a: terms:085493 ! terms_C85493

[Term]
id: terms:0105456
name: Nonrenal CL Norm by SA
def: "The total clearance of a substance from the blood minus the renal clearance divided by the surface area."[]
is_a: terms:085493 ! terms_C85493

[Term]
id: terms:0105457
name: Nonrenal CL Norm by WT
def: "The total clearance of a substance from the blood minus the renal clearance divided by the weight."[]
is_a: terms:085493 ! terms_C85493

[Term]
id: terms:0105458
name: Renal CL Norm by BMI
def: "The clearance of a substance from the blood by the kidneys divided by the body mass index."[]
is_a: terms:085493 ! terms_C85493

[Term]
id: terms:0105459
name: Renal CL Norm by Dose
def: "The clearance of a substance from the blood by the kidneys divided by the dose."[]
is_a: terms:085493 ! terms_C85493

[Term]
id: terms:0105460
name: Renal CL Norm by SA
def: "The clearance of a substance from the blood by the kidneys divided by the surface area."[]
is_a: terms:085493 ! terms_C85493

[Term]
id: terms:0105461
name: Renal CL Norm by WT
def: "The clearance of a substance from the blood by the kidneys divided by the weight."[]
is_a: terms:085493 ! terms_C85493

[Term]
id: terms:0111333
name: Vz for Dose Int
def: "The volume of distribution associated with the terminal slope following intravascular administration, calculated using AUCTAU."[]
is_a: terms:085493 ! terms_C85493

[Term]
id: terms:0111364
name: Vz for Dose Int by F
def: "The volume of distribution associated with the terminal slope following extravascular administration divided by the fraction of dose absorbed, calculated using AUCTAU."[]
is_a: terms:085493 ! terms_C85493

[Term]
id: terms:0111365
name: Vz for Dose Int by F Norm by BMI
def: "The volume of distribution associated with the terminal slope following extravascular administration divided by the fraction of dose absorbed, calculated using AUCTAU, divided by the body mass index."[]
is_a: terms:085493 ! terms_C85493

[Term]
id: terms:0111366
name: Vz for Dose Int by F Norm by Dose
def: "The volume of distribution associated with the terminal slope following extravascular administration divided by the fraction of dose absorbed, calculated using AUCTAU, divided by the dose."[]
is_a: terms:085493 ! terms_C85493

[Term]
id: terms:0111367
name: Vz for Dose Int by F Norm by SA
def: "The volume of distribution associated with the terminal slope following extravascular administration divided by the fraction of dose absorbed, calculated using AUCTAU, divided by the surface area."[]
is_a: terms:085493 ! terms_C85493

[Term]
id: terms:0111368
name: Vz for Dose Int by F Norm by WT
def: "The volume of distribution associated with the terminal slope following extravascular administration divided by the fraction of dose absorbed, calculated using AUCTAU, divided by the weight."[]
is_a: terms:085493 ! terms_C85493

[Term]
id: terms:0111369
name: Vz for Dose Int Norm by BMI
def: "The volume of distribution associated with the terminal slope following intravascular administration, calculated using AUCTAU, divided by the body mass index."[]
is_a: terms:085493 ! terms_C85493

[Term]
id: terms:0111370
name: Vz for Dose Int Norm by Dose
def: "The volume of distribution associated with the terminal slope following intravascular administration, calculated using AUCTAU, divided by the dose."[]
is_a: terms:085493 ! terms_C85493

[Term]
id: terms:0111371
name: Vz for Dose Int Norm by SA
def: "The volume of distribution associated with the terminal slope following intravascular administration, calculated using AUCTAU, divided by the surface area."[]
is_a: terms:085493 ! terms_C85493

[Term]
id: terms:0111372
name: Vz for Dose Int Norm by WT
def: "The volume of distribution associated with the terminal slope following intravascular administration, calculated using AUCTAU, divided by the weight."[]
is_a: terms:085493 ! terms_C85493

[Term]
id: terms:0112032
name: Amt Rec Infinity Obs
def: "The cumulative amount recovered from the specimen type specified in PPSPEC extrapolated to infinity, calculated using the observed value of the last non-zero concentration."[]
is_a: terms:085493 ! terms_C85493

[Term]
id: terms:0112033
name: Amt Rec Infinity Pred
def: "The cumulative amount recovered from the specimen type specified in PPSPEC extrapolated to infinity, calculated using the predicted value of the last non-zero concentration."[]
is_a: terms:085493 ! terms_C85493

[Term]
id: terms:0112034
name: Pct Rec Infinity Obs
def: "The percentage of the administered dose that is recovered from the specimen type specified in PPSPEC extrapolated to infinity, calculated using the observed value of the last non-zero concentration."[]
is_a: terms:085493 ! terms_C85493

[Term]
id: terms:0112035
name: Pct Rec Infinity Pred
def: "The percentage of the administered dose that is recovered from the specimen type specified in PPSPEC extrapolated to infinity, calculated using the predicted value of the last non-zero concentration."[]
is_a: terms:085493 ! terms_C85493

[Term]
id: terms:0112223
name: Amt Rec Infinity Obs Norm by BMI
def: "The cumulative amount recovered from the specimen type specified in PPSPEC extrapolated to infinity, calculated using the observed value of the last non-zero concentration, divided by the body mass index."[]
is_a: terms:085493 ! terms_C85493

[Term]
id: terms:0112224
name: Amt Rec Infinity Obs Norm by SA
def: "The cumulative amount recovered from the specimen type specified in PPSPEC extrapolated to infinity, calculated using the observed value of the last non-zero concentration, divided by the surface area."[]
is_a: terms:085493 ! terms_C85493

[Term]
id: terms:0112225
name: Amt Rec Infinity Obs Norm by WT
def: "The cumulative amount recovered from the specimen type specified in PPSPEC extrapolated to infinity, calculated using the observed value of the last non-zero concentration, divided by the weight."[]
is_a: terms:085493 ! terms_C85493

[Term]
id: terms:0112226
name: Amt Rec Infinity Pred Norm by BMI
def: "The cumulative amount recovered from the specimen type specified in PPSPEC extrapolated to infinity, calculated using the predicted value of the last non-zero concentration, divided by the body mass index."[]
is_a: terms:085493 ! terms_C85493

[Term]
id: terms:0112227
name: Amt Rec Infinity Pred Norm by SA
def: "The cumulative amount recovered from the specimen type specified in PPSPEC extrapolated to infinity, calculated using the predicted value of the last non-zero concentration, divided by the surface area."[]
is_a: terms:085493 ! terms_C85493

[Term]
id: terms:0112228
name: Amt Rec Infinity Pred Norm by WT
def: "The cumulative amount recovered from the specimen type specified in PPSPEC extrapolated to infinity, calculated using the predicted value of the last non-zero concentration, divided by the weight."[]
is_a: terms:085493 ! terms_C85493

[Term]
id: terms:0112287
name: Hemodialysis Clearance
def: "The clearance of a substance from the blood during a hemodialysis session."[]
is_a: terms:085493 ! terms_C85493

[Term]
id: terms:0112389
name: Pct Rec Infinity Obs Norm by BMI
def: "The percentage of the administered dose that is recovered from the specimen type specified in PPSPEC extrapolated to infinity, calculated using the observed value of the last non-zero concentration, divided by the body mass index."[]
is_a: terms:085493 ! terms_C85493

[Term]
id: terms:0112390
name: Pct Rec Infinity Obs Norm by SA
def: "The percentage of the administered dose that is recovered from the specimen type specified in PPSPEC extrapolated to infinity, calculated using the observed value of the last non-zero concentration, divided by the surface area."[]
is_a: terms:085493 ! terms_C85493

[Term]
id: terms:0112391
name: Pct Rec Infinity Obs Norm by WT
def: "The percentage of the administered dose that is recovered from the specimen type specified in PPSPEC extrapolated to infinity, calculated using the observed value of the last non-zero concentration, divided by the weight."[]
is_a: terms:085493 ! terms_C85493

[Term]
id: terms:0112392
name: Pct Rec Infinity Pred Norm by BMI
def: "The percentage of the administered dose that is recovered from the specimen type specified in PPSPEC extrapolated to infinity, calculated using the predicted value of the last non-zero concentration, divided by the body mass index."[]
is_a: terms:085493 ! terms_C85493

[Term]
id: terms:0112393
name: Pct Rec Infinity Pred Norm by SA
def: "The percentage of the administered dose that is recovered from the specimen type specified in PPSPEC extrapolated to infinity, calculated using the predicted value of the last non-zero concentration, divided by the surface area."[]
is_a: terms:085493 ! terms_C85493

[Term]
id: terms:0112394
name: Pct Rec Infinity Pred Norm by WT
def: "The percentage of the administered dose that is recovered from the specimen type specified in PPSPEC extrapolated to infinity, calculated using the predicted value of the last non-zero concentration, divided by the weight."[]
is_a: terms:085493 ! terms_C85493

[Term]
id: terms:0114121
name: Total CL by F for Dose Int
def: "The total body clearance for extravascular administration divided by the fraction of dose absorbed, calculated using AUCTAU."[]
is_a: terms:085493 ! terms_C85493

[Term]
id: terms:0114122
name: Total CL for Dose Int
def: "The total body clearance for intravascular administration, calculated using AUCTAU."[]
is_a: terms:085493 ! terms_C85493

[Term]
id: terms:0114226
name: Total CL by F for Dose Int Norm by Dose
def: "The total body clearance for extravascular administration divided by the fraction of dose absorbed, calculated using AUCTAU, divided by the dose."[]
is_a: terms:085493 ! terms_C85493

[Term]
id: terms:0114227
name: Total CL by F for Dose Int Norm by BMI
def: "The total body clearance for extravascular administration divided by the fraction of dose absorbed, calculated using AUCTAU, divided by the body mass index."[]
is_a: terms:085493 ! terms_C85493

[Term]
id: terms:0114228
name: Total CL by F for Dose Int Norm by SA
def: "The total body clearance for extravascular administration divided by the fraction of dose absorbed, calculated using AUCTAU, divided by the surface area."[]
is_a: terms:085493 ! terms_C85493

[Term]
id: terms:0114229
name: Total CL by F for Dose Int Norm by WT
def: "The total body clearance for extravascular administration divided by the fraction of dose absorbed, calculated using AUCTAU, divided by the weight."[]
is_a: terms:085493 ! terms_C85493

[Term]
id: terms:0114230
name: Total CL for Dose Int Norm by Dose
def: "The total body clearance for intravascular administration, calculated using AUCTAU, divided by the dose."[]
is_a: terms:085493 ! terms_C85493

[Term]
id: terms:0114231
name: Total CL for Dose Int Norm by BMI
def: "The total body clearance for intravascular administration, calculated using AUCTAU, divided by the body mass index."[]
is_a: terms:085493 ! terms_C85493

[Term]
id: terms:0114232
name: Total CL for Dose Int Norm by SA
def: "The total body clearance for intravascular administration, calculated using AUCTAU, divided by the surface area."[]
is_a: terms:085493 ! terms_C85493

[Term]
id: terms:0114233
name: Total CL for Dose Int Norm by WT
def: "The total body clearance for intravascular administration, calculated using AUCTAU, divided by the weight."[]
is_a: terms:085493 ! terms_C85493

[Term]
id: terms:0114234
name: Accumulation Index using Lambda z
def: "Predicted accumulation ratio for area under the curve (AUC) calculated using the Lambda z estimated from single dose data."[]
is_a: terms:085493 ! terms_C85493

[Term]
id: terms:0116213
name: Hemodialysis Extraction Ratio
def: "The fractional content of a substance removed from the blood during a hemodialysis session."[]
is_a: terms:085493 ! terms_C85493

[Term]
id: terms:0120723
name: Mean Absorption Time
def: "Mean absorption time of a substance administered by extravascular dosing."[]
is_a: terms:085493 ! terms_C85493

[Term]
id: terms:0120724
name: MRT Extravasc Infinity Obs
def: "The mean residence time (MRT) extrapolated to infinity for a substance administered by extravascular dosing, calculated using the observed value of the last non-zero concentration. Extravascular MRT includes Mean Absorption Time (MAT)."[]
is_a: terms:085493 ! terms_C85493

[Term]
id: terms:0120725
name: MRT Extravasc Infinity Pred
def: "The mean residence time (MRT) extrapolated to infinity for a substance administered by extravascular dosing, calculated using the predicted value of the last non-zero concentration. Extravascular MRT includes Mean Absorption Time (MAT)."[]
is_a: terms:085493 ! terms_C85493

[Term]
id: terms:0120726
name: MRT Extravasc to Last Nonzero Conc
def: "Mean residence time (MRT) from the time of dosing to the time of the last measurable concentration for a substance administered by extravascular dosing. Extravascular MRT includes Mean Absorption Time (MAT)."[]
is_a: terms:085493 ! terms_C85493

[Term]
id: terms:0121134
name: MRT Intravasc Infinity Obs
def: "The mean residence time (MRT) extrapolated to infinity for a substance administered by intravascular dosing, calculated using the observed value of the last non-zero concentration."[]
is_a: terms:085493 ! terms_C85493

[Term]
id: terms:0121136
name: MRT Intravasc Infinity Pred
def: "The mean residence time (MRT) extrapolated to infinity for a substance administered by intravascular dosing, calculated using the predicted value of the last non-zero concentration."[]
is_a: terms:085493 ! terms_C85493

[Term]
id: terms:0121137
name: MRT Intravasc to Last Nonzero Conc
def: "Mean residence time (MRT) from the time of dosing to the time of the last measurable concentration, for a substance administered by intravascular dosing."[]
is_a: terms:085493 ! terms_C85493

[Term]
id: terms:0122049
name: Renal CL from T1 to T2
def: "The clearance of a substance from the blood by the kidneys over the interval from T1 to T2."[]
is_a: terms:085493 ! terms_C85493

[Term]
id: terms:0122050
name: Renal CL for Dose Int
def: "The clearance of a substance from the blood by the kidneys, calculated using AUCTAU."[]
is_a: terms:085493 ! terms_C85493

[Term]
id: terms:0122329
name: Accumulation Ratio AUC from T1 to T2
def: "The area under the curve from T1 to T2 at steady state divided by the area under the curve from T1 to T2 during the initial dosing interval."[]
is_a: terms:085493 ! terms_C85493

[Term]
id: terms:0122330
name: Renal CL from T1 to T2 Norm by BMI
def: "The clearance of a substance from the blood by the kidneys over the interval from T1 to T2 divided by the body mass index."[]
is_a: terms:085493 ! terms_C85493

[Term]
id: terms:0122331
name: Renal CL from T1 to T2 Norm by Dose
def: "The clearance of a substance from the blood by the kidneys over the interval from T1 to T2 divided by the dose."[]
is_a: terms:085493 ! terms_C85493

[Term]
id: terms:0122332
name: Renal CL from T1 to T2 Norm by SA
def: "The clearance of a substance from the blood by the kidneys over the interval from T1 to T2 divided by the surface area."[]
is_a: terms:085493 ! terms_C85493

[Term]
id: terms:0122333
name: Renal CL from T1 to T2 Norm by WT
def: "The clearance of a substance from the blood by the kidneys over the interval from T1 to T2 divided by the weight."[]
is_a: terms:085493 ! terms_C85493

[Term]
id: terms:0122334
name: Renal CL for Dose Int Norm by BMI
def: "The clearance of a substance from the blood by the kidneys, calculated using AUCTAU, divided by the body mass index."[]
is_a: terms:085493 ! terms_C85493

[Term]
id: terms:0122335
name: Renal CL for Dose Int Norm by Dose
def: "The clearance of a substance from the blood by the kidneys, calculated using AUCTAU, divided by the dose."[]
is_a: terms:085493 ! terms_C85493

[Term]
id: terms:0122336
name: Renal CL for Dose Int Norm by SA
def: "The clearance of a substance from the blood by the kidneys, calculated using AUCTAU, divided by the surface area."[]
is_a: terms:085493 ! terms_C85493

[Term]
id: terms:0122337
name: Renal CL for Dose Int Norm by WT
def: "The clearance of a substance from the blood by the kidneys, calculated using AUCTAU, divided by the weight."[]
is_a: terms:085493 ! terms_C85493

[Term]
id: terms:0122338
name: Stationarity Ratio AUC
def: "The area under the curve (AUCTAU) at steady state divided by the area under the curve extrapolated to infinity for the initial dosing interval."[]
is_a: terms:085493 ! terms_C85493

[Term]
id: terms:0122339
name: Trough Peak Ratio
def: "The concentration at the start of a dosing interval divided by the maximum concentration during the dosing interval."[]
is_a: terms:085493 ! terms_C85493

[Term]
id: terms:0200002
name: Unassigned
def: "PK parameter has not yet been assigned."[]
is_a: terms:085493 ! terms_C85493

[Term]
id: terms:0200003
name: Unknown
def: "PK parameter is unknown."[]
is_a: terms:085493 ! terms_C85493

[Term]
id: terms:041185
name: Concentration
def: "The quantity of a specified substance in a unit volume or weight of another substance."[]
is_a: terms:085493 ! terms_C85493

[Term]
id: terms:070918
name: Max Conc
def: "The maximum concentration occurring at Tmax."[]
is_a: terms:085493 ! terms_C85493

[Term]
id: terms:070919
name: Time of CMAX
def: "The time of maximum observed concentration sampled during a dosing interval."[]
is_a: terms:085493 ! terms_C85493

[Term]
id: terms:075913
name: Renal CL
def: "The clearance of a substance from the blood by the kidneys."[]
is_a: terms:085493 ! terms_C85493

[Term]
id: terms:085542
name: R Squared
def: "The goodness of fit statistic for the terminal elimination phase."[]
is_a: terms:085493 ! terms_C85493

[Term]
id: terms:085553
name: R Squared Adjusted
def: "The goodness of fit statistic for the terminal elimination phase, adjusted for the number of time points used in the estimation of Lambda z."[]
is_a: terms:085493 ! terms_C85493

[Term]
id: terms:085564
name: AUC All
def: "The area under the curve (AUC) from the time of dosing to the time of the last observation, regardless of whether the last concentration is measurable or not."[]
is_a: terms:085493 ! terms_C85493

[Term]
id: terms:085565
name: AUC to Last Nonzero Conc
def: "The area under the curve (AUC) from the time of dosing to the last measurable concentration."[]
is_a: terms:085493 ! terms_C85493

[Term]
id: terms:085566
name: AUC from T1 to T2
def: "The area under the curve (AUC) over the interval from T1 to T2."[]
is_a: terms:085493 ! terms_C85493

[Term]
id: terms:085567
name: AUC Over Dosing Interval
def: "The area under the curve (AUC) for the defined interval between doses (TAU)."[]
is_a: terms:085493 ! terms_C85493

[Term]
id: terms:085569
name: AUMC to Last Nonzero Conc
def: "The area under the moment curve (AUMC) from the time of dosing to the last measurable concentration."[]
is_a: terms:085493 ! terms_C85493

[Term]
id: terms:085570
name: AUMC Over Dosing Interval
def: "The area under the first moment curve (AUMC) for the defined interval between doses (TAU)."[]
is_a: terms:085493 ! terms_C85493

[Term]
id: terms:085571
name: AURC to Last Nonzero Rate
def: "The area under the urinary excretion rate curve (AURC) from time zero to the time of the last measurable concentration."[]
is_a: terms:085493 ! terms_C85493

[Term]
id: terms:085572
name: AURC from T1 to T2
def: "The area under the urinary excretion rate curve (AURC) over the interval from T1 to T2."[]
is_a: terms:085493 ! terms_C85493

[Term]
id: terms:085575
name: Average Concentration
def: "AUCTAU divided by TAU."[]
is_a: terms:085493 ! terms_C85493

[Term]
id: terms:085579
name: Min Conc
def: "The minimum concentration between dose time and dose time plus Tau (at Tmin)."[]
is_a: terms:085493 ! terms_C85493

[Term]
id: terms:085580
name: Midpoint of Interval of Last Nonzero ER
def: "The midpoint of collection interval associated with last measurable excretion rate."[]
is_a: terms:085493 ! terms_C85493

[Term]
id: terms:085581
name: Fluctuation%
def: "The difference between Cmin and Cmax standardized to Cavg, between dose time and Tau."[]
is_a: terms:085493 ! terms_C85493

[Term]
id: terms:085644
name: Initial Conc
def: "Initial concentration. Given only for bolus IV models."[]
is_a: terms:085493 ! terms_C85493

[Term]
id: terms:085652
name: Lambda z
def: "The first order rate constant associated with the terminal (log-linear) portion of the curve."[]
is_a: terms:085493 ! terms_C85493

[Term]
id: terms:085653
name: Lambda z Lower Limit
def: "The lower limit on time for values to be included in the calculation of Lambda z."[]
is_a: terms:085493 ! terms_C85493

[Term]
id: terms:085654
name: Lambda z Upper Limit
def: "The upper limit on time for values to be included in the calculation of Lambda z."[]
is_a: terms:085493 ! terms_C85493

[Term]
id: terms:085655
name: Last Nonzero Conc
def: "The concentration corresponding to Tlast."[]
is_a: terms:085493 ! terms_C85493

[Term]
id: terms:085656
name: Last Meas Excretion Rate
def: "The last measurable (positive) excretion rate determined for the specimen type specified in PPSPEC."[]
is_a: terms:085493 ! terms_C85493

[Term]
id: terms:085698
name: Max Conc Norm by Dose
def: "The maximum concentration occurring at Tmax, divided by the dose."[]
is_a: terms:085493 ! terms_C85493

[Term]
id: terms:085699
name: Max Excretion Rate
def: "The maximum excretion rate determined for the specimen type specified in PPSPEC."[]
is_a: terms:085493 ! terms_C85493

[Term]
id: terms:085761
name: AUC Infinity Obs
def: "The area under the curve (AUC) extrapolated to infinity, calculated using the observed value of the last non-zero concentration."[]
is_a: terms:085493 ! terms_C85493

[Term]
id: terms:085763
name: AUC %Back Extrapolation Obs
def: "Applies only for intravascular bolus dosing. The area under the curve (AUC) from the first measured concentration value back extrapolated to the concentration value at time zero as a percentage of the area under the curve extrapolated to infinity using the observed value of the last non-zero concentration."[]
is_a: terms:085493 ! terms_C85493

[Term]
id: terms:085764
name: AUC %Extrapolation Obs
def: "The area under the curve (AUC) from the last observed non-zero concentration value to infinity as a percentage of the area under the curve extrapolated to infinity."[]
is_a: terms:085493 ! terms_C85493

[Term]
id: terms:085765
name: AUMC Infinity Obs
def: "The area under the moment curve (AUMC) extrapolated to infinity, calculated using the observed value of the last non-zero concentration."[]
is_a: terms:085493 ! terms_C85493

[Term]
id: terms:085766
name: AUMC % Extrapolation Obs
def: "The area under the moment curve (AUMC) from the last observed non-zero concentration value to infinity as a percentage of the area under the moment curve extrapolated to infinity."[]
is_a: terms:085493 ! terms_C85493

[Term]
id: terms:085767
name: AURC Infinity Obs
def: "The area under the urinary excretion rate curve (AURC) extrapolated to infinity, calculated using the observed value of the last excretion rate."[]
is_a: terms:085493 ! terms_C85493

[Term]
id: terms:085768
name: AURC % Extrapolation Obs
def: "The area under the urinary excretion rate curve (AURC) from the last observed non-zero rate value to infinity as a percentage of the area under the urinary excretion rate curve extrapolated to infinity."[]
is_a: terms:085493 ! terms_C85493

[Term]
id: terms:085770
name: Vol Dist Steady State Obs
def: "The volume of distribution at steady state based on the observed CLST for a substance administered by intravascular dosing."[]
is_a: terms:085493 ! terms_C85493

[Term]
id: terms:085772
name: Total CL Obs by F
def: "The total body clearance for extravascular administration divided by the fraction of dose absorbed, calculated using the observed value of the last non-zero concentration."[]
is_a: terms:085493 ! terms_C85493

[Term]
id: terms:085773
name: Total CL Obs
def: "The total body clearance for intravascular administration, calculated using the observed value of the last non-zero concentration."[]
is_a: terms:085493 ! terms_C85493

[Term]
id: terms:085774
name: Vz Obs
def: "The volume of distribution associated with the terminal slope following intravascular administration, calculated using the observed value of the last non-zero concentration."[]
is_a: terms:085493 ! terms_C85493

[Term]
id: terms:085775
name: Vz Obs by F
def: "The volume of distribution associated with the terminal slope following extravascular administration divided by the fraction of dose absorbed, calculated using the observed value of the last non-zero concentration."[]
is_a: terms:085493 ! terms_C85493

[Term]
id: terms:085785
name: AUC Infinity Pred
def: "The area under the curve (AUC) extrapolated to infinity, calculated using the predicted value of the last non-zero concentration."[]
is_a: terms:085493 ! terms_C85493

[Term]
id: terms:085786
name: AUC Infinity Pred Norm by Dose
def: "The area under the curve (AUC) extrapolated to infinity, calculated using the predicted value of the last non-zero concentration, divided by the dose."[]
is_a: terms:085493 ! terms_C85493

[Term]
id: terms:085787
name: AUC %Back Extrapolation Pred
def: "Applies only for intravascular bolus dosing. The area under the curve (AUC) from the first measured concentration value back extrapolated to the concentration value at time zero as a percentage of the area under the curve extrapolated to infinity using the predicted value of the last non-zero concentration."[]
is_a: terms:085493 ! terms_C85493

[Term]
id: terms:085788
name: AUC %Extrapolation Pred
def: "The area under the curve (AUC) from the last predicted non-zero concentration value to infinity as a percentage of the area under the curve extrapolated to infinity."[]
is_a: terms:085493 ! terms_C85493

[Term]
id: terms:085789
name: AUMC Infinity Pred
def: "The area under the moment curve (AUMC) extrapolated to infinity, calculated using the predicted value of the last non-zero concentration."[]
is_a: terms:085493 ! terms_C85493

[Term]
id: terms:085790
name: AUMC % Extrapolation Pred
def: "The area under the moment curve (AUMC) from the last predicted non-zero concentration value to infinity as a percentage of the area under the moment curve extrapolated to infinity."[]
is_a: terms:085493 ! terms_C85493

[Term]
id: terms:085791
name: AURC Infinity Pred
def: "The area under the urinary excretion rate curve (AURC) extrapolated to infinity, calculated using the predicted value of the last non-zero excretion rate."[]
is_a: terms:085493 ! terms_C85493

[Term]
id: terms:085792
name: AURC % Extrapolation Pred
def: "The area under the urinary excretion rate curve (AURC) from the last predicted non-zero rate value to infinity as a percentage of the area under the urinary excretion rate curve extrapolated to infinity."[]
is_a: terms:085493 ! terms_C85493

[Term]
id: terms:085794
name: Vol Dist Steady State Pred
def: "The volume of distribution at steady state based on the predicted CLST for a substance administered by intravascular dosing."[]
is_a: terms:085493 ! terms_C85493

[Term]
id: terms:085796
name: Total CL Pred by F
def: "The total body clearance for extravascular administration divided by the fraction of dose absorbed, calculated using the predicted value of the last non-zero concentration."[]
is_a: terms:085493 ! terms_C85493

[Term]
id: terms:085797
name: Total CL Pred
def: "The total body clearance for intravascular administration, calculated using the predicted value of the last non-zero concentration."[]
is_a: terms:085493 ! terms_C85493

[Term]
id: terms:085798
name: Vz Pred
def: "The volume of distribution associated with the terminal slope following intravascular administration, calculated using the predicted value of the last non-zero concentration."[]
is_a: terms:085493 ! terms_C85493

[Term]
id: terms:085799
name: Vz Pred by F
def: "The volume of distribution associated with the terminal slope following extravascular administration divided by the fraction of dose absorbed, calculated using the predicted value of the last non-zero concentration."[]
is_a: terms:085493 ! terms_C85493

[Term]
id: terms:085816
name: Number of Points for Lambda z
def: "The number of time points used in computing Lambda z."[]
is_a: terms:085493 ! terms_C85493

[Term]
id: terms:085817
name: Sum of Urine Vol
def: "The sum of urine volumes that are used for PK parameters."[]
is_a: terms:085493 ! terms_C85493

[Term]
id: terms:085818
name: Half-Life Lambda z
def: "Terminal half-life."[]
is_a: terms:085493 ! terms_C85493

[Term]
id: terms:085821
name: Correlation Between TimeX and Log ConcY
def: "The correlation between time (X) and log concentration (Y) for the points used in the estimation of lambda z."[]
is_a: terms:085493 ! terms_C85493

[Term]
id: terms:085822
name: Time of Last Nonzero Conc
def: "The time of the last measurable (positive) concentration."[]
is_a: terms:085493 ! terms_C85493

[Term]
id: terms:085823
name: Midpoint of Interval of Maximum ER
def: "The midpoint of collection interval associated with the maximum excretion rate."[]
is_a: terms:085493 ! terms_C85493

[Term]
id: terms:085824
name: Time Until First Nonzero Conc
def: "The time prior to the first measurable (non-zero) concentration."[]
is_a: terms:085493 ! terms_C85493

[Term]
id: terms:085825
name: Time of CMIN Observation
def: "The time of minimum concentration sampled during a dosing interval."[]
is_a: terms:085493 ! terms_C85493

[Term]
id: terms:085841
name: AURC All
def: "The area under the urinary excretion rate curve (AURC) from time zero to the time of the last observation, regardless of whether the last observation is a measurable concentration or not."[]
is_a: terms:085493 ! terms_C85493

[Term]
id: terms:092305
name: AUC to Last Nonzero Conc Norm by WT
def: "The area under the curve (AUC) from the time of dosing to the last measurable concentration divided by the weight."[]
is_a: terms:085493 ! terms_C85493

[Term]
id: terms:092306
name: AUC All Norm by Dose
def: "The area under the curve (AUC) from the time of dosing to the time of the last observation divided by the dose, regardless of whether the last concentration is measurable or not."[]
is_a: terms:085493 ! terms_C85493

[Term]
id: terms:092307
name: AUC All Norm by SA
def: "The area under the curve (AUC) from the time of dosing to the time of the last observation divided by the surface area, regardless of whether the last concentration is measurable or not."[]
is_a: terms:085493 ! terms_C85493

[Term]
id: terms:092308
name: AUC All Norm by WT
def: "The area under the curve (AUC) from the time of dosing to the time of the last observation divided by the weight, regardless of whether the last concentration is measurable or not."[]
is_a: terms:085493 ! terms_C85493

[Term]
id: terms:092309
name: AUC to Last Nonzero Conc Norm by BMI
def: "The area under the curve (AUC) from the time of dosing to the last measurable concentration divided by the body mass index."[]
is_a: terms:085493 ! terms_C85493

[Term]
id: terms:092310
name: AUC to Last Nonzero Conc Norm by Dose
def: "The area under the curve (AUC) from the time of dosing to the last measurable concentration divided by the dose."[]
is_a: terms:085493 ! terms_C85493

[Term]
id: terms:092311
name: AUC to Last Nonzero Conc Norm by SA
def: "The area under the curve (AUC) from the time of dosing to the last measurable concentration divided by the surface area."[]
is_a: terms:085493 ! terms_C85493

[Term]
id: terms:092312
name: AUC from T1 to T2 Norm by BMI
def: "The area under the curve (AUC) over the interval from T1 to T2 divided by the body mass index."[]
is_a: terms:085493 ! terms_C85493

[Term]
id: terms:092313
name: AUC from T1 to T2 Norm by Dose
def: "The area under the curve (AUC) over the interval from T1 to T2 divided by the dose."[]
is_a: terms:085493 ! terms_C85493

[Term]
id: terms:092314
name: AUC from T1 to T2 Norm by SA
def: "The area under the curve (AUC) over the interval from T1 to T2 divided by the surface area."[]
is_a: terms:085493 ! terms_C85493

[Term]
id: terms:092315
name: AUC from T1 to T2 Norm by WT
def: "The area under the curve (AUC) over the interval from T1 to T2 divided by the weight."[]
is_a: terms:085493 ! terms_C85493

[Term]
id: terms:092316
name: AUC Infinity Obs Norm by BMI
def: "The area under the curve (AUC) extrapolated to infinity, calculated using the observed value of the last non-zero concentration, divided by the body mass index."[]
is_a: terms:085493 ! terms_C85493

[Term]
id: terms:092317
name: AUC Infinity Obs Norm by SA
def: "The area under the curve (AUC) extrapolated to infinity, calculated using the observed value of the last non-zero concentration, divided by the surface area."[]
is_a: terms:085493 ! terms_C85493

[Term]
id: terms:092318
name: AUC Infinity Obs Norm by WT
def: "The area under the curve (AUC) extrapolated to infinity, calculated using the observed value of the last non-zero concentration, divided by the weight."[]
is_a: terms:085493 ! terms_C85493

[Term]
id: terms:092319
name: AUC Infinity Pred Norm by BMI
def: "The area under the curve (AUC) extrapolated to infinity, calculated using the predicted value of the last non-zero concentration, divided by the body mass index."[]
is_a: terms:085493 ! terms_C85493

[Term]
id: terms:092320
name: AUC Infinity Pred Norm by SA
def: "The area under the curve (AUC) extrapolated to infinity, calculated using the predicted value of the last non-zero concentration, divided by the surface area."[]
is_a: terms:085493 ! terms_C85493

[Term]
id: terms:092321
name: AUC Infinity Pred Norm by WT
def: "The area under the curve (AUC) extrapolated to infinity, calculated using the predicted value of the last non-zero concentration, divided by the weight."[]
is_a: terms:085493 ! terms_C85493

[Term]
id: terms:092322
name: AUC Over Dosing Interval Norm by BMI
def: "The area under the curve (AUC) for the defined interval between doses (TAU) divided by the body mass index."[]
is_a: terms:085493 ! terms_C85493

[Term]
id: terms:092323
name: AUC Over Dosing Interval Norm by Dose
def: "The area under the curve (AUC) for the defined interval between doses (TAU) divided by the dose."[]
is_a: terms:085493 ! terms_C85493

[Term]
id: terms:092324
name: AUC Over Dosing Interval Norm by SA
def: "The area under the curve (AUC) for the defined interval between doses (TAU) divided by the surface area."[]
is_a: terms:085493 ! terms_C85493

[Term]
id: terms:092325
name: AUC Over Dosing Interval Norm by WT
def: "The area under the curve (AUC) for the defined interval between doses (TAU) divided by the weight."[]
is_a: terms:085493 ! terms_C85493

[Term]
id: terms:092326
name: AUMC to Last Nonzero Conc Norm by BMI
def: "The area under the moment curve (AUMC) from the time of dosing to the last measurable concentration divided by the body mass index."[]
is_a: terms:085493 ! terms_C85493

[Term]
id: terms:092327
name: AUMC to Last Nonzero Conc Norm by Dose
def: "The area under the moment curve (AUMC) from the time of dosing to the last measurable concentration divided by the dose."[]
is_a: terms:085493 ! terms_C85493

[Term]
id: terms:092328
name: AUMC to Last Nonzero Conc Norm by SA
def: "The area under the moment curve (AUMC) from the time of dosing to the last measurable concentration divided by the surface area."[]
is_a: terms:085493 ! terms_C85493

[Term]
id: terms:092329
name: AUMC to Last Nonzero Conc Norm by WT
def: "The area under the moment curve (AUMC) from the time of dosing to the last measurable concentration divided by the weight."[]
is_a: terms:085493 ! terms_C85493

[Term]
id: terms:092330
name: AUMC Infinity Obs Norm by BMI
def: "The area under the moment curve (AUMC) extrapolated to infinity, calculated using the observed value of the last non-zero concentration, divided by the body mass index."[]
is_a: terms:085493 ! terms_C85493

[Term]
id: terms:092331
name: AUMC Infinity Obs Norm by Dose
def: "The area under the moment curve (AUMC) extrapolated to infinity, calculated using the observed value of the last non-zero concentration, divided by the dose."[]
is_a: terms:085493 ! terms_C85493

[Term]
id: terms:092332
name: AUMC Infinity Obs Norm by SA
def: "The area under the moment curve (AUMC) extrapolated to infinity, calculated using the observed value of the last non-zero concentration, divided by the surface area."[]
is_a: terms:085493 ! terms_C85493

[Term]
id: terms:092333
name: AUMC Infinity Obs Norm by WT
def: "The area under the moment curve (AUMC) extrapolated to infinity, calculated using the observed value of the last non-zero concentration, divided by the weight."[]
is_a: terms:085493 ! terms_C85493

[Term]
id: terms:092334
name: AUMC Infinity Pred Norm by BMI
def: "The area under the moment curve (AUMC) extrapolated to infinity, calculated using the predicted value of the last non-zero concentration, divided by the body mass index."[]
is_a: terms:085493 ! terms_C85493

[Term]
id: terms:092335
name: AUMC Infinity Pred Norm by Dose
def: "The area under the moment curve (AUMC) extrapolated to infinity, calculated using the predicted value of the last non-zero concentration, divided by the dose."[]
is_a: terms:085493 ! terms_C85493

[Term]
id: terms:092336
name: AUMC Infinity Pred Norm by SA
def: "The area under the moment curve (AUMC) extrapolated to infinity, calculated using the predicted value of the last non-zero concentration, divided by the surface area."[]
is_a: terms:085493 ! terms_C85493

[Term]
id: terms:092337
name: AUMC Infinity Pred Norm by WT
def: "The area under the moment curve (AUMC) extrapolated to infinity, calculated using the predicted value of the last non-zero concentration, divided by the weight."[]
is_a: terms:085493 ! terms_C85493

[Term]
id: terms:092338
name: AUMC Over Dosing Interval Norm by BMI
def: "The area under the first moment curve (AUMC) for the defined interval between doses (TAU) divided by the body mass index."[]
is_a: terms:085493 ! terms_C85493

[Term]
id: terms:092339
name: AUMC Over Dosing Interval Norm by Dose
def: "The area under the first moment curve (AUMC) for the defined interval between doses (TAU) divided by the dose."[]
is_a: terms:085493 ! terms_C85493

[Term]
id: terms:092340
name: AUMC Over Dosing Interval Norm by SA
def: "The area under the first moment curve (AUMC) for the defined interval between doses (TAU) divided by the surface area."[]
is_a: terms:085493 ! terms_C85493

[Term]
id: terms:092341
name: AUMC Over Dosing Interval Norm by WT
def: "The area under the first moment curve (AUMC) for the defined interval between doses (TAU) divided by the weight."[]
is_a: terms:085493 ! terms_C85493

[Term]
id: terms:092342
name: AURC All Norm by BMI
def: "The area under the urinary excretion rate curve (AURC) from time zero to the last measurable rate divided by the body mass index."[]
is_a: terms:085493 ! terms_C85493

[Term]
id: terms:092343
name: AURC All Norm by Dose
def: "The area under the urinary excretion rate curve (AURC) from time zero to the last measurable rate divided by the dose."[]
is_a: terms:085493 ! terms_C85493

[Term]
id: terms:092344
name: AURC All Norm by SA
def: "The area under the urinary excretion rate curve (AURC) from time zero to the last measurable rate divided by the surface area."[]
is_a: terms:085493 ! terms_C85493

[Term]
id: terms:092345
name: AURC All Norm by WT
def: "The area under the urinary excretion rate curve (AURC) from time zero to the last measurable rate divided by the weight."[]
is_a: terms:085493 ! terms_C85493

[Term]
id: terms:092346
name: AURC Dosing to Last Conc Norm by BMI
def: "The area under the urinary excretion rate curve (AURC) from time zero to the last measurable rate, divided by the body mass index."[]
is_a: terms:085493 ! terms_C85493

[Term]
id: terms:092347
name: AURC Dosing to Last Conc Norm by Dose
def: "The area under the urinary excretion rate curve (AURC) from time zero to the last measurable rate, divided by the dose."[]
is_a: terms:085493 ! terms_C85493

[Term]
id: terms:092348
name: AURC Dosing to Last Conc Norm by SA
def: "The area under the urinary excretion rate curve (AURC) from time zero to the last measurable rate, divided by the surface area."[]
is_a: terms:085493 ! terms_C85493

[Term]
id: terms:092349
name: AURC Dosing to Last Conc Norm by WT
def: "The area under the urinary excretion rate curve (AURC) from time zero to the last measurable rate, divided by the weight."[]
is_a: terms:085493 ! terms_C85493

[Term]
id: terms:092350
name: AURC from T1 to T2 Norm by BMI
def: "The area under the urinary excretion rate curve (AURC) over the interval from T1 to T2 divided by the body mass index."[]
is_a: terms:085493 ! terms_C85493

[Term]
id: terms:092351
name: AURC from T1 to T2 Norm by Dose
def: "The area under the urinary excretion rate curve (AURC) over the interval from T1 to T2 divided by the dose."[]
is_a: terms:085493 ! terms_C85493

[Term]
id: terms:092352
name: AURC from T1 to T2 Norm by SA
def: "The area under the urinary excretion rate curve (AURC) over the interval from T1 to T2 divided by the surface area."[]
is_a: terms:085493 ! terms_C85493

[Term]
id: terms:092353
name: AURC from T1 to T2 Norm by WT
def: "The area under the urinary excretion rate curve (AURC) over the interval from T1 to T2 divided by the weight."[]
is_a: terms:085493 ! terms_C85493

[Term]
id: terms:092354
name: AURC Infinity Obs Norm by BMI
def: "The area under the urinary excretion rate curve (AURC) extrapolated to infinity, calculated using the observed value of the last excretion rate, divided by the body mass index."[]
is_a: terms:085493 ! terms_C85493

[Term]
id: terms:092355
name: AURC Infinity Obs Norm by Dose
def: "The area under the urinary excretion rate curve (AURC) extrapolated to infinity, calculated using the observed value of the last excretion rate, divided by the dose."[]
is_a: terms:085493 ! terms_C85493

[Term]
id: terms:092356
name: AURC Infinity Obs Norm by SA
def: "The area under the urinary excretion rate curve (AURC) extrapolated to infinity, calculated using the observed value of the last excretion rate, divided by the surface area."[]
is_a: terms:085493 ! terms_C85493

[Term]
id: terms:092357
name: AURC Infinity Obs Norm by WT
def: "The area under the urinary excretion rate curve (AURC) extrapolated to infinity, calculated using the observed value of the last excretion rate, divided by the weight."[]
is_a: terms:085493 ! terms_C85493

[Term]
id: terms:092358
name: AURC Infinity Pred Norm by BMI
def: "The area under the urinary excretion rate curve (AURC) extrapolated to infinity, calculated using the predicted value of the last non-zero excretion rate, divded by the body mass index."[]
is_a: terms:085493 ! terms_C85493

[Term]
id: terms:092359
name: AURC Infinity Pred Norm by Dose
def: "The area under the urinary excretion rate curve (AURC) extrapolated to infinity, calculated using the predicted value of the last non-zero excretion rate, divded by the dose."[]
is_a: terms:085493 ! terms_C85493

[Term]
id: terms:092360
name: AURC Infinity Pred Norm by SA
def: "The area under the urinary excretion rate curve (AURC) extrapolated to infinity, calculated using the predicted value of the last non-zero excretion rate, divded by the surface area."[]
is_a: terms:085493 ! terms_C85493

[Term]
id: terms:092361
name: AURC Infinity Pred Norm by WT
def: "The area under the urinary excretion rate curve (AURC) extrapolated to infinity, calculated using the predicted value of the last non-zero excretion rate, divded by the weight."[]
is_a: terms:085493 ! terms_C85493

[Term]
id: terms:092362
name: AUC All Norm by BMI
def: "The area under the curve (AUC) from the time of dosing to the time of the last observation divided by the body mass index, regardless of whether the last concentration is measurable or not."[]
is_a: terms:085493 ! terms_C85493

[Term]
id: terms:092367
name: Average Conc Norm by BMI
def: "AUCTAU divided by TAU and then divided by the body mass index."[]
is_a: terms:085493 ! terms_C85493

[Term]
id: terms:092368
name: Average Conc Norm by Dose
def: "AUCTAU divided by TAU and then divided by the dose."[]
is_a: terms:085493 ! terms_C85493

[Term]
id: terms:092369
name: Average Conc Norm by SA
def: "AUCTAU divided by TAU and then divided by the surface area."[]
is_a: terms:085493 ! terms_C85493

[Term]
id: terms:092370
name: Average Conc Norm by WT
def: "AUCTAU divided by TAU and then divided by the weight."[]
is_a: terms:085493 ! terms_C85493

[Term]
id: terms:092371
name: Max Conc Norm by BMI
def: "The maximum concentration occurring at Tmax, divided by the body mass index."[]
is_a: terms:085493 ! terms_C85493

[Term]
id: terms:092372
name: Max Conc Norm by SA
def: "The maximum concentration occurring at Tmax, divided by the surface area."[]
is_a: terms:085493 ! terms_C85493

[Term]
id: terms:092373
name: Max Conc Norm by WT
def: "The maximum concentration occurring at Tmax, divided by the weight."[]
is_a: terms:085493 ! terms_C85493

[Term]
id: terms:092374
name: Min Conc Norm by BMI
def: "The minimum concentration between dose time and dose time plus Tau (at Tmin) divided by the body mass index."[]
is_a: terms:085493 ! terms_C85493

[Term]
id: terms:092375
name: Min Conc Norm by Dose
def: "The minimum concentration between dose time and dose time plus Tau (at Tmin) divided by the dose."[]
is_a: terms:085493 ! terms_C85493

[Term]
id: terms:092376
name: Min Conc Norm by SA
def: "The minimum concentration between dose time and dose time plus Tau (at Tmin) divided by the surface area."[]
is_a: terms:085493 ! terms_C85493

[Term]
id: terms:092377
name: Min Conc Norm by WT
def: "The minimum concentration between dose time and dose time plus Tau (at Tmin) divided by the weight."[]
is_a: terms:085493 ! terms_C85493

[Term]
id: terms:092383
name: Initial Conc Norm by BMI
def: "Initial concentration divided by the body mass index. Given only for bolus IV models."[]
is_a: terms:085493 ! terms_C85493

[Term]
id: terms:092384
name: Initial Conc Norm by Dose
def: "Initial concentration divided by the dose. Given only for bolus IV models."[]
is_a: terms:085493 ! terms_C85493

[Term]
id: terms:092385
name: Initial Conc Norm by SA
def: "Initial concentration divided by the surface area. Given only for bolus IV models."[]
is_a: terms:085493 ! terms_C85493

[Term]
id: terms:092386
name: Initial Conc Norm by WT
def: "Initial concentration divided by the weight. Given only for bolus IV models."[]
is_a: terms:085493 ! terms_C85493

[Term]
id: terms:092387
name: Last Nonzero Conc Norm by BMI
def: "The concentration corresponding to Tlast divided by the body mass index."[]
is_a: terms:085493 ! terms_C85493

[Term]
id: terms:092388
name: Last Nonzero Conc Norm by Dose
def: "The concentration corresponding to Tlast divided by the dose."[]
is_a: terms:085493 ! terms_C85493

[Term]
id: terms:092389
name: Last Nonzero Conc Norm by SA
def: "The concentration corresponding to Tlast divided by the surface area."[]
is_a: terms:085493 ! terms_C85493

[Term]
id: terms:092390
name: Last Nonzero Conc Norm by WT
def: "The concentration corresponding to Tlast divided by the weight."[]
is_a: terms:085493 ! terms_C85493

[Term]
id: terms:092391
name: Last Meas Excretion Rate Norm by BMI
def: "The last measurable (positive) excretion rate divided by the body mass index."[]
is_a: terms:085493 ! terms_C85493

[Term]
id: terms:092392
name: Last Meas Excretion Rate Norm by Dose
def: "The last measurable (positive) excretion rate divided by the dose."[]
is_a: terms:085493 ! terms_C85493

[Term]
id: terms:092393
name: Last Meas Excretion Rate Norm by SA
def: "The last measurable (positive) excretion rate divided by the surface area."[]
is_a: terms:085493 ! terms_C85493

[Term]
id: terms:092394
name: Last Meas Excretion Rate Norm by WT
def: "The last measurable (positive) excretion rate divided by the weight."[]
is_a: terms:085493 ! terms_C85493

[Term]
id: terms:092395
name: Max Excretion Rate Norm by BMI
def: "The maximum excretion rate divided by the body mass index."[]
is_a: terms:085493 ! terms_C85493

[Term]
id: terms:092396
name: Max Excretion Rate Norm by Dose
def: "The maximum excretion rate divided by the dose."[]
is_a: terms:085493 ! terms_C85493

[Term]
id: terms:092397
name: Max Excretion Rate Norm by SA
def: "The maximum excretion rate divided by the surface area."[]
is_a: terms:085493 ! terms_C85493

[Term]
id: terms:092398
name: Max Excretion Rate Norm by WT
def: "The maximum excretion rate divided by the weight."[]
is_a: terms:085493 ! terms_C85493

[Term]
id: terms:092399
name: Total CL Obs by F Norm by BMI
def: "The total body clearance for extravascular administration divided by the fraction of dose absorbed, calculated using the observed value of the last non-zero concentration, divided by the body mass index."[]
is_a: terms:085493 ! terms_C85493

[Term]
id: terms:092400
name: Total CL Obs by F Norm by Dose
def: "The total body clearance for extravascular administration divided by the fraction of dose absorbed, calculated using the observed value of the last non-zero concentration, divided by the dose."[]
is_a: terms:085493 ! terms_C85493

[Term]
id: terms:092401
name: Total CL Obs by F Norm by SA
def: "The total body clearance for extravascular administration divided by the fraction of dose absorbed, calculated using the observed value of the last non-zero concentration, divided by the surface area."[]
is_a: terms:085493 ! terms_C85493

[Term]
id: terms:092402
name: Total CL Obs by F Norm by WT
def: "The total body clearance for extravascular administration divided by the fraction of dose absorbed, calculated using the observed value of the last non-zero concentration, divided by the weight."[]
is_a: terms:085493 ! terms_C85493

[Term]
id: terms:092403
name: Total CL Obs Norm by BMI
def: "The total body clearance for intravascular administration, calculated using the observed value of the last non-zero concentration, divided by the body mass index."[]
is_a: terms:085493 ! terms_C85493

[Term]
id: terms:092404
name: Total CL Obs Norm by Dose
def: "The total body clearance for intravascular administration, calculated using the observed value of the last non-zero concentration, divided by the dose."[]
is_a: terms:085493 ! terms_C85493

[Term]
id: terms:092405
name: Total CL Obs Norm by SA
def: "The total body clearance for intravascular administration, calculated using the observed value of the last non-zero concentration, divided by the surface area."[]
is_a: terms:085493 ! terms_C85493

[Term]
id: terms:092406
name: Total CL Obs Norm by WT
def: "The total body clearance for intravascular administration, calculated using the observed value of the last non-zero concentration, divided by the weight."[]
is_a: terms:085493 ! terms_C85493

[Term]
id: terms:092407
name: Vz Obs Norm by BMI
def: "The volume of distribution associated with the terminal slope following intravascular administration, calculated using the observed value of the last non-zero concentration, divided by the body mass index."[]
is_a: terms:085493 ! terms_C85493

[Term]
id: terms:092408
name: Vz Obs Norm by SA
def: "The volume of distribution associated with the terminal slope following intravascular administration, calculated using the observed value of the last non-zero concentration, divided by the surface area."[]
is_a: terms:085493 ! terms_C85493

[Term]
id: terms:092409
name: Vz Obs Norm by WT
def: "The volume of distribution associated with the terminal slope following intravascular administration, calculated using the observed value of the last non-zero concentration, divided by the weight."[]
is_a: terms:085493 ! terms_C85493

[Term]
id: terms:092410
name: Vz Obs by F Norm by BMI
def: "The volume of distribution associated with the terminal slope following extravascular administration divided by the fraction of dose absorbed, calculated using the observed value of the last non-zero concentration, divided by the body mass index."[]
is_a: terms:085493 ! terms_C85493

[Term]
id: terms:092411
name: Vz Obs by F Norm by SA
def: "The volume of distribution associated with the terminal slope following extravascular administration divided by the fraction of dose absorbed, calculated using the observed value of the last non-zero concentration, divided by the surface area."[]
is_a: terms:085493 ! terms_C85493

[Term]
id: terms:092412
name: Vz Obs by F Norm by WT
def: "The volume of distribution associated with the terminal slope following extravascular administration divided by the fraction of dose absorbed, calculated using the observed value of the last non-zero concentration, divided by the weight."[]
is_a: terms:085493 ! terms_C85493

[Term]
id: terms:092417
name: Total CL Pred by F Norm by BMI
def: "The total body clearance for extravascular administration divided by the fraction of dose absorbed, calculated using the predicted value of the last non-zero concentration, divided by body mass index."[]
is_a: terms:085493 ! terms_C85493

[Term]
id: terms:092418
name: Total CL Pred by F Norm by Dose
def: "The total body clearance for extravascular administration divided by the fraction of dose absorbed, calculated using the predicted value of the last non-zero concentration, divided by the dose."[]
is_a: terms:085493 ! terms_C85493

[Term]
id: terms:092419
name: Total CL Pred by F Norm by SA
def: "The total body clearance for extravascular administration divided by the fraction of dose absorbed, calculated using the predicted value of the last non-zero concentration, divided by the surface area."[]
is_a: terms:085493 ! terms_C85493

[Term]
id: terms:092420
name: Total CL Pred by F Norm by WT
def: "The total body clearance for extravascular administration divided by the fraction of dose absorbed, calculated using the predicted value of the last non-zero concentration, divided by the weight."[]
is_a: terms:085493 ! terms_C85493

[Term]
id: terms:092421
name: Total CL Pred Norm by BMI
def: "The total body clearance for intravascular administration, calculated using the predicted value of the last non-zero concentration, divided by the body mass index."[]
is_a: terms:085493 ! terms_C85493

[Term]
id: terms:092422
name: Total CL Pred Norm by Dose
def: "The total body clearance for intravascular administration, calculated using the predicted value of the last non-zero concentration, divided by the dose."[]
is_a: terms:085493 ! terms_C85493

[Term]
id: terms:092423
name: Total CL Pred Norm by SA
def: "The total body clearance for intravascular administration, calculated using the predicted value of the last non-zero concentration, divided by the surface area."[]
is_a: terms:085493 ! terms_C85493

[Term]
id: terms:092424
name: Total CL Pred Norm by WT
def: "The total body clearance for intravascular administration, calculated using the predicted value of the last non-zero concentration, divided by the weight."[]
is_a: terms:085493 ! terms_C85493

[Term]
id: terms:092425
name: Vz Pred Norm by BMI
def: "The volume of distribution associated with the terminal slope following intravascular administration, calculated using the predicted value of the last non-zero concentration, divided by the body mass index."[]
is_a: terms:085493 ! terms_C85493

[Term]
id: terms:092426
name: Vz Pred Norm by SA
def: "The volume of distribution associated with the terminal slope following intravascular administration, calculated using the predicted value of the last non-zero concentration, divided by the surface area."[]
is_a: terms:085493 ! terms_C85493

[Term]
id: terms:092427
name: Vz Pred Norm by WT
def: "The volume of distribution associated with the terminal slope following intravascular administration, calculated using the predicted value of the last non-zero concentration, divided by the weight."[]
is_a: terms:085493 ! terms_C85493

[Term]
id: terms:092428
name: Vz Pred by F Norm by BMI
def: "The volume of distribution associated with the terminal slope following extravascular administration divided by the fraction of dose absorbed, calculated using the predicted value of the last non-zero concentration, divided by the body mass index."[]
is_a: terms:085493 ! terms_C85493

[Term]
id: terms:092429
name: Vz Pred by F Norm by SA
def: "The volume of distribution associated with the terminal slope following extravascular administration divided by the fraction of dose absorbed, calculated using the predicted value of the last non-zero concentration, divided by the surface area."[]
is_a: terms:085493 ! terms_C85493

[Term]
id: terms:092430
name: Vz Pred by F Norm by WT
def: "The volume of distribution associated with the terminal slope following extravascular administration divided by the fraction of dose absorbed, calculated using the predicted value of the last non-zero concentration, divided by the weight."[]
is_a: terms:085493 ! terms_C85493

[Term]
id: terms:095007
name: Effective Half-Life
def: "The drug half-life that quantifies the accumulation ratio of a drug following multiple dosing."[]
is_a: terms:085493 ! terms_C85493

[Term]
id: terms:096695
name: AUC Infinity Obs Norm by Dose
def: "The area under the curve (AUC) extrapolated to infinity, calculated using the observed value of the last non-zero concentration, divided by the dose."[]
is_a: terms:085493 ! terms_C85493

[Term]
id: terms:0KPARM:2000307
name: Concentration at t=0
def: "Concentration of analyte prior to dosing at T=0 (observed or extrapolated)"[]
is_a: terms:085493 ! terms_C85493

[Term]
id: terms:0KPARM:2000309
name: Concentration at T=24hr
def: "concentration of analyte at 24 hours post administration. For a qd dosing regimen this term corresponds to c trough (not at ss)"[]
is_a: terms:085493 ! terms_C85493

[Term]
id: terms:0KPARM:2000311
name: AUC all, unbound
def: "The area under the curve (AUC) from the time of dosing to the time of the last observation, regardless of whether the last concentration is measurable or not. Calculation based on free (unbound) concentrations of analyte"[]
is_a: terms:085493 ! terms_C85493

[Term]
id: terms:0KPARM:2000313
name: AUC ratio male/female
def: "The area under the curve (AUC) from the time of dosing to the time of the last observation, regardless of whether the last concentration is measurable or not. AUCs compared between males and females"[]
is_a: terms:085493 ! terms_C85493

[Term]
id: terms:0KPARM:2000315
name: exposure
def: "The ratio (male/female) of time of maximum observed concentration sampled during a dosing interval"[]
is_a: terms:085493 ! terms_C85493

[Term]
id: terms:0KPARM:2000317
name: time of sampling
def: "time of sampling from plasma or tissue after dosing"[]
is_a: terms:085493 ! terms_C85493

[Term]
id: terms:0KPARM:2000319
name: Dose
def: "administered dose (mg/kg) irrespective of route of administration"[]
is_a: terms:085493 ! terms_C85493

[Term]
id: terms:0KPARM:2000321
name: renal excretion
def: "Amount of drug related material excreted renally (urine) relative to administered dose"[]
is_a: terms:085493 ! terms_C85493

[Term]
id: terms:0KPARM:2000323
name: Exposure ratio drug/ metabolite
def: "The area under the curve (AUC) for parent drug vs a given metabolite from the time of dosing to the time of the last observation, regardless of whether the last concentration is measurable or not"[]
is_a: terms:085493 ! terms_C85493

[Term]
id: terms:0KPARM:2000325
name: tissue/plasma ratio
def: "concentration ratio for any given tissue and plasma at given time point or at tmax"[]
is_a: terms:085493 ! terms_C85493

[Term]
id: terms:0KPARM:2000327
name: bioavailability
def: "Dose normalized exposure ratio of drug as calculated by AUC obtained after dosing via a particular route (oral, inhalation, nasal, etc.) divided by observed AUC after respective iv administration"[]
is_a: terms:085493 ! terms_C85493

[Term]
id: terms:0KPARM:2000559
name: Cmax ratio male/female
def: "The ratio of the maximal concentrations as observed in the concentration-time profile for males versus females"[]
is_a: terms:085493 ! terms_C85493

[Term]
id: terms:0KPARM:2000729
name: tissue concentration
def: "Concentration of an analyte in a tissue other then blood or plsama"[]
is_a: terms:085493 ! terms_C85493

[Term]
id: terms:0KPARM:2000731
name: Tissue Cmax
def: "Maximun concentration as observed in a tiisue (not blood, plasma, serum)"[]
is_a: terms:085493 ! terms_C85493

[Term]
id: terms:0KPARM:2000733
name: Tissue AUC
def: "The area below the time-concentration profile as observed in a tissue between t1 and t2"[]
is_a: terms:085493 ! terms_C85493

