format-version: 1.2
data-version: 1
date: 29:01:2018 01:11
auto-generated-by: OntoBrowser Export Service

[Term]
id: terms:066732
name: terms_C66732

[Term]
id: terms:016576
name: F
def: "A person who belongs to the sex that normally produces ova. The term is used to indicate biological sex distinctions, or cultural gender role distinctions, or both. (NCI)"[]
is_a: terms:066732 ! terms_C66732

[Term]
id: terms:020197
name: M
def: "A person who belongs to the sex that normally produces sperm. The term is used to indicate biological sex distinctions, cultural gender role distinctions, or both. (NCI)"[]
is_a: terms:066732 ! terms_C66732

[Term]
id: terms:049636
name: BOTH
def: "One and the other; relating to or being two in conjunction. (NCI)"[]
is_a: terms:066732 ! terms_C66732

