format-version: 1.2
data-version: 1
date: 29:01:2018 01:11
auto-generated-by: OntoBrowser Export Service

[Term]
id: terms:077808
name: terms_C77808

[Term]
id: terms:014191
name: CAT
def: "The domestic cat, Felis catus. (NCI)"[]
is_a: terms:077808 ! terms_C77808

[Term]
id: terms:014192
name: BOVINE
def: "The domesticated ungulates, Bos primigenius taurus and Bos primigenius indicus."[]
is_a: terms:077808 ! terms_C77808

[Term]
id: terms:014193
name: CHICKEN
def: "The common domestic fowl, Gallus gallus. (NCI)"[]
is_a: terms:077808 ! terms_C77808

[Term]
id: terms:014201
name: DOG
def: "The domestic dog, Canis familiaris. (NCI)"[]
synonym: "Dog" EXACT [VX]
synonym: "Dogs" EXACT [VX]
is_a: terms:077808 ! terms_C77808

[Term]
id: terms:014207
name: FISH
def: "Any jawed or jawless organisms in the phylum Chordata including the jawless fish, armored fish, cartilaginous fish, ray-finned fish and lobe-finned fish."[]
is_a: terms:077808 ! terms_C77808

[Term]
id: terms:014210
name: GOAT
def: "Any one of several species in the genus Capra, most commonly Capra hircus."[]
is_a: terms:077808 ! terms_C77808

[Term]
id: terms:014211
name: GUINEA PIG
def: "The domesticated guinea pig, Cavia porcellus. (NCI)"[]
is_a: terms:077808 ! terms_C77808

[Term]
id: terms:014212
name: HAMSTER
def: "Any member of the subfamily cricetinae and the genuses Mesocricetus, Phodopus, Cricetus, Cricetulus, Allocricetulus, Cansumys and Tscherskia."[]
is_a: terms:077808 ! terms_C77808

[Term]
id: terms:014222
name: HORSE
def: "The domestic horse, Equus caballus. (NCI)"[]
is_a: terms:077808 ! terms_C77808

[Term]
id: terms:014238
name: MOUSE
def: "Any of numerous species of small rodents belonging to the genus Mus and various related genera of the family Muridae. (NCI)"[]
synonym: "Mouse" EXACT [VX]
synonym: "mouse" EXACT [VX]
is_a: terms:077808 ! terms_C77808

[Term]
id: terms:014243
name: MONKEY
def: "Any haplorhine primate not belonging to the family Tarsiidae, Hylobatidae, Pongidae, or Hominidae; this does not correspond to any taxon. This group is divided into Old World monkeys (Cercopithecidae) and New World monkeys (Callitrichidae and Cebidae)."[]
synonym: "Cynomolgus" NARROW [VX]
synonym: "Cynomolgus monkey" NARROW [VX]
synonym: "Cynomolgus monkeys" NARROW [VX]
synonym: "Macaca" NARROW [VX]
synonym: "Macaca fascicularis" NARROW [VX]
synonym: "Monkey" EXACT [VX]
synonym: "Monkey (Macaca mulatta)" NARROW [VX]
synonym: "Monkey cynomolgus" NARROW [VX]
synonym: "Monkey Â¿ynomolgus" NARROW [VX]
synonym: "Monkeys" EXACT [VX]
synonym: "Monkeys (Macaca fascicularis)" NARROW [VX]
synonym: "Primate" EXACT [VX]
synonym: "Rhesus monkey" NARROW [VX]
is_a: terms:077808 ! terms_C77808

[Term]
id: terms:014252
name: BABOON
def: "Multiple species of large terrestrial monkeys in the genus Papio, including P. hamadryas, P. papio, P. anubis, P. cynocephalus and P. ursinus."[]
is_a: terms:077808 ! terms_C77808

[Term]
id: terms:014264
name: RABBIT
def: "Various members of the family Leporidae, especially those of the genus Sylvilagus. (NCI)"[]
is_a: terms:077808 ! terms_C77808

[Term]
id: terms:014265
name: FROG
def: "An amphibian in the order Anura, which includes the toads. (NCI)"[]
is_a: terms:077808 ! terms_C77808

[Term]
id: terms:014266
name: RAT
def: "Any of numerous species of rodents belonging to the genus Rattus and/or various related genera of the family Muridae."[]
synonym: "Rat" EXACT [VX]
synonym: "Rat Charles River CD" NARROW [VX]
synonym: "Rats" EXACT [VX]
synonym: "Wistar rat" NARROW [VX]
synonym: "Wistar rats" NARROW [VX]
synonym: "rat" EXACT [VX]
is_a: terms:077808 ! terms_C77808

[Term]
id: terms:014273
name: SHEEP
def: "Any one of several species in the genus Ovis, most commonly Ovis aries."[]
is_a: terms:077808 ! terms_C77808

[Term]
id: terms:014280
name: PIG
def: "The domestic pig Sus scrofa domestica. (NCI)"[]
synonym: "Pig" EXACT [VX]
is_a: terms:077808 ! terms_C77808

[Term]
id: terms:014297
name: CHIMPANZEE
def: "The anthropoid ape, Pan troglodytes."[]
is_a: terms:077808 ! terms_C77808

[Term]
id: terms:0200004
name: UNASSIGNED
def: "Species has not yet been assigned."[]
is_a: terms:077808 ! terms_C77808

[Term]
id: terms:0200005
name: UNKNOWN
def: "Species is unknown."[]
is_a: terms:077808 ! terms_C77808

[Term]
id: terms:077097
name: FERRET
def: "The common domestic mammal, Mustela putorious."[]
is_a: terms:077808 ! terms_C77808

[Term]
id: terms:077115
name: MARMOSET
def: "The common marmoset, Callithrix jacchus."[]
synonym: "Marmosets" EXACT [VX]
is_a: terms:077808 ! terms_C77808

[Term]
id: terms:077807
name: GERBIL
def: "Any of the small mammals belonging to the Gerbillinae subfamily."[]
is_a: terms:077808 ! terms_C77808

[Term]
id: terms:091812
name: PIGEON
def: "A member of the Columbidae family of birds, most commonly referring to the species Columba livia."[]
is_a: terms:077808 ! terms_C77808

[Term]
id: terms:091813
name: QUAIL
def: "A member of the Phasianidae family of pheasants that includes several genera, including Cotumix, Anurophasis, Perdicula and Ophrysia."[]
is_a: terms:077808 ! terms_C77808

[Term]
id: terms:091815
name: CHINCHILLA
def: "A member of the Chinchillidae family of crepuscular rodents."[]
is_a: terms:077808 ! terms_C77808

[Term]
id: terms:091816
name: MASTOMYS
def: "A genus of rodent in the family muridae."[]
is_a: terms:077808 ! terms_C77808

