format-version: 1.2
data-version: 1
date: 29:01:2018 01:11
auto-generated-by: OntoBrowser Export Service

[Term]
id: terms:085493
name: terms_C85493

[Term]
id: terms:0102356
name: Accumulation Ratio AUCTAU
def: "The area under the curve (AUCTAU) at steady state divided by the area under the curve (AUCTAU) over the initial dosing interval."[]
synonym: "AI (Day90/Day1)" RELATED [VX]
synonym: "ARAUC" EXACT [SEND]
synonym: "AUC ratio" RELATED [VX]
synonym: "AUC(0-24) accumulation ratio" EXACT [VX]
synonym: "AUC(0-24)ss" RELATED [VX]
synonym: "AUC(0-24h)(Day 15/Day 1)" RELATED [VX]
synonym: "AUC(0-42)" RELATED [VX]
synonym: "AUC(0-8/24)" RELATED [VX]
synonym: "AUC(0-8/24) (AZ13263197)" RELATED [VX]
synonym: "AUC(0.0833-24h) (Day 15/Day 1)" RELATED [VX]
synonym: "AUC(0.0833-24h) (Day 17/Day 1)" RELATED [VX]
synonym: "AUC(Day 14/Day 0)" RELATED [VX]
synonym: "AUC(Day 21/Day 0)" RELATED [VX]
synonym: "AUC(Day 28)/AUC(Day 0)" RELATED [VX]
synonym: "AUC(day 28)/AUC(Day 0)" RELATED [VX]
synonym: "AUC*" EXACT [VX]
synonym: "AUCday14/AUCday0" RELATED [VX]
synonym: "Accumulation factor Day 7/Day 1" RELATED [VX]
synonym: "Accumulation factors (AUC)" EXACT [VX]
synonym: "Accumulation index" RELATED [VX]
synonym: "Accumulation ratio (AUC24 on Day 8/AUC24 on Day 1)" RELATED [VX]
synonym: "Accumulation ratio for AUC24 (RacAUC(24)d28/d1)" RELATED [VX]
synonym: "Accumulation ratios (AUC)" EXACT [VX]
synonym: "Composite AUC(0-24h)" RELATED [VX]
synonym: "Linearity AUC" RELATED [VX]
synonym: "MR-2 (AUC(0-24)_(BAY 43-9006)/AUC(24)_(BAY 67-3472)" RELATED [VX]
synonym: "R A3 (AUC_Day 30/AUC_Day 1" RELATED [VX]
synonym: "RA1" RELATED [VX]
synonym: "RA3" RELATED [VX]
synonym: "Ra1" RELATED [VX]
synonym: "Ra2" RELATED [VX]
synonym: "Ra3" RELATED [VX]
synonym: "Rac" RELATED [VX]
synonym: "Rac ( AUC 24 Day7/Day1)" RELATED [VX]
synonym: "Rac (AUC 24 day7/AUC 24 day1)" RELATED [VX]
synonym: "Rac (AUC)" RELATED [VX]
synonym: "Rac (AUC24 Day 7 / AUC24 Day 1)" RELATED [VX]
synonym: "Rac (AUC24 on Day 8/AUC24 on Day 1)" RELATED [VX]
synonym: "Rac (AUC24Day7/AUC24Day1)" RELATED [VX]
synonym: "Rac (Day 7/ Day 1)" RELATED [VX]
synonym: "Rac (day1/day7)" RELATED [VX]
synonym: "Rac (day7/day1)" RELATED [VX]
synonym: "Rac: AUC24 on Day 7/ AUC24 on Day 1" RELATED [VX]
is_a: terms:085493 ! terms_C85493

[Term]
id: terms:0102357
name: Accumulation Ratio Cmax
def: "The maximum concentration at steady state divided by the maximum concentration during the initial dosing interval."[]
synonym: "Accumulation Ratio (C24h)" RELATED [VX]
synonym: "Accumulation factor(Cmax)" RELATED [VX]
synonym: "Accumulation ratio [Cmax Day7/Cmax Day1] (R Cmax)" RELATED [VX]
synonym: "Accumulation ratio [Cmax Day7/Day1]" RELATED [VX]
synonym: "Accumulation ratio calculated from  dried blood spot data Cmax" RELATED [VX]
synonym: "Accumulation ratio of Cmax (Rac(Cmax))" RELATED [VX]
synonym: "C max D28/D1" RELATED [VX]
synonym: "Cmax (Day 15/Day 1)" RELATED [VX]
synonym: "Cmax (Day 17/Day 1)" RELATED [VX]
synonym: "Cmax (mean Day1/Day5)" RELATED [VX]
synonym: "Cmax ratio" RELATED [VX]
synonym: "Cmax ratio Day7/Day1" RELATED [VX]
synonym: "Cmax ratio [Cmax(Day24)/Cmax(Day1)] (RCmax)" RELATED [VX]
synonym: "Cmax(Day 14/Day 0)" RELATED [VX]
synonym: "Cmax(Day 15/Day 1)" RELATED [VX]
synonym: "Cmax(Day 21/Day 0)" RELATED [VX]
synonym: "Cmax(Day 28)/Cmax(Day 0)" RELATED [VX]
synonym: "Cmax(day 28)/Cmax(Day 0)" RELATED [VX]
synonym: "Cmax/dose ratio" RELATED [VX]
synonym: "Cmax2/Cmax1" RELATED [VX]
synonym: "Linearity Cmax" RELATED [VX]
synonym: "R A1 (Cmax_Day 30/C max_Day 1" RELATED [VX]
synonym: "Rac  Cmax" RELATED [VX]
synonym: "Rac (Cmax)" RELATED [VX]
synonym: "Rac(Cmax)" RELATED [VX]
is_a: terms:085493 ! terms_C85493

[Term]
id: terms:0102358
name: Accumulation Ratio Cmin
def: "The minimum concentration at steady state divided by the minimum concentration during the initial dosing interval."[]
synonym: "Accumulation factors (C24h)" RELATED [VX]
synonym: "Accumulation ratio for C5min (R C5min )" RELATED [VX]
synonym: "Accumulation ratios (C24h)" RELATED [VX]
synonym: "C min" RELATED [VX]
is_a: terms:085493 ! terms_C85493

[Term]
id: terms:0102359
name: Amt Rec from T1 to T2
def: "The cumulative amount recovered from the specimen type specified in PPSPEC over the interval from T1 to T2."[]
is_a: terms:085493 ! terms_C85493

[Term]
id: terms:0102360
name: Amt Rec from T1 to T2 Norm by BMI
def: "The cumulative amount recovered from the specimen type specified in PPSPEC over the interval from T1 to T2 divided by body mass index."[]
is_a: terms:085493 ! terms_C85493

[Term]
id: terms:0102361
name: Amt Rec from T1 to T2 Norm by SA
def: "The cumulative amount recovered from the specimen type specified in PPSPEC over the interval from T1 to T2 divided by surface area."[]
is_a: terms:085493 ! terms_C85493

[Term]
id: terms:0102362
name: Amt Rec from T1 to T2 Norm by WT
def: "The cumulative amount recovered from the specimen type specified in PPSPEC over the interval from T1 to T2 divided by weight."[]
is_a: terms:085493 ! terms_C85493

[Term]
id: terms:0102363
name: Amt Rec Over Dosing Interval
def: "The cumulative amount recovered from the specimen type specified in PPSPEC between doses (TAU)."[]
is_a: terms:085493 ! terms_C85493

[Term]
id: terms:0102364
name: Amt Rec Over Dosing Interval Norm by BMI
def: "The cumulative amount recovered from the specimen type specified in PPSPEC between doses (TAU) divided by body mass index."[]
is_a: terms:085493 ! terms_C85493

[Term]
id: terms:0102365
name: Amt Rec Over Dosing Interval Norm by SA
def: "The cumulative amount recovered from the specimen type specified in PPSPEC between doses (TAU) divided by surface area."[]
is_a: terms:085493 ! terms_C85493

[Term]
id: terms:0102366
name: Amt Rec Over Dosing Interval Norm by WT
def: "The cumulative amount recovered from the specimen type specified in PPSPEC between doses (TAU) divided by weight."[]
is_a: terms:085493 ! terms_C85493

[Term]
id: terms:0102367
name: Conc by BMI
def: "The concentration divided by body mass index."[]
is_a: terms:085493 ! terms_C85493

[Term]
id: terms:0102368
name: Conc by Dose
def: "The concentration divided by dose."[]
synonym: "CONCD" EXACT [SEND]
synonym: "Css^a/Dose" RELATED [VX]
synonym: "Mean lymph node concetration/dose (Cmean/dose)" RELATED [VX]
synonym: "Mean plasma concentration dose-normalized" RELATED [VX]
synonym: "Mean spleen concetration/dose (Cmean/dose)" RELATED [VX]
synonym: "Mean thymus concetration/dose (Cmean/dose)" RELATED [VX]
synonym: "Normalized concentration" RELATED [VX]
synonym: "Normalized plasma concentrations" RELATED [VX]
is_a: terms:085493 ! terms_C85493

[Term]
id: terms:0102369
name: Conc by SA
def: "The concentration divided by surface area."[]
is_a: terms:085493 ! terms_C85493

[Term]
id: terms:0102370
name: Conc by WT
def: "The concentration divided by weight."[]
is_a: terms:085493 ! terms_C85493

[Term]
id: terms:0102371
name: Vol Dist Initial
def: "The initial volume of distribution for a substance administered by bolus intravascular dosing."[]
synonym: "Vd" RELATED [VX]
is_a: terms:085493 ! terms_C85493

[Term]
id: terms:0102372
name: Vol Dist Initial Norm by BMI
def: "The initial volume of distribution for a substance administered by bolus intravascular dosing divided by the body mass index."[]
is_a: terms:085493 ! terms_C85493

[Term]
id: terms:0102373
name: Vol Dist Initial Norm by Dose
def: "The initial volume of distribution for a substance administered by bolus intravascular dosing divided by the dose."[]
is_a: terms:085493 ! terms_C85493

[Term]
id: terms:0102374
name: Vol Dist Initial Norm by SA
def: "The initial volume of distribution for a substance administered by bolus intravascular dosing divided by the surface area."[]
is_a: terms:085493 ! terms_C85493

[Term]
id: terms:0102375
name: Vol Dist Initial Norm by WT
def: "The initial volume of distribution for a substance administered by bolus intravascular dosing divided by the weight."[]
is_a: terms:085493 ! terms_C85493

[Term]
id: terms:0102376
name: Nonrenal CL
def: "The total clearance of a substance from the blood less the renal clearance."[]
is_a: terms:085493 ! terms_C85493

[Term]
id: terms:0102377
name: Vol Dist Steady State Obs Norm by BMI
def: "The volume of distribution at steady state based on the observed CLST for a substance administered by intravascular dosing divided by the body mass index."[]
is_a: terms:085493 ! terms_C85493

[Term]
id: terms:0102378
name: Vol Dist Steady State Obs Norm by Dose
def: "The volume of distribution at steady state based on the observed CLST for a substance administered by intravascular dosing divided by the dose."[]
is_a: terms:085493 ! terms_C85493

[Term]
id: terms:0102379
name: Vol Dist Steady State Obs Norm by SA
def: "The volume of distribution at steady state based on the observed CLST for a substance administered by intravascular dosing divided by the surface area."[]
is_a: terms:085493 ! terms_C85493

[Term]
id: terms:0102380
name: Vol Dist Steady State Obs Norm by WT
def: "The volume of distribution at steady state based on the observed CLST for a substance administered by intravascular dosing divided by the weight."[]
is_a: terms:085493 ! terms_C85493

[Term]
id: terms:0102381
name: Peak Trough Ratio
def: "The maximum concentration during a dosing interval divided by the concentration at the end of the dosing interval."[]
synonym: "C24/Cmax" RELATED [VX]
synonym: "Cmin/Cmax" RELATED [VX]
synonym: "PTROUGHR" EXACT [SEND]
is_a: terms:085493 ! terms_C85493

[Term]
id: terms:0102382
name: Pct Rec from T1 to T2
def: "The percentage of the administered dose that is recovered from the specimen type specified in PPSPEC, over the interval between T1 and T2."[]
is_a: terms:085493 ! terms_C85493

[Term]
id: terms:0102383
name: Pct Rec from T1 to T2 Norm by BMI
def: "The percentage of the administered dose that is recovered from the specimen type specified in PPSPEC, over the interval between T1 and T2 divided by body mass index."[]
is_a: terms:085493 ! terms_C85493

[Term]
id: terms:0102384
name: Pct Rec from T1 to T2 Norm by SA
def: "The percentage of the administered dose that is recovered from the specimen type specified in PPSPEC, over the interval between T1 and T2 divided by surface area."[]
is_a: terms:085493 ! terms_C85493

[Term]
id: terms:0102385
name: Pct Rec from T1 to T2 Norm by WT
def: "The percentage of the administered dose that is recovered from the specimen type specified in PPSPEC, over the interval between T1 and T2 divided by weight."[]
is_a: terms:085493 ! terms_C85493

[Term]
id: terms:0102386
name: Pct Rec Over Dosing Interval
def: "The percentage of the administered dose that is recovered from the specimen type specified in PPSPEC, between doses (TAU)."[]
is_a: terms:085493 ! terms_C85493

[Term]
id: terms:0102387
name: Pct Rec Over Dosing Interval Norm by BMI
def: "The percentage of the administered dose that is recovered from the specimen type specified in PPSPEC, between doses (TAU) divided by the body mass index."[]
is_a: terms:085493 ! terms_C85493

[Term]
id: terms:0102388
name: Pct Rec Over Dosing Interval Norm by SA
def: "The percentage of the administered dose that is recovered from the specimen type specified in PPSPEC, between doses (TAU) divided by surface area."[]
is_a: terms:085493 ! terms_C85493

[Term]
id: terms:0102389
name: Pct Rec Over Dosing Interval Norm by WT
def: "The percentage of the administered dose that is recovered from the specimen type specified in PPSPEC, between doses (TAU) divided by weight."[]
is_a: terms:085493 ! terms_C85493

[Term]
id: terms:0102390
name: Vol Dist Steady State Pred Norm by BMI
def: "The volume of distribution at steady state based on the predicted CLST for a substance administered by intravascular dosing divided by the body mass index."[]
is_a: terms:085493 ! terms_C85493

[Term]
id: terms:0102391
name: Vol Dist Steady State Pred Norm by Dose
def: "The volume of distribution at steady state based on the predicted CLST for a substance administered by intravascular dosing divided by the dose."[]
is_a: terms:085493 ! terms_C85493

[Term]
id: terms:0102392
name: Vol Dist Steady State Pred Norm by SA
def: "The volume of distribution at steady state based on the predicted CLST for a substance administered by intravascular dosing divided by the surface area."[]
is_a: terms:085493 ! terms_C85493

[Term]
id: terms:0102393
name: Vol Dist Steady State Pred Norm by WT
def: "The volume of distribution at steady state based on the predicted CLST for a substance administered by intravascular dosing divided by the weight."[]
is_a: terms:085493 ! terms_C85493

[Term]
id: terms:0102394
name: Conc Trough
def: "Concentration at end of dosing interval."[]
synonym: "Plasma trough level" RELATED [VX]
synonym: "Pre-dose concentration of drug before the second daily dosing (Cmin2)" RELATED [VX]
is_a: terms:085493 ! terms_C85493

[Term]
id: terms:0102395
name: Conc Trough by BMI
def: "The trough concentration divided by body mass index."[]
is_a: terms:085493 ! terms_C85493

[Term]
id: terms:0102396
name: Conc Trough by Dose
def: "The trough concentration divided by dose."[]
is_a: terms:085493 ! terms_C85493

[Term]
id: terms:0102397
name: Conc Trough by SA
def: "The trough concentration divided by surface area."[]
is_a: terms:085493 ! terms_C85493

[Term]
id: terms:0102398
name: Conc Trough by WT
def: "The trough concentration divided by weight."[]
is_a: terms:085493 ! terms_C85493

[Term]
id: terms:0102426
name: Accumulation Ratio Ctrough
def: "The trough concentration at steady state divided by the trough concentration during the initial dosing interval."[]
is_a: terms:085493 ! terms_C85493

[Term]
id: terms:0102683
name: Vz Obs Norm by Dose
def: "The volume of distribution associated with the terminal slope following intravascular administration, calculated using the observed value of the last non-zero concentration, divided by the dose."[]
is_a: terms:085493 ! terms_C85493

[Term]
id: terms:0102696
name: Vz Pred Norm by Dose
def: "The volume of distribution associated with the terminal slope following intravascular administration, calculated using the predicted value of the last non-zero concentration, divided by the dose."[]
is_a: terms:085493 ! terms_C85493

[Term]
id: terms:0102729
name: Vz Obs by F Norm by Dose
def: "The volume of distribution associated with the terminal slope following extravascular administration divided by the fraction of dose absorbed, calculated using the observed value of the last non-zero concentration, divided by the dose."[]
is_a: terms:085493 ! terms_C85493

[Term]
id: terms:0102730
name: Vz Pred by F Norm by Dose
def: "The volume of distribution associated with the terminal slope following extravascular administration divided by the fraction of dose absorbed, calculated using the predicted value of the last non-zero concentration, divided by the dose."[]
is_a: terms:085493 ! terms_C85493

[Term]
id: terms:0105449
name: Excret Rate from T1 to T2
def: "The excretion rate over the interval from T1 to T2, determined for the specimen type specified in PPSPEC."[]
is_a: terms:085493 ! terms_C85493

[Term]
id: terms:0105450
name: Excret Rate from T1 to T2 Norm by BMI
def: "The excretion rate over the interval from T1 to T2 divided by the body mass index, determined for the specimen type specified in PPSPEC."[]
is_a: terms:085493 ! terms_C85493

[Term]
id: terms:0105451
name: Excret Rate from T1 to T2 Norm by Dose
def: "The excretion rate over the interval from T1 to T2 divided by the dose, determined for the specimen type specified in PPSPEC."[]
is_a: terms:085493 ! terms_C85493

[Term]
id: terms:0105452
name: Excret Rate from T1 to T2 Norm by SA
def: "The excretion rate over the interval from T1 to T2 divided by the surface area, determined for the specimen type specified in PPSPEC."[]
is_a: terms:085493 ! terms_C85493

[Term]
id: terms:0105453
name: Excret Rate from T1 to T2 Norm by WT
def: "The excretion rate over the interval from T1 to T2 divided by the weight, determined for the specimen type specified in PPSPEC."[]
is_a: terms:085493 ! terms_C85493

[Term]
id: terms:0105454
name: Nonrenal CL Norm by BMI
def: "The total clearance of a substance from the blood minus the renal clearance divided by the body mass index."[]
is_a: terms:085493 ! terms_C85493

[Term]
id: terms:0105455
name: Nonrenal CL Norm by Dose
def: "The total clearance of a substance from the blood minus the renal clearance divided by the dose."[]
is_a: terms:085493 ! terms_C85493

[Term]
id: terms:0105456
name: Nonrenal CL Norm by SA
def: "The total clearance of a substance from the blood minus the renal clearance divided by the surface area."[]
is_a: terms:085493 ! terms_C85493

[Term]
id: terms:0105457
name: Nonrenal CL Norm by WT
def: "The total clearance of a substance from the blood minus the renal clearance divided by the weight."[]
is_a: terms:085493 ! terms_C85493

[Term]
id: terms:0105458
name: Renal CL Norm by BMI
def: "The clearance of a substance from the blood by the kidneys divided by the body mass index."[]
is_a: terms:085493 ! terms_C85493

[Term]
id: terms:0105459
name: Renal CL Norm by Dose
def: "The clearance of a substance from the blood by the kidneys divided by the dose."[]
is_a: terms:085493 ! terms_C85493

[Term]
id: terms:0105460
name: Renal CL Norm by SA
def: "The clearance of a substance from the blood by the kidneys divided by the surface area."[]
is_a: terms:085493 ! terms_C85493

[Term]
id: terms:0105461
name: Renal CL Norm by WT
def: "The clearance of a substance from the blood by the kidneys divided by the weight."[]
is_a: terms:085493 ! terms_C85493

[Term]
id: terms:0111333
name: Vz for Dose Int
def: "The volume of distribution associated with the terminal slope following intravascular administration, calculated using AUCTAU."[]
is_a: terms:085493 ! terms_C85493

[Term]
id: terms:0111364
name: Vz for Dose Int by F
def: "The volume of distribution associated with the terminal slope following extravascular administration divided by the fraction of dose absorbed, calculated using AUCTAU."[]
is_a: terms:085493 ! terms_C85493

[Term]
id: terms:0111365
name: Vz for Dose Int by F Norm by BMI
def: "The volume of distribution associated with the terminal slope following extravascular administration divided by the fraction of dose absorbed, calculated using AUCTAU, divided by the body mass index."[]
is_a: terms:085493 ! terms_C85493

[Term]
id: terms:0111366
name: Vz for Dose Int by F Norm by Dose
def: "The volume of distribution associated with the terminal slope following extravascular administration divided by the fraction of dose absorbed, calculated using AUCTAU, divided by the dose."[]
synonym: "Vc/f" RELATED [VX]
is_a: terms:085493 ! terms_C85493

[Term]
id: terms:0111367
name: Vz for Dose Int by F Norm by SA
def: "The volume of distribution associated with the terminal slope following extravascular administration divided by the fraction of dose absorbed, calculated using AUCTAU, divided by the surface area."[]
is_a: terms:085493 ! terms_C85493

[Term]
id: terms:0111368
name: Vz for Dose Int by F Norm by WT
def: "The volume of distribution associated with the terminal slope following extravascular administration divided by the fraction of dose absorbed, calculated using AUCTAU, divided by the weight."[]
is_a: terms:085493 ! terms_C85493

[Term]
id: terms:0111369
name: Vz for Dose Int Norm by BMI
def: "The volume of distribution associated with the terminal slope following intravascular administration, calculated using AUCTAU, divided by the body mass index."[]
is_a: terms:085493 ! terms_C85493

[Term]
id: terms:0111370
name: Vz for Dose Int Norm by Dose
def: "The volume of distribution associated with the terminal slope following intravascular administration, calculated using AUCTAU, divided by the dose."[]
is_a: terms:085493 ! terms_C85493

[Term]
id: terms:0111371
name: Vz for Dose Int Norm by SA
def: "The volume of distribution associated with the terminal slope following intravascular administration, calculated using AUCTAU, divided by the surface area."[]
is_a: terms:085493 ! terms_C85493

[Term]
id: terms:0111372
name: Vz for Dose Int Norm by WT
def: "The volume of distribution associated with the terminal slope following intravascular administration, calculated using AUCTAU, divided by the weight."[]
is_a: terms:085493 ! terms_C85493

[Term]
id: terms:0112032
name: Amt Rec Infinity Obs
def: "The cumulative amount recovered from the specimen type specified in PPSPEC extrapolated to infinity, calculated using the observed value of the last non-zero concentration."[]
is_a: terms:085493 ! terms_C85493

[Term]
id: terms:0112033
name: Amt Rec Infinity Pred
def: "The cumulative amount recovered from the specimen type specified in PPSPEC extrapolated to infinity, calculated using the predicted value of the last non-zero concentration."[]
is_a: terms:085493 ! terms_C85493

[Term]
id: terms:0112034
name: Pct Rec Infinity Obs
def: "The percentage of the administered dose that is recovered from the specimen type specified in PPSPEC extrapolated to infinity, calculated using the observed value of the last non-zero concentration."[]
is_a: terms:085493 ! terms_C85493

[Term]
id: terms:0112035
name: Pct Rec Infinity Pred
def: "The percentage of the administered dose that is recovered from the specimen type specified in PPSPEC extrapolated to infinity, calculated using the predicted value of the last non-zero concentration."[]
is_a: terms:085493 ! terms_C85493

[Term]
id: terms:0112223
name: Amt Rec Infinity Obs Norm by BMI
def: "The cumulative amount recovered from the specimen type specified in PPSPEC extrapolated to infinity, calculated using the observed value of the last non-zero concentration, divided by the body mass index."[]
is_a: terms:085493 ! terms_C85493

[Term]
id: terms:0112224
name: Amt Rec Infinity Obs Norm by SA
def: "The cumulative amount recovered from the specimen type specified in PPSPEC extrapolated to infinity, calculated using the observed value of the last non-zero concentration, divided by the surface area."[]
is_a: terms:085493 ! terms_C85493

[Term]
id: terms:0112225
name: Amt Rec Infinity Obs Norm by WT
def: "The cumulative amount recovered from the specimen type specified in PPSPEC extrapolated to infinity, calculated using the observed value of the last non-zero concentration, divided by the weight."[]
is_a: terms:085493 ! terms_C85493

[Term]
id: terms:0112226
name: Amt Rec Infinity Pred Norm by BMI
def: "The cumulative amount recovered from the specimen type specified in PPSPEC extrapolated to infinity, calculated using the predicted value of the last non-zero concentration, divided by the body mass index."[]
is_a: terms:085493 ! terms_C85493

[Term]
id: terms:0112227
name: Amt Rec Infinity Pred Norm by SA
def: "The cumulative amount recovered from the specimen type specified in PPSPEC extrapolated to infinity, calculated using the predicted value of the last non-zero concentration, divided by the surface area."[]
is_a: terms:085493 ! terms_C85493

[Term]
id: terms:0112228
name: Amt Rec Infinity Pred Norm by WT
def: "The cumulative amount recovered from the specimen type specified in PPSPEC extrapolated to infinity, calculated using the predicted value of the last non-zero concentration, divided by the weight."[]
is_a: terms:085493 ! terms_C85493

[Term]
id: terms:0112287
name: Hemodialysis Clearance
def: "The clearance of a substance from the blood during a hemodialysis session."[]
is_a: terms:085493 ! terms_C85493

[Term]
id: terms:0112389
name: Pct Rec Infinity Obs Norm by BMI
def: "The percentage of the administered dose that is recovered from the specimen type specified in PPSPEC extrapolated to infinity, calculated using the observed value of the last non-zero concentration, divided by the body mass index."[]
is_a: terms:085493 ! terms_C85493

[Term]
id: terms:0112390
name: Pct Rec Infinity Obs Norm by SA
def: "The percentage of the administered dose that is recovered from the specimen type specified in PPSPEC extrapolated to infinity, calculated using the observed value of the last non-zero concentration, divided by the surface area."[]
is_a: terms:085493 ! terms_C85493

[Term]
id: terms:0112391
name: Pct Rec Infinity Obs Norm by WT
def: "The percentage of the administered dose that is recovered from the specimen type specified in PPSPEC extrapolated to infinity, calculated using the observed value of the last non-zero concentration, divided by the weight."[]
is_a: terms:085493 ! terms_C85493

[Term]
id: terms:0112392
name: Pct Rec Infinity Pred Norm by BMI
def: "The percentage of the administered dose that is recovered from the specimen type specified in PPSPEC extrapolated to infinity, calculated using the predicted value of the last non-zero concentration, divided by the body mass index."[]
is_a: terms:085493 ! terms_C85493

[Term]
id: terms:0112393
name: Pct Rec Infinity Pred Norm by SA
def: "The percentage of the administered dose that is recovered from the specimen type specified in PPSPEC extrapolated to infinity, calculated using the predicted value of the last non-zero concentration, divided by the surface area."[]
is_a: terms:085493 ! terms_C85493

[Term]
id: terms:0112394
name: Pct Rec Infinity Pred Norm by WT
def: "The percentage of the administered dose that is recovered from the specimen type specified in PPSPEC extrapolated to infinity, calculated using the predicted value of the last non-zero concentration, divided by the weight."[]
is_a: terms:085493 ! terms_C85493

[Term]
id: terms:0114121
name: Total CL by F for Dose Int
def: "The total body clearance for extravascular administration divided by the fraction of dose absorbed, calculated using AUCTAU."[]
is_a: terms:085493 ! terms_C85493

[Term]
id: terms:0114122
name: Total CL for Dose Int
def: "The total body clearance for intravascular administration, calculated using AUCTAU."[]
is_a: terms:085493 ! terms_C85493

[Term]
id: terms:0114226
name: Total CL by F for Dose Int Norm by Dose
def: "The total body clearance for extravascular administration divided by the fraction of dose absorbed, calculated using AUCTAU, divided by the dose."[]
is_a: terms:085493 ! terms_C85493

[Term]
id: terms:0114227
name: Total CL by F for Dose Int Norm by BMI
def: "The total body clearance for extravascular administration divided by the fraction of dose absorbed, calculated using AUCTAU, divided by the body mass index."[]
is_a: terms:085493 ! terms_C85493

[Term]
id: terms:0114228
name: Total CL by F for Dose Int Norm by SA
def: "The total body clearance for extravascular administration divided by the fraction of dose absorbed, calculated using AUCTAU, divided by the surface area."[]
is_a: terms:085493 ! terms_C85493

[Term]
id: terms:0114229
name: Total CL by F for Dose Int Norm by WT
def: "The total body clearance for extravascular administration divided by the fraction of dose absorbed, calculated using AUCTAU, divided by the weight."[]
is_a: terms:085493 ! terms_C85493

[Term]
id: terms:0114230
name: Total CL for Dose Int Norm by Dose
def: "The total body clearance for intravascular administration, calculated using AUCTAU, divided by the dose."[]
is_a: terms:085493 ! terms_C85493

[Term]
id: terms:0114231
name: Total CL for Dose Int Norm by BMI
def: "The total body clearance for intravascular administration, calculated using AUCTAU, divided by the body mass index."[]
is_a: terms:085493 ! terms_C85493

[Term]
id: terms:0114232
name: Total CL for Dose Int Norm by SA
def: "The total body clearance for intravascular administration, calculated using AUCTAU, divided by the surface area."[]
is_a: terms:085493 ! terms_C85493

[Term]
id: terms:0114233
name: Total CL for Dose Int Norm by WT
def: "The total body clearance for intravascular administration, calculated using AUCTAU, divided by the weight."[]
is_a: terms:085493 ! terms_C85493

[Term]
id: terms:0114234
name: Accumulation Index using Lambda z
def: "Predicted accumulation ratio for area under the curve (AUC) calculated using the Lambda z estimated from single dose data."[]
is_a: terms:085493 ! terms_C85493

[Term]
id: terms:0116213
name: Hemodialysis Extraction Ratio
def: "The fractional content of a substance removed from the blood during a hemodialysis session."[]
is_a: terms:085493 ! terms_C85493

[Term]
id: terms:0120723
name: Mean Absorption Time
def: "Mean absorption time of a substance administered by extravascular dosing."[]
is_a: terms:085493 ! terms_C85493

[Term]
id: terms:0120724
name: MRT Extravasc Infinity Obs
def: "The mean residence time (MRT) extrapolated to infinity for a substance administered by extravascular dosing, calculated using the observed value of the last non-zero concentration. Extravascular MRT includes Mean Absorption Time (MAT)."[]
synonym: "MRT_INF" RELATED [VX]
is_a: terms:085493 ! terms_C85493

[Term]
id: terms:0120725
name: MRT Extravasc Infinity Pred
def: "The mean residence time (MRT) extrapolated to infinity for a substance administered by extravascular dosing, calculated using the predicted value of the last non-zero concentration. Extravascular MRT includes Mean Absorption Time (MAT)."[]
is_a: terms:085493 ! terms_C85493

[Term]
id: terms:0120726
name: MRT Extravasc to Last Nonzero Conc
def: "Mean residence time (MRT) from the time of dosing to the time of the last measurable concentration for a substance administered by extravascular dosing. Extravascular MRT includes Mean Absorption Time (MAT)."[]
synonym: "MRTEVLST" EXACT [SEND]
is_a: terms:085493 ! terms_C85493

[Term]
id: terms:0121134
name: MRT Intravasc Infinity Obs
def: "The mean residence time (MRT) extrapolated to infinity for a substance administered by intravascular dosing, calculated using the observed value of the last non-zero concentration."[]
synonym: "MRTIVIFO" EXACT [SEND]
synonym: "MRTlast" RELATED [VX]
synonym: "Mrt" RELATED [VX]
is_a: terms:085493 ! terms_C85493

[Term]
id: terms:0121136
name: MRT Intravasc Infinity Pred
def: "The mean residence time (MRT) extrapolated to infinity for a substance administered by intravascular dosing, calculated using the predicted value of the last non-zero concentration."[]
synonym: "Mean residence time (MRT) (model dependent analysis)" RELATED [VX]
is_a: terms:085493 ! terms_C85493

[Term]
id: terms:0121137
name: MRT Intravasc to Last Nonzero Conc
def: "Mean residence time (MRT) from the time of dosing to the time of the last measurable concentration, for a substance administered by intravascular dosing."[]
synonym: "MRT_LST" RELATED [VX]
is_a: terms:085493 ! terms_C85493

[Term]
id: terms:0122049
name: Renal CL from T1 to T2
def: "The clearance of a substance from the blood by the kidneys over the interval from T1 to T2."[]
is_a: terms:085493 ! terms_C85493

[Term]
id: terms:0122050
name: Renal CL for Dose Int
def: "The clearance of a substance from the blood by the kidneys, calculated using AUCTAU."[]
is_a: terms:085493 ! terms_C85493

[Term]
id: terms:0122329
name: Accumulation Ratio AUC from T1 to T2
def: "The area under the curve from T1 to T2 at steady state divided by the area under the curve from T1 to T2 during the initial dosing interval."[]
synonym: "AI Day 90/Day 1" RELATED [VX]
synonym: "ARAUCINT" EXACT [SEND]
synonym: "AUC 0-24h D28/D1" RELATED [VX]
synonym: "AUC ratio (D155/D1)" RELATED [VX]
synonym: "AUC ratio (D155/D29)" RELATED [VX]
synonym: "AUC ratio (D156/D1)" RELATED [VX]
synonym: "AUC ratio (D156/D31)" RELATED [VX]
synonym: "AUC ratio (D177/D29)" RELATED [VX]
synonym: "AUC ratio (D177/D30)" RELATED [VX]
synonym: "AUC ratio (D29/D1)" RELATED [VX]
synonym: "AUC ratio (D31/D1)" RELATED [VX]
synonym: "AUC ratio between periods R1=AUC(0-24 h) Week 4/ AUC(0-24 h) Week 0" RELATED [VX]
synonym: "AUC ratio between periods R2=AUC(0-24 h) Week 13/ AUC(0-24 h) Week 0" RELATED [VX]
synonym: "AUC ratio between periods R3=AUC(0-24 h) Week 13/ AUC(0-24 h) Week 4" RELATED [VX]
synonym: "AUC ratio between periods R3=AUC(0-24 h) Week 13/ AUC(0-24 h) Week 5" RELATED [VX]
synonym: "AUC ratio between periods R3=AUC(0-24 h) Week 13/ AUC(0-24 h) Week 6" RELATED [VX]
synonym: "AUC(0-24) accumulation ratio (Rac)" RELATED [VX]
synonym: "AUC(0-24) accumulation ratio week13/day1 (Rac)" RELATED [VX]
synonym: "AUC(0-24) accumulation ratio week26/day1 (Rac)" RELATED [VX]
synonym: "AUC(0-24) accumulation ratio week52/day1 (Rac)" RELATED [VX]
synonym: "AUC(24-8)" RELATED [VX]
synonym: "AUC(mean Day1/Day5)" RELATED [VX]
synonym: "AUGm Day 93/AUC0-24 Day 29" RELATED [VX]
synonym: "AUGm Day 93/AUC0-24 Day 30" RELATED [VX]
synonym: "Accum.factor" RELATED [VX]
synonym: "Accumul. ratios" RELATED [VX]
synonym: "Accumulation Ratio" RELATED [VX]
synonym: "Accumulation Ratio (AUC)" RELATED [VX]
synonym: "Accumulation factor" RELATED [VX]
synonym: "Accumulation factor(AUC)" RELATED [VX]
synonym: "Accumulation index [(AUC(0-24h)Day28/AUC(0-24h)Day1] (Rac)" RELATED [VX]
synonym: "Accumulation index [(AUC(0-24h)Week13/AUC(0-24h)Day1] (Rac)" RELATED [VX]
synonym: "Accumulation index [AUC(0-24h)Day24/AUC(0-24h)Day1] (Rac)" RELATED [VX]
synonym: "Accumulation ratio" RELATED [VX]
synonym: "Accumulation ratio (AUC(0-24) on day 14 / AUC(0-24) on day 1) (Rac)" RELATED [VX]
synonym: "Accumulation ratio (AUC(0-24h)Day7/AUC(0-inf)Day1)" RELATED [VX]
synonym: "Accumulation ratio (Rac (AUC) D5/D1)" RELATED [VX]
synonym: "Accumulation ratio (Rac (AUC))" RELATED [VX]
synonym: "Accumulation ratio (Rac (D28/D1))" RELATED [VX]
synonym: "Accumulation ratio (Rac AUC(0-24))" RELATED [VX]
synonym: "Accumulation ratio (Rac(AUC(0-24h)))" RELATED [VX]
synonym: "Accumulation ratio (Rac(D28/D1))" RELATED [VX]
synonym: "Accumulation ratio (Rac)" RELATED [VX]
synonym: "Accumulation ratio [AUC(0-24)Day7/AUC(0-24)Day1] (Rac)" RELATED [VX]
synonym: "Accumulation ratio [AUC(0-24h)Day7/AUC(0-24h)Day1] (Rac(AUC))" RELATED [VX]
synonym: "Accumulation ratio calculated from  dried blood spot data (AUC)" RELATED [VX]
synonym: "Accumulation ratio calculated from  dried blood spot data AUC(0-24)" RELATED [VX]
synonym: "Accumulation ratio expected at day 1 (single dose) (Rac D1)" RELATED [VX]
synonym: "Accumulation ratio for AUC(0-24)" RELATED [VX]
synonym: "Accumulation ratio for C(EOI)" RELATED [VX]
synonym: "Accumulation ratio in blood (Rc)" RELATED [VX]
synonym: "Accumulation ratio of AUC (Rac)" RELATED [VX]
synonym: "Factor of accumulation (Rac)" RELATED [VX]
synonym: "Mean AUC 24 week 13/ mean AUC 24 week 4" RELATED [VX]
synonym: "R ac (AUC 0-24) Day7/Day1" RELATED [VX]
synonym: "Rac (AUC Day8/AUC Day1)" RELATED [VX]
synonym: "Rac (AUC. D8/D1)" RELATED [VX]
synonym: "Rac (AUC24 Day 28 / AUC24 Day 1)" RELATED [VX]
synonym: "Rac (AUC24 on Day 14/AUC24 on Day 1)" RELATED [VX]
synonym: "Rac (AUC24 on Day 28/AUC24 on Day 1)" RELATED [VX]
synonym: "Rac (AUC24 on Day 4/AUC24 on Day 1)" RELATED [VX]
synonym: "Rac (AUCt,day8/AUCt,day1)" RELATED [VX]
synonym: "Rac (Day 29/Day 1)" RELATED [VX]
synonym: "Rac (Day 8/Day 1)" RELATED [VX]
synonym: "Rac AUC (Day 182/Day 86)" RELATED [VX]
synonym: "Rac Day8/Day1" RELATED [VX]
synonym: "Racc (Day 8/Day 1)" RELATED [VX]
synonym: "Ratio of AUC(0-24) from week 4 to day 1 (R(A3))" RELATED [VX]
synonym: "Systemic accumulation factor" RELATED [VX]
is_a: terms:085493 ! terms_C85493

[Term]
id: terms:0122330
name: Renal CL from T1 to T2 Norm by BMI
def: "The clearance of a substance from the blood by the kidneys over the interval from T1 to T2 divided by the body mass index."[]
is_a: terms:085493 ! terms_C85493

[Term]
id: terms:0122331
name: Renal CL from T1 to T2 Norm by Dose
def: "The clearance of a substance from the blood by the kidneys over the interval from T1 to T2 divided by the dose."[]
is_a: terms:085493 ! terms_C85493

[Term]
id: terms:0122332
name: Renal CL from T1 to T2 Norm by SA
def: "The clearance of a substance from the blood by the kidneys over the interval from T1 to T2 divided by the surface area."[]
is_a: terms:085493 ! terms_C85493

[Term]
id: terms:0122333
name: Renal CL from T1 to T2 Norm by WT
def: "The clearance of a substance from the blood by the kidneys over the interval from T1 to T2 divided by the weight."[]
is_a: terms:085493 ! terms_C85493

[Term]
id: terms:0122334
name: Renal CL for Dose Int Norm by BMI
def: "The clearance of a substance from the blood by the kidneys, calculated using AUCTAU, divided by the body mass index."[]
is_a: terms:085493 ! terms_C85493

[Term]
id: terms:0122335
name: Renal CL for Dose Int Norm by Dose
def: "The clearance of a substance from the blood by the kidneys, calculated using AUCTAU, divided by the dose."[]
is_a: terms:085493 ! terms_C85493

[Term]
id: terms:0122336
name: Renal CL for Dose Int Norm by SA
def: "The clearance of a substance from the blood by the kidneys, calculated using AUCTAU, divided by the surface area."[]
is_a: terms:085493 ! terms_C85493

[Term]
id: terms:0122337
name: Renal CL for Dose Int Norm by WT
def: "The clearance of a substance from the blood by the kidneys, calculated using AUCTAU, divided by the weight."[]
is_a: terms:085493 ! terms_C85493

[Term]
id: terms:0122338
name: Stationarity Ratio AUC
def: "The area under the curve (AUCTAU) at steady state divided by the area under the curve extrapolated to infinity for the initial dosing interval."[]
is_a: terms:085493 ! terms_C85493

[Term]
id: terms:0122339
name: Trough Peak Ratio
def: "The concentration at the start of a dosing interval divided by the maximum concentration during the dosing interval."[]
is_a: terms:085493 ! terms_C85493

[Term]
id: terms:0200002
name: Unassigned
def: "PK parameter has not yet been assigned."[]
is_a: terms:085493 ! terms_C85493

[Term]
id: terms:0200003
name: Unknown
def: "PK parameter is unknown."[]
is_a: terms:085493 ! terms_C85493

[Term]
id: terms:041185
name: Concentration
def: "The quantity of a specified substance in a unit volume or weight of another substance."[]
synonym: "Blood concentration" RELATED [VX]
synonym: "Blood concentration after 4th dose" RELATED [VX]
synonym: "Blood concentration pool" RELATED [VX]
synonym: "Blood concentrations" RELATED [VX]
synonym: "Blood concentrations (pigmented rats)" RELATED [VX]
synonym: "Blood level" RELATED [VX]
synonym: "Brain concentration" NARROW [VX]
synonym: "Brain concentrations" RELATED [VX]
synonym: "C" EXACT [VX]
synonym: "C (0-5h)" RELATED [VX]
synonym: "C (1)" RELATED [VX]
synonym: "C (10min)" RELATED [VX]
synonym: "C (8)" RELATED [VX]
synonym: "C 0.25h" RELATED [VX]
synonym: "C 0.5h" RELATED [VX]
synonym: "C 0.67h" RELATED [VX]
synonym: "C 12h" RELATED [VX]
synonym: "C 15min" RELATED [VX]
synonym: "C 1h" RELATED [VX]
synonym: "C 2min" RELATED [VX]
synonym: "C 3h" RELATED [VX]
synonym: "C 4h" RELATED [VX]
synonym: "C EOI" RELATED [VX]
synonym: "C ah" RELATED [VX]
synonym: "C end of infusion" RELATED [VX]
synonym: "C eoi" RELATED [VX]
synonym: "C in brain" RELATED [VX]
synonym: "C inf" RELATED [VX]
synonym: "C mean" RELATED [VX]
synonym: "C of GGA_IRIS_SER041-8" RELATED [VX]
synonym: "C t+8: just before second daily gavage" RELATED [VX]
synonym: "C(1)" RELATED [VX]
synonym: "C(10min)" RELATED [VX]
synonym: "C(120h)" RELATED [VX]
synonym: "C(15 min)" RELATED [VX]
synonym: "C(5min)" RELATED [VX]
synonym: "C(8h)" RELATED [VX]
synonym: "C(end of infusion)" RELATED [VX]
synonym: "C(heart)" RELATED [VX]
synonym: "C(muscle)" RELATED [VX]
synonym: "C(serum)" RELATED [VX]
synonym: "C(t)" RELATED [VX]
synonym: "C0.167" RELATED [VX]
synonym: "C0.17h" RELATED [VX]
synonym: "C0.5 h" RELATED [VX]
synonym: "C1" RELATED [VX]
synonym: "C10h" RELATED [VX]
synonym: "C15min (after the 1st daily infusion)" RELATED [VX]
synonym: "C15min (after the 2nd daily infusion)" RELATED [VX]
synonym: "C1h" RELATED [VX]
synonym: "C24.5h lung" RELATED [VX]
synonym: "C3h" RELATED [VX]
synonym: "C4h" RELATED [VX]
synonym: "C5h" RELATED [VX]
synonym: "C5min" RELATED [VX]
synonym: "C6min" RELATED [VX]
synonym: "CONC" EXACT [SEND]
synonym: "Cblood" RELATED [VX]
synonym: "Cbrain" RELATED [VX]
synonym: "Cend" RELATED [VX]
synonym: "Ceoi" RELATED [VX]
synonym: "Cerebellum concentration" RELATED [VX]
synonym: "Chest skin concentration" RELATED [VX]
synonym: "Cinf" RELATED [VX]
synonym: "Compound levels in serum" RELATED [VX]
synonym: "Conc. RO18-0647" RELATED [VX]
synonym: "Concentration" EXACT [VX]
synonym: "Concentration (cortex)" RELATED [VX]
synonym: "Concentration (liver)" RELATED [VX]
synonym: "Concentration (pelvis)" RELATED [VX]
synonym: "Concentration (urine)" RELATED [VX]
synonym: "Concentration at end of infusion (C(EOI))" RELATED [VX]
synonym: "Concentration in Testes" RELATED [VX]
synonym: "Concentration in Whole Blood" RELATED [VX]
synonym: "Concentration in blood" RELATED [VX]
synonym: "Concentration in brain" RELATED [VX]
synonym: "Concentration in cerebro spinal fluid" RELATED [VX]
synonym: "Concentration in heart tissue" RELATED [VX]
synonym: "Concentration in kidney" RELATED [VX]
synonym: "Concentration in liver" RELATED [VX]
synonym: "Concentration in lung" RELATED [VX]
synonym: "Concentration in lymph nodes" RELATED [VX]
synonym: "Concentration in plasma" NARROW [VX]
synonym: "Concentration in serum" NARROW [VX]
synonym: "Concentration in skin" RELATED [VX]
synonym: "Concentration in testes" RELATED [VX]
synonym: "Concentration in the plasma" RELATED [VX]
synonym: "Concentration in uterine tissue" RELATED [VX]
synonym: "Concentration of proteins (females)" NARROW [VX]
synonym: "Concentration of proteins (males)" NARROW [VX]
synonym: "Concentration of radioactivity in blood" RELATED [VX]
synonym: "Concentration of radioactivity in plasma" RELATED [VX]
synonym: "Concentrations" EXACT [VX]
synonym: "Concentrations in dried blood spot" RELATED [VX]
synonym: "Concentrations in heart" RELATED [VX]
synonym: "Concentrations in plasma" RELATED [VX]
synonym: "Concentrations of AZ12250736 in plasma" RELATED [VX]
synonym: "Cplasma" NARROW [VX]
synonym: "Css" RELATED [VX]
synonym: "Css 8 h" RELATED [VX]
synonym: "Css(C8h)" RELATED [VX]
synonym: "Ct" RELATED [VX]
synonym: "Ctau" RELATED [VX]
synonym: "Determined plasma concentration" RELATED [VX]
synonym: "Diencephalon concentration" RELATED [VX]
synonym: "Ear skin concentration" RELATED [VX]
synonym: "Fat tissue concentration" NARROW [VX]
synonym: "Free plasma concentration" RELATED [VX]
synonym: "Frontal cortex concentration" RELATED [VX]
synonym: "Ganciclovir concentration" RELATED [VX]
synonym: "Geometric plasma level" RELATED [VX]
synonym: "HTF919 Concentration" RELATED [VX]
synonym: "Heart concentration" RELATED [VX]
synonym: "Hypothalamus concentrations" RELATED [VX]
synonym: "Liver concentration" NARROW [VX]
synonym: "Lung concentration" RELATED [VX]
synonym: "Lymph node concentration" NARROW [VX]
synonym: "Mean  plasma concentration" NARROW [VX]
synonym: "Mean blood concentration" NARROW [VX]
synonym: "Mean blood concentrations" NARROW [VX]
synonym: "Mean concentration" NARROW [VX]
synonym: "Mean plasma concentration" NARROW [VX]
synonym: "Mean plasma concentrations" NARROW [VX]
synonym: "Mesn plasma concentrations" NARROW [VX]
synonym: "Mycophenolic acid concentration" RELATED [VX]
synonym: "Mycophenolic acid glucuronide concentration" RELATED [VX]
synonym: "Occipital cortex concentration" RELATED [VX]
synonym: "Pancreas concentration" NARROW [VX]
synonym: "Pasma concentration" NARROW [VX]
synonym: "Perietal cortex concentration" RELATED [VX]
synonym: "Plasma  concentration" NARROW [VX]
synonym: "Plasma Concenteration" RELATED [VX]
synonym: "Plasma Concentration" NARROW [VX]
synonym: "Plasma Concentrations" NARROW [VX]
synonym: "Plasma Glucose concentration" RELATED [VX]
synonym: "Plasma Glucose level" NARROW [VX]
synonym: "Plasma conc." RELATED [VX]
synonym: "Plasma concenteration" RELATED [VX]
synonym: "Plasma concentration" NARROW [VX]
synonym: "Plasma concentration (0 hours during infusion)" RELATED [VX]
synonym: "Plasma concentration (1 hour during infusion)" RELATED [VX]
synonym: "Plasma concentration (10th administration)" RELATED [VX]
synonym: "Plasma concentration (1st administration)" RELATED [VX]
synonym: "Plasma concentration (2 hour during infusion)" RELATED [VX]
synonym: "Plasma concentration (2d administration)" RELATED [VX]
synonym: "Plasma concentration (3 hours during infusion)" RELATED [VX]
synonym: "Plasma concentration (4 hours during infusion)" RELATED [VX]
synonym: "Plasma concentration (9th administration)" RELATED [VX]
synonym: "Plasma concentration (arithmetic)" NARROW [VX]
synonym: "Plasma concentration (exsanguination)" RELATED [VX]
synonym: "Plasma concentration (predose)" NARROW [VX]
synonym: "Plasma concentration (recovery animals)" RELATED [VX]
synonym: "Plasma concentration (subdose)" NARROW [VX]
synonym: "Plasma concentration at the end of infusion" RELATED [VX]
synonym: "Plasma concentration in pups" NARROW [VX]
synonym: "Plasma concentration observed 28 days after dose (C28)" RELATED [VX]
synonym: "Plasma concentration of AR-C90439XX" RELATED [VX]
synonym: "Plasma concentration of AZD1305" RELATED [VX]
synonym: "Plasma concentration predose" NARROW [VX]
synonym: "Plasma concentration( dark)" NARROW [VX]
synonym: "Plasma concentration( light)" NARROW [VX]
synonym: "Plasma concentrations" NARROW [VX]
synonym: "Plasma concentrations of the test compound" RELATED [VX]
synonym: "Plasma concetration" RELATED [VX]
synonym: "Plasma count" RELATED [VX]
synonym: "Plasma level" NARROW [VX]
synonym: "Plasma levels" RELATED [VX]
synonym: "Plasma ultrafiltrate concentration" NARROW [VX]
synonym: "Plasma-ultrafiltrate platinum concentration" RELATED [VX]
synonym: "Plasms concentration" RELATED [VX]
synonym: "Platinum concentration" RELATED [VX]
synonym: "Pool plasma concentration" RELATED [VX]
synonym: "Pooled blood concentration" RELATED [VX]
synonym: "Pooled plasma concentration" RELATED [VX]
synonym: "Repeated dose Blood concentration" RELATED [VX]
synonym: "Salivary gland concentration" NARROW [VX]
synonym: "Serum concentration" NARROW [VX]
synonym: "Serum concentration at steady state" RELATED [VX]
synonym: "Serum concentration, Fasted" RELATED [VX]
synonym: "Serum concentration, Fed" RELATED [VX]
synonym: "Serum concentration. Fasted" RELATED [VX]
synonym: "Serum level" NARROW [VX]
synonym: "Serum levels of the test compound" RELATED [VX]
synonym: "Single dose Blood concentration" RELATED [VX]
synonym: "Striatum concentration" RELATED [VX]
synonym: "Temporal cortex concentration" RELATED [VX]
synonym: "Testes concentration" NARROW [VX]
synonym: "Testes homogenate concentration" RELATED [VX]
synonym: "Testes interstitial fluid concentration" RELATED [VX]
synonym: "The observed concentration at the end of infusion (C inf)" RELATED [VX]
synonym: "Tissue concentration (bone marrow)" RELATED [VX]
synonym: "Tissue concentration (duodenum)" RELATED [VX]
synonym: "Tissue concentration (heart)" RELATED [VX]
synonym: "Tissue concentration (kidney)" RELATED [VX]
synonym: "Tissue concentration (liver)" RELATED [VX]
synonym: "Tissue concentration (skeletal muscle)" RELATED [VX]
synonym: "Tissue concentration(choroid+pigmented epithelium layer)" RELATED [VX]
synonym: "Tissue concentration(retina)" RELATED [VX]
synonym: "Tissue concentrations - skin" RELATED [VX]
synonym: "Total concentration" RELATED [VX]
synonym: "Urine concentration" RELATED [VX]
synonym: "Urine concentration AR-C90441XX" RELATED [VX]
synonym: "Urine concentration of AR-C90439XX" RELATED [VX]
synonym: "Urine concentration of AR-C90441XX" RELATED [VX]
synonym: "Whole blood concentration" RELATED [VX]
synonym: "ZD2486 concentration" RELATED [VX]
synonym: "ZK 152.387-antigen level" RELATED [VX]
synonym: "plasma concentrations" NARROW [VX]
is_a: terms:085493 ! terms_C85493

[Term]
id: terms:070918
name: Max Conc
def: "The maximum concentration occurring at Tmax."[]
synonym: "C high" RELATED [VX]
synonym: "C m a x" RELATED [VX]
synonym: "C max" EXACT [VX]
synonym: "C max (1st treatment)" RELATED [VX]
synonym: "C max (2nd treatment)" RELATED [VX]
synonym: "C max (3rd treatment)" RELATED [VX]
synonym: "C max (brain)" RELATED [VX]
synonym: "C max (liver)" RELATED [VX]
synonym: "C max (plasma)" RELATED [VX]
synonym: "C max 2" RELATED [VX]
synonym: "C max brain" RELATED [VX]
synonym: "C max geometric mean" RELATED [VX]
synonym: "C max liver" RELATED [VX]
synonym: "C max plasma" RELATED [VX]
synonym: "C max1" RELATED [VX]
synonym: "C(max)" EXACT [VX]
synonym: "CMAX" EXACT [SEND]
synonym: "CMAX" EXACT [VX]
synonym: "Camx" RELATED [VX]
synonym: "Cmac" RELATED [VX]
synonym: "Cmax" EXACT [VX]
synonym: "Cmax  (metabolite X)" NARROW [VX]
synonym: "Cmax  in brain" RELATED [VX]
synonym: "Cmax (10th administration)" RELATED [VX]
synonym: "Cmax (1st administration)" RELATED [VX]
synonym: "Cmax (1st dosing)" NARROW [VX]
synonym: "Cmax (2d administration)" RELATED [VX]
synonym: "Cmax (2nd dosing)" NARROW [VX]
synonym: "Cmax (9th administration)" RELATED [VX]
synonym: "Cmax (AVE8324)" NARROW [VX]
synonym: "Cmax (AZ12326299)" NARROW [VX]
synonym: "Cmax (AZ13263197)" NARROW [VX]
synonym: "Cmax (BAY 43-9695 (M1))" NARROW [VX]
synonym: "Cmax (BIIF 1148)" NARROW [VX]
synonym: "Cmax (ICS 205-930)" NARROW [VX]
synonym: "Cmax (Lu 33-108)" NARROW [VX]
synonym: "Cmax (Metabolite CGP 10000)" RELATED [VX]
synonym: "Cmax (Metabolite GP 47680)" RELATED [VX]
synonym: "Cmax (Metabolite ICS-5-0H)" NARROW [VX]
synonym: "Cmax (Metabolite ICS-6-0H)" NARROW [VX]
synonym: "Cmax (N-desmethyl metabolite M594347)" NARROW [VX]
synonym: "Cmax (RU 36384)" NARROW [VX]
synonym: "Cmax (Rat #6 12hr point)" RELATED [VX]
synonym: "Cmax (SB235365)" NARROW [VX]
synonym: "Cmax (SR 121407)" NARROW [VX]
synonym: "Cmax (SSR-epimer)" NARROW [VX]
synonym: "Cmax (Testes)" RELATED [VX]
synonym: "Cmax (Whole Blood)" RELATED [VX]
synonym: "Cmax (ZK 811694)" NARROW [VX]
synonym: "Cmax (acid metabolite)" NARROW [VX]
synonym: "Cmax (after 1st dosing)" NARROW [VX]
synonym: "Cmax (after 2nd dosing)" NARROW [VX]
synonym: "Cmax (concentration of burst)" RELATED [VX]
synonym: "Cmax (dose 1)" RELATED [VX]
synonym: "Cmax (dose 2)" RELATED [VX]
synonym: "Cmax (dose corrected)" NARROW [VX]
synonym: "Cmax (dried blood samples)" RELATED [VX]
synonym: "Cmax (end of infusion)" RELATED [VX]
synonym: "Cmax (geometric)" NARROW [VX]
synonym: "Cmax (lung)" RELATED [VX]
synonym: "Cmax (mean)" NARROW [VX]
synonym: "Cmax (metabolite X)" NARROW [VX]
synonym: "Cmax (metabolite X1)" NARROW [VX]
synonym: "Cmax (metabolite X2)" NARROW [VX]
synonym: "Cmax (metabolite x)" NARROW [VX]
synonym: "Cmax (metabolite)" NARROW [VX]
synonym: "Cmax (multiple dose)" RELATED [VX]
synonym: "Cmax (multiple dose, after 1st daily dose)" NARROW [VX]
synonym: "Cmax (multiple dose, after 2nd daily dose)" NARROW [VX]
synonym: "Cmax (recovery animals)" RELATED [VX]
synonym: "Cmax (single dose)" NARROW [VX]
synonym: "Cmax 1" NARROW [VX]
synonym: "Cmax 1 (2x30umol/kg)" NARROW [VX]
synonym: "Cmax 1 (2x40 umol/kg)" NARROW [VX]
synonym: "Cmax 2" NARROW [VX]
synonym: "Cmax 2 (2x 40 umol/kg)" NARROW [VX]
synonym: "Cmax 2 (2x30 umol/kg)" NARROW [VX]
synonym: "Cmax RDA136" RELATED [VX]
synonym: "Cmax SDA137" RELATED [VX]
synonym: "Cmax TRI476" RELATED [VX]
synonym: "Cmax after 1st dose" RELATED [VX]
synonym: "Cmax after 2d dose" RELATED [VX]
synonym: "Cmax after the 1st dosing" RELATED [VX]
synonym: "Cmax after the 2nd dosing" RELATED [VX]
synonym: "Cmax blood" RELATED [VX]
synonym: "Cmax blood radioactivity" RELATED [VX]
synonym: "Cmax free" NARROW [VX]
synonym: "Cmax in blood" RELATED [VX]
synonym: "Cmax in brain" RELATED [VX]
synonym: "Cmax in plasma" RELATED [VX]
synonym: "Cmax lung" RELATED [VX]
synonym: "Cmax mg/mL" NARROW [VX]
synonym: "Cmax micronised" RELATED [VX]
synonym: "Cmax norm" NARROW [VX]
synonym: "Cmax plasma" RELATED [VX]
synonym: "Cmax plasma radioactivity" RELATED [VX]
synonym: "Cmax repeated dose (1st dose)" RELATED [VX]
synonym: "Cmax repeated dose (2nd dose)" RELATED [VX]
synonym: "Cmax single dose (1st dose)" RELATED [VX]
synonym: "Cmax ss" NARROW [VX]
synonym: "Cmax total" NARROW [VX]
synonym: "Cmax wet bead milled" RELATED [VX]
synonym: "Cmax(Steady state- Days 14 & 22,combined)" RELATED [VX]
synonym: "Cmax(single dose)" NARROW [VX]
synonym: "Cmax, dose 1" RELATED [VX]
synonym: "Cmax, dose 2" RELATED [VX]
synonym: "Cmax, dose 3" RELATED [VX]
synonym: "Cmax,ss" NARROW [VX]
synonym: "Cmax,ss (Lu 33-180)" NARROW [VX]
synonym: "Cmax.1" NARROW [VX]
synonym: "Cmax.2" NARROW [VX]
synonym: "Cmax1" NARROW [VX]
synonym: "Cmax2" NARROW [VX]
synonym: "CmaxT1" RELATED [VX]
synonym: "CmaxT2" RELATED [VX]
synonym: "Composite Cmax" RELATED [VX]
synonym: "Cpmax" RELATED [VX]
synonym: "Cssmax" RELATED [VX]
synonym: "Cu max" RELATED [VX]
synonym: "Cu,max" RELATED [VX]
synonym: "Experimental maximum concentration (Cmax)" RELATED [VX]
synonym: "Highest observed concentration in blood (Cmax)" RELATED [VX]
synonym: "Max. blood concentration (Cmax)" RELATED [VX]
synonym: "Max. plasma concentration (Cmax)" RELATED [VX]
synonym: "Maximal concentration (Cmax)" RELATED [VX]
synonym: "Maximum concentration (Cmax)" RELATED [VX]
synonym: "Maximum concentration observed (Cmax)" RELATED [VX]
synonym: "Maximum concentration of drug (Cmax)" RELATED [VX]
synonym: "Maximum mean plasma concentration (Cmax )" RELATED [VX]
synonym: "Maximum observed concentration (Cmax)" RELATED [VX]
synonym: "Maximum observed plasma concentration (Cmax)" RELATED [VX]
synonym: "Maximum plasma concentration (Cmax)" RELATED [VX]
synonym: "Maximum plasma concentrations (Cmax )" RELATED [VX]
synonym: "Maximum plasma concentrations (Cmax)" RELATED [VX]
synonym: "Maximum plasma concentrations after first daily dose (Cmax1)" RELATED [VX]
synonym: "Maximum plasma concentrations after second daily dose (Cmax2)" RELATED [VX]
synonym: "Maximum total plasma concentratio" RELATED [VX]
synonym: "Mean C max" RELATED [VX]
synonym: "Mean Cmax" NARROW [VX]
synonym: "Mean Cmax Day 1,14,28" RELATED [VX]
synonym: "Mean highest plasma concentration (Cmax)" RELATED [VX]
synonym: "Mean maximum plasma concentration (Cmax)" RELATED [VX]
synonym: "Mean peak blood concentraion (Cmax)" RELATED [VX]
synonym: "Mean peak blood concentraion/dose (Cmax/dose)" RELATED [VX]
synonym: "Mean peak concentration (Cmax )" RELATED [VX]
synonym: "Mean peak concentration (Cmax)" RELATED [VX]
synonym: "Mean peak serum concentration (Cmax)" RELATED [VX]
synonym: "Mean plasma concentrationC8 hours" RELATED [VX]
synonym: "Observed C max" RELATED [VX]
synonym: "Observed Cmax" RELATED [VX]
synonym: "Observed maximum concentration (Cmax)" RELATED [VX]
synonym: "Observed maximum concentration of drug after the first daily dosing (Cmax1)" RELATED [VX]
synonym: "Observed maximum concentration of drug after the second daily dosing (Cmax2)" RELATED [VX]
synonym: "Observed maximum concentration of drug after the second daily dosing(Cmax2)" RELATED [VX]
synonym: "Observed maximum plasma concentration corresponding to the first peak (Cmax1)" RELATED [VX]
synonym: "Observed maximum plasma concentration corresponding to the second peak (Cmax2)" RELATED [VX]
synonym: "Peak concentration (Cmax)" RELATED [VX]
synonym: "Plasma Cmax" NARROW [VX]
synonym: "Plasma ultrafiltrate Cmax" NARROW [VX]
synonym: "Putative C max" RELATED [VX]
synonym: "The maximum observed concentration (Cmax)" RELATED [VX]
synonym: "Unbound Cmax" RELATED [VX]
synonym: "c max" EXACT [VX]
is_a: terms:085493 ! terms_C85493

[Term]
id: terms:070919
name: Time of CMAX
def: "The time of maximum observed concentration sampled during a dosing interval."[]
synonym: "Apparent Tmax (Testes)" RELATED [VX]
synonym: "Apparent Tmax (Whole Blood)" RELATED [VX]
synonym: "Blood Tmax" RELATED [VX]
synonym: "Blood tmax" RELATED [VX]
synonym: "Experimental time of maximum concentration (Tmax)" RELATED [VX]
synonym: "First time to reach C max (Tmax)" RELATED [VX]
synonym: "First time to reach Cmax (tmax)" RELATED [VX]
synonym: "Mean Tmax" RELATED [VX]
synonym: "Mean Tmax from Day 1,14,28" RELATED [VX]
synonym: "Median Tmax" NARROW [VX]
synonym: "Median Tmax micronised" RELATED [VX]
synonym: "Median Tmax wet bead milled" RELATED [VX]
synonym: "Observed t max" RELATED [VX]
synonym: "Observed tmax" RELATED [VX]
synonym: "Plasma Tmax" EXACT [VX]
synonym: "Plasma tmax" EXACT [VX]
synonym: "Plasma ultrafiltrate tmax" NARROW [VX]
synonym: "T max" EXACT [VX]
synonym: "T max (1st treatment)" NARROW [VX]
synonym: "T max (2nd treatment)" NARROW [VX]
synonym: "T max (3rd treatment)" NARROW [VX]
synonym: "T(max)" EXACT [VX]
synonym: "TMAX" EXACT [VX]
synonym: "TMAX" EXACT [SEND]
synonym: "TMax" EXACT [VX]
synonym: "Time associated with Cmax (tmax)" RELATED [VX]
synonym: "Time at  Cmax (t max )" RELATED [VX]
synonym: "Time at Cmax (t max )" RELATED [VX]
synonym: "Time corresponding to Cmax (tmax)" RELATED [VX]
synonym: "Time of C max (tmax)" RELATED [VX]
synonym: "Time of Cmax (Tmax)" EXACT [VX]
synonym: "Time of Cmax (t max)" EXACT [VX]
synonym: "Time of Cmax (tmax)" EXACT [VX]
synonym: "Time of maximum concentration (Tmax)" RELATED [VX]
synonym: "Time of maximum observed concentration (Tmax)" RELATED [VX]
synonym: "Time of maximum observed concentration (t max)" RELATED [VX]
synonym: "Time of maximum observed concentration (tmax)" RELATED [VX]
synonym: "Time of maximum observed plasma concentration (t max)" RELATED [VX]
synonym: "Time of maximum plasma concentration (t max)" RELATED [VX]
synonym: "Time of observed maximum concentration (tmax)" RELATED [VX]
synonym: "Time of occurrence of Cmax (tmax)" RELATED [VX]
synonym: "Time to Cmax (Tmax)" RELATED [VX]
synonym: "Time to Cmax (tmax)" RELATED [VX]
synonym: "Time to maximum concentration (t max)" RELATED [VX]
synonym: "Time to maximum concentration (tmax)" RELATED [VX]
synonym: "Time to maximum plasma concentration (Tmax)" RELATED [VX]
synonym: "Time to reach highest plasma concentration (tmax)" RELATED [VX]
synonym: "Time to reach maximum concentration (tmax)" RELATED [VX]
synonym: "Time to reach maximum concentration after the first daily dosing (tmax1)" RELATED [VX]
synonym: "Time to reach maximum concentration after the second daily dosing (tmax2)" RELATED [VX]
synonym: "Time to reach maximum plasma concentration (Tmax)" RELATED [VX]
synonym: "Time to reach peak concentration (Tmax)" RELATED [VX]
synonym: "Time to reach peak concentration in blood (tmax)" RELATED [VX]
synonym: "Time to reach the first maximum concentration (tmax1)" RELATED [VX]
synonym: "Time to reach the maximum plasma concentration (Tmax)" RELATED [VX]
synonym: "Time to reach the peak concentration in blood (tmax)" RELATED [VX]
synonym: "Time to reach the second maximum concentration (tmax2)" RELATED [VX]
synonym: "Tmax" EXACT [VX]
synonym: "Tmax  (9th administration)" RELATED [VX]
synonym: "Tmax  (metabolite X)" NARROW [VX]
synonym: "Tmax  in brain" RELATED [VX]
synonym: "Tmax (10th administration)" RELATED [VX]
synonym: "Tmax (1st administration)" RELATED [VX]
synonym: "Tmax (1st dosing)" NARROW [VX]
synonym: "Tmax (2d administration)" RELATED [VX]
synonym: "Tmax (2nd dosing)" NARROW [VX]
synonym: "Tmax (ICS 205-930)" NARROW [VX]
synonym: "Tmax (Lu 33-108)" NARROW [VX]
synonym: "Tmax (Metabolite CGP 10000)" RELATED [VX]
synonym: "Tmax (Metabolite GP 47680)" RELATED [VX]
synonym: "Tmax (Metabolite ICS-5-0H)" NARROW [VX]
synonym: "Tmax (Metabolite ICS-6-0H)" NARROW [VX]
synonym: "Tmax (Rat #6 12hr point)" RELATED [VX]
synonym: "Tmax (SR 121407)" NARROW [VX]
synonym: "Tmax (SSR-epimer)" NARROW [VX]
synonym: "Tmax (ZK 811694)" NARROW [VX]
synonym: "Tmax (a)" NARROW [VX]
synonym: "Tmax (acid metabolite)" NARROW [VX]
synonym: "Tmax (after 1st dosing)" NARROW [VX]
synonym: "Tmax (after 2nd dosing" NARROW [VX]
synonym: "Tmax (blood)" RELATED [VX]
synonym: "Tmax (dose 1)" RELATED [VX]
synonym: "Tmax (dose 2)" RELATED [VX]
synonym: "Tmax (high value)" RELATED [VX]
synonym: "Tmax (highest value)" RELATED [VX]
synonym: "Tmax (low value)" RELATED [VX]
synonym: "Tmax (lowest value)" RELATED [VX]
synonym: "Tmax (metabolite X)" NARROW [VX]
synonym: "Tmax (metabolite x)" NARROW [VX]
synonym: "Tmax (metabolite)" NARROW [VX]
synonym: "Tmax (multiple dose)" RELATED [VX]
synonym: "Tmax (multiple dose, after 1st daily dose)" NARROW [VX]
synonym: "Tmax (multiple dose, after 2nd daily dose)" NARROW [VX]
synonym: "Tmax (plasma)" RELATED [VX]
synonym: "Tmax (single dose)" NARROW [VX]
synonym: "Tmax 1" RELATED [VX]
synonym: "Tmax 2" RELATED [VX]
synonym: "Tmax RDA136" RELATED [VX]
synonym: "Tmax SDA137" RELATED [VX]
synonym: "Tmax TRI476" RELATED [VX]
synonym: "Tmax after the 1st dosing" RELATED [VX]
synonym: "Tmax after the 2nd dosing" RELATED [VX]
synonym: "Tmax hours after dose (dose 1)" RELATED [VX]
synonym: "Tmax hours after dose (dose 2)" RELATED [VX]
synonym: "Tmax in blood" RELATED [VX]
synonym: "Tmax in plasma" RELATED [VX]
synonym: "Tmax median" EXACT [VX]
synonym: "Tmax range" RELATED [VX]
synonym: "Tmax repeated dose (1st dose)" RELATED [VX]
synonym: "Tmax repeated dose (2st dose)" RELATED [VX]
synonym: "Tmax single dose (1st dose)" RELATED [VX]
synonym: "Tmax(Steady state- Days 14 & 22,combined)" RELATED [VX]
synonym: "Tmax(metabolite X)" NARROW [VX]
synonym: "Tmax(single dose)" NARROW [VX]
synonym: "Tmax1" NARROW [VX]
synonym: "Tmax2" NARROW [VX]
synonym: "t  max" EXACT [VX]
synonym: "t max" EXACT [VX]
synonym: "t max (1st dosing)" RELATED [VX]
synonym: "t max (2nd dosing)" RELATED [VX]
synonym: "t max (brain)" RELATED [VX]
synonym: "t max (liver)" RELATED [VX]
synonym: "t max (median)" RELATED [VX]
synonym: "t max (plasma)" EXACT [VX]
synonym: "t max (recovery animals)" RELATED [VX]
synonym: "t max 1" RELATED [VX]
synonym: "t max after 1st dose" RELATED [VX]
synonym: "t max after 2d dose" RELATED [VX]
synonym: "t max blood" EXACT [VX]
synonym: "t max median" RELATED [VX]
synonym: "t max plasma" EXACT [VX]
synonym: "t max(mean Day1/Day5)" RELATED [VX]
synonym: "t max.1" RELATED [VX]
synonym: "t(max)" EXACT [VX]
synonym: "tmac" RELATED [VX]
synonym: "tmax" EXACT [VX]
synonym: "tmax a" NARROW [VX]
synonym: "tmax blood" RELATED [VX]
synonym: "tmax blood radioactivity" RELATED [VX]
synonym: "tmax plasma" RELATED [VX]
synonym: "tmax plasma radioactivity" RELATED [VX]
synonym: "tmax1" NARROW [VX]
synonym: "tmax2" NARROW [VX]
is_a: terms:085493 ! terms_C85493

[Term]
id: terms:075913
name: Renal CL
def: "The clearance of a substance from the blood by the kidneys."[]
synonym: "RENALCL" EXACT [SEND]
synonym: "Renal clearance (CLr)" RELATED [VX]
is_a: terms:085493 ! terms_C85493

[Term]
id: terms:085542
name: R Squared
def: "The goodness of fit statistic for the terminal elimination phase."[]
synonym: "R2" EXACT [SEND]
is_a: terms:085493 ! terms_C85493

[Term]
id: terms:085553
name: R Squared Adjusted
def: "The goodness of fit statistic for the terminal elimination phase, adjusted for the number of time points used in the estimation of Lambda z."[]
is_a: terms:085493 ! terms_C85493

[Term]
id: terms:085564
name: AUC All
def: "The area under the curve (AUC) from the time of dosing to the time of the last observation, regardless of whether the last concentration is measurable or not."[]
synonym: "AUC" RELATED [VX]
synonym: "AUC ( 0 - 2 4 h )" RELATED [VX]
synonym: "AUC (0-1 day)" RELATED [VX]
synonym: "AUC (0-1.5h)" RELATED [VX]
synonym: "AUC (0-10h)" NARROW [VX]
synonym: "AUC (0-10h) (2x30umol/kg)" NARROW [VX]
synonym: "AUC (0-10h) (2x40 umol/kg)" NARROW [VX]
synonym: "AUC (0-12)" NARROW [VX]
synonym: "AUC (0-12.25h)" RELATED [VX]
synonym: "AUC (0-168h)" RELATED [VX]
synonym: "AUC (0-16h)" RELATED [VX]
synonym: "AUC (0-18)" NARROW [VX]
synonym: "AUC (0-23 hr)" NARROW [VX]
synonym: "AUC (0-24 h)" NARROW [VX]
synonym: "AUC (0-24 h)b.i.d (multiple dose)" RELATED [VX]
synonym: "AUC (0-24 hr)" RELATED [VX]
synonym: "AUC (0-24)" NARROW [VX]
synonym: "AUC (0-24) (SR 121407)" NARROW [VX]
synonym: "AUC (0-24) (dose normalised)" NARROW [VX]
synonym: "AUC (0-24) in blood" RELATED [VX]
synonym: "AUC (0-24) in plasma" RELATED [VX]
synonym: "AUC (0-24.5h)" NARROW [VX]
synonym: "AUC (0-24h)" NARROW [VX]
synonym: "AUC (0-24h) (2x30umol/kg)" NARROW [VX]
synonym: "AUC (0-24h) (2x40umol/kg)" NARROW [VX]
synonym: "AUC (0-24h) (AZ12326299)" NARROW [VX]
synonym: "AUC (0-24h) (recovery animals)" RELATED [VX]
synonym: "AUC (0-24hr)" NARROW [VX]
synonym: "AUC (0-25)" RELATED [VX]
synonym: "AUC (0-25h)" RELATED [VX]
synonym: "AUC (0-26h)" NARROW [VX]
synonym: "AUC (0-29 day)" RELATED [VX]
synonym: "AUC (0-3)" RELATED [VX]
synonym: "AUC (0-3h)" RELATED [VX]
synonym: "AUC (0-4)" NARROW [VX]
synonym: "AUC (0-48)" RELATED [VX]
synonym: "AUC (0-48h)" RELATED [VX]
synonym: "AUC (0-48h) blood" RELATED [VX]
synonym: "AUC (0-48h) plasma" RELATED [VX]
synonym: "AUC (0-4h)" NARROW [VX]
synonym: "AUC (0-5 day)" RELATED [VX]
synonym: "AUC (0-5h)" RELATED [VX]
synonym: "AUC (0-5hr)" RELATED [VX]
synonym: "AUC (0-6 hr)" RELATED [VX]
synonym: "AUC (0-6)" NARROW [VX]
synonym: "AUC (0-7)norm" RELATED [VX]
synonym: "AUC (0-72) (blood)" RELATED [VX]
synonym: "AUC (0-72) (plasma)" RELATED [VX]
synonym: "AUC (0-72h)" RELATED [VX]
synonym: "AUC (0-7h)" NARROW [VX]
synonym: "AUC (0-8 h)" NARROW [VX]
synonym: "AUC (0-8)" NARROW [VX]
synonym: "AUC (0-8-24h)" RELATED [VX]
synonym: "AUC (0-8.25h)" RELATED [VX]
synonym: "AUC (0-8h)" NARROW [VX]
synonym: "AUC (0-8hr)" RELATED [VX]
synonym: "AUC (0-9)" NARROW [VX]
synonym: "AUC (0-T last)" RELATED [VX]
synonym: "AUC (0-i)" RELATED [VX]
synonym: "AUC (0-inf) (single dose)" RELATED [VX]
synonym: "AUC (0-last)" RELATED [VX]
synonym: "AUC (0-t)" NARROW [VX]
synonym: "AUC (0-t) micronised" RELATED [VX]
synonym: "AUC (0-t) wet bead milled" RELATED [VX]
synonym: "AUC (0-tlast)" RELATED [VX]
synonym: "AUC (1st dosing)" RELATED [VX]
synonym: "AUC (24h)" RELATED [VX]
synonym: "AUC (2nd dosing)" RELATED [VX]
synonym: "AUC (8)" RELATED [VX]
synonym: "AUC (AZ12326299)" RELATED [VX]
synonym: "AUC (ICS 205-930)" RELATED [VX]
synonym: "AUC (Metabolite 206-607)" RELATED [VX]
synonym: "AUC (Metabolite ICS-5-0H)" RELATED [VX]
synonym: "AUC (Metabolite ICS-6-0H)" RELATED [VX]
synonym: "AUC (all)" EXACT [VX]
synonym: "AUC (days 1 - 5)" RELATED [VX]
synonym: "AUC (metabolite X)" RELATED [VX]
synonym: "AUC (metabolite x)" RELATED [VX]
synonym: "AUC (model dependent analysis)" RELATED [VX]
synonym: "AUC (model independent analysis)" RELATED [VX]
synonym: "AUC (tot 24h)" RELATED [VX]
synonym: "AUC (tot)" RELATED [VX]
synonym: "AUC (tot24h)" RELATED [VX]
synonym: "AUC (total)" EXACT [VX]
synonym: "AUC 0-0.5hr" NARROW [VX]
synonym: "AUC 0-2.5h" NARROW [VX]
synonym: "AUC 0-24" NARROW [VX]
synonym: "AUC 0-24 (SSR-epimer)" NARROW [VX]
synonym: "AUC 0-24 (plasma-ultrafiltrate)" RELATED [VX]
synonym: "AUC 0-24 h" NARROW [VX]
synonym: "AUC 0-24 normalised to a dose of 100 mg/kg" NARROW [VX]
synonym: "AUC 0-24.5h" NARROW [VX]
synonym: "AUC 0-24h" NARROW [VX]
synonym: "AUC 0-24h (AVE8324)" NARROW [VX]
synonym: "AUC 0-24h)" NARROW [VX]
synonym: "AUC 0-29 days" RELATED [VX]
synonym: "AUC 0-4" NARROW [VX]
synonym: "AUC 0-48" RELATED [VX]
synonym: "AUC 0-4h" NARROW [VX]
synonym: "AUC 0-7" NARROW [VX]
synonym: "AUC 0-72" NARROW [VX]
synonym: "AUC 0-8" NARROW [VX]
synonym: "AUC 0-8h" NARROW [VX]
synonym: "AUC 0-8h after 1st dose" RELATED [VX]
synonym: "AUC 0-8h after first dose" RELATED [VX]
synonym: "AUC 0-8h repeated dose (1st dose, 1xdose)" RELATED [VX]
synonym: "AUC 0-8h repeated dose (2nd dose, 1xdose)" RELATED [VX]
synonym: "AUC 0-8h single dose (1st dose, 1xdose)" RELATED [VX]
synonym: "AUC 0-8hours" RELATED [VX]
synonym: "AUC 0-96" RELATED [VX]
synonym: "AUC 0-N" RELATED [VX]
synonym: "AUC 0-last" RELATED [VX]
synonym: "AUC 0-t" NARROW [VX]
synonym: "AUC 0-tlast" NARROW [VX]
synonym: "AUC 12" RELATED [VX]
synonym: "AUC 24" NARROW [VX]
synonym: "AUC 24 h" RELATED [VX]
synonym: "AUC 24h" NARROW [VX]
synonym: "AUC 2h" RELATED [VX]
synonym: "AUC 8" RELATED [VX]
synonym: "AUC a)" RELATED [VX]
synonym: "AUC all" EXACT [VX]
synonym: "AUC blood" RELATED [VX]
synonym: "AUC blood radioactivity" RELATED [VX]
synonym: "AUC burst" RELATED [VX]
synonym: "AUC finity blood" RELATED [VX]
synonym: "AUC finity plasma" RELATED [VX]
synonym: "AUC geometric mean" RELATED [VX]
synonym: "AUC inf blood" RELATED [VX]
synonym: "AUC inf plasma" RELATED [VX]
synonym: "AUC last" RELATED [VX]
synonym: "AUC last (0-24h)" RELATED [VX]
synonym: "AUC last (total)" RELATED [VX]
synonym: "AUC log. trapeze" RELATED [VX]
synonym: "AUC lung" RELATED [VX]
synonym: "AUC ods" RELATED [VX]
synonym: "AUC of radioactivity plasma" RELATED [VX]
synonym: "AUC of radioactivity, total components detected" RELATED [VX]
synonym: "AUC plasma" RELATED [VX]
synonym: "AUC plasma radioactivity" RELATED [VX]
synonym: "AUC ss" RELATED [VX]
synonym: "AUC ss/24" RELATED [VX]
synonym: "AUC t" RELATED [VX]
synonym: "AUC tlast" RELATED [VX]
synonym: "AUC tot" RELATED [VX]
synonym: "AUC total" EXACT [VX]
synonym: "AUC(-0-12)" NARROW [VX]
synonym: "AUC(0-0.583)" RELATED [VX]
synonym: "AUC(0-0.5h)" RELATED [VX]
synonym: "AUC(0-0.8.25)" RELATED [VX]
synonym: "AUC(0-00)" RELATED [VX]
synonym: "AUC(0-1.25)" NARROW [VX]
synonym: "AUC(0-1.5)" RELATED [VX]
synonym: "AUC(0-10)" NARROW [VX]
synonym: "AUC(0-12 h)" RELATED [VX]
synonym: "AUC(0-12)" NARROW [VX]
synonym: "AUC(0-120 h)" NARROW [VX]
synonym: "AUC(0-120h)" NARROW [VX]
synonym: "AUC(0-12h)" NARROW [VX]
synonym: "AUC(0-14)" RELATED [VX]
synonym: "AUC(0-16)" RELATED [VX]
synonym: "AUC(0-168 h)" RELATED [VX]
synonym: "AUC(0-168)" RELATED [VX]
synonym: "AUC(0-168h)" RELATED [VX]
synonym: "AUC(0-168h) blood" RELATED [VX]
synonym: "AUC(0-168h) blood pool" RELATED [VX]
synonym: "AUC(0-18h)" NARROW [VX]
synonym: "AUC(0-1h)" RELATED [VX]
synonym: "AUC(0-2 h)" NARROW [VX]
synonym: "AUC(0-2)" RELATED [VX]
synonym: "AUC(0-20)" RELATED [VX]
synonym: "AUC(0-20.18h)" RELATED [VX]
synonym: "AUC(0-21.8h)" RELATED [VX]
synonym: "AUC(0-22)" NARROW [VX]
synonym: "AUC(0-22h)" RELATED [VX]
synonym: "AUC(0-23.2h)" RELATED [VX]
synonym: "AUC(0-23h)" RELATED [VX]
synonym: "AUC(0-24 h)" NARROW [VX]
synonym: "AUC(0-24 h) plasma" RELATED [VX]
synonym: "AUC(0-24 h) plasma, lost during sample processing or HPLC" RELATED [VX]
synonym: "AUC(0-24 h) plasma, sum of additional trace metabolites (not assigned)" RELATED [VX]
synonym: "AUC(0-24 h) plasma, total components detected" RELATED [VX]
synonym: "AUC(0-24 h) plasma, total in original sample" RELATED [VX]
synonym: "AUC(0-24 h)(metabolite X)" NARROW [VX]
synonym: "AUC(0-24 hr)" RELATED [VX]
synonym: "AUC(0-24)" NARROW [VX]
synonym: "AUC(0-24) (AZ13263197)" NARROW [VX]
synonym: "AUC(0-24) (Metabolite CGP 10000)" RELATED [VX]
synonym: "AUC(0-24) (Metabolite GP 47680)" RELATED [VX]
synonym: "AUC(0-24) (N-desmethyl metabolite M594347)" NARROW [VX]
synonym: "AUC(0-24) (acid metabolite)" NARROW [VX]
synonym: "AUC(0-24) (dried blood samples)" NARROW [VX]
synonym: "AUC(0-24) (metabolite X)" NARROW [VX]
synonym: "AUC(0-24) (metabolite)" NARROW [VX]
synonym: "AUC(0-24) (normalized to dose 1 mg/kg)" NARROW [VX]
synonym: "AUC(0-24) blood" RELATED [VX]
synonym: "AUC(0-24) plasma" NARROW [VX]
synonym: "AUC(0-24), lost during HPLC" RELATED [VX]
synonym: "AUC(0-24), lost during sample processing" RELATED [VX]
synonym: "AUC(0-24), sum of additional trace metabolites (not assigned)" RELATED [VX]
synonym: "AUC(0-24), total components detected" RELATED [VX]
synonym: "AUC(0-24), total radioactivity in original sample" RELATED [VX]
synonym: "AUC(0-24)h" NARROW [VX]
synonym: "AUC(0-24)nom" RELATED [VX]
synonym: "AUC(0-24.5h)" NARROW [VX]
synonym: "AUC(0-240" RELATED [VX]
synonym: "AUC(0-240h)" RELATED [VX]
synonym: "AUC(0-24h)" NARROW [VX]
synonym: "AUC(0-24h) (RU 36384)" NARROW [VX]
synonym: "AUC(0-24h) (ZK 811694)" NARROW [VX]
synonym: "AUC(0-24h) (brain)" RELATED [VX]
synonym: "AUC(0-24h) (geometric)" NARROW [VX]
synonym: "AUC(0-24h) (liver)" RELATED [VX]
synonym: "AUC(0-24h) (metabolite X)" NARROW [VX]
synonym: "AUC(0-24h) (plasma)" RELATED [VX]
synonym: "AUC(0-24h) RDA136" RELATED [VX]
synonym: "AUC(0-24h) SDA137" RELATED [VX]
synonym: "AUC(0-24h) TRI476" RELATED [VX]
synonym: "AUC(0-24h) blood" RELATED [VX]
synonym: "AUC(0-24h) pool" RELATED [VX]
synonym: "AUC(0-24h) pool plasma" RELATED [VX]
synonym: "AUC(0-24h)(metabolite X)" NARROW [VX]
synonym: "AUC(0-24hr)" NARROW [VX]
synonym: "AUC(0-24hr)  in brain" RELATED [VX]
synonym: "AUC(0-24hrs)" NARROW [VX]
synonym: "AUC(0-25)" RELATED [VX]
synonym: "AUC(0-28)" RELATED [VX]
synonym: "AUC(0-28d)" RELATED [VX]
synonym: "AUC(0-2h)" NARROW [VX]
synonym: "AUC(0-3)" RELATED [VX]
synonym: "AUC(0-3.7h)" RELATED [VX]
synonym: "AUC(0-30)" NARROW [VX]
synonym: "AUC(0-336)" RELATED [VX]
synonym: "AUC(0-36)" RELATED [VX]
synonym: "AUC(0-3h)" RELATED [VX]
synonym: "AUC(0-4)" NARROW [VX]
synonym: "AUC(0-4)ss" NARROW [VX]
synonym: "AUC(0-4.25h) plasma" RELATED [VX]
synonym: "AUC(0-48)" RELATED [VX]
synonym: "AUC(0-48h)" RELATED [VX]
synonym: "AUC(0-5 days)" RELATED [VX]
synonym: "AUC(0-5)" NARROW [VX]
synonym: "AUC(0-5.5h)" RELATED [VX]
synonym: "AUC(0-50)" RELATED [VX]
synonym: "AUC(0-5h)" NARROW [VX]
synonym: "AUC(0-6 h)" NARROW [VX]
synonym: "AUC(0-6 hr)" RELATED [VX]
synonym: "AUC(0-6)" NARROW [VX]
synonym: "AUC(0-6.333hr)" RELATED [VX]
synonym: "AUC(0-7)" NARROW [VX]
synonym: "AUC(0-7.5)" RELATED [VX]
synonym: "AUC(0-720)" RELATED [VX]
synonym: "AUC(0-72h)" RELATED [VX]
synonym: "AUC(0-7h)" NARROW [VX]
synonym: "AUC(0-7hr)" RELATED [VX]
synonym: "AUC(0-8 h)" NARROW [VX]
synonym: "AUC(0-8)" NARROW [VX]
synonym: "AUC(0-8)a" NARROW [VX]
synonym: "AUC(0-8.25)" NARROW [VX]
synonym: "AUC(0-8.25h) plasma" RELATED [VX]
synonym: "AUC(0-8h)" NARROW [VX]
synonym: "AUC(0-9)" NARROW [VX]
synonym: "AUC(0-96 or 168)" RELATED [VX]
synonym: "AUC(0-T last)" RELATED [VX]
synonym: "AUC(0-Tlast)" NARROW [VX]
synonym: "AUC(0-i)" RELATED [VX]
synonym: "AUC(0-inf) plasma" RELATED [VX]
synonym: "AUC(0-inf) pool plasma" RELATED [VX]
synonym: "AUC(0-last)" RELATED [VX]
synonym: "AUC(0-t hours)" RELATED [VX]
synonym: "AUC(0-t)" NARROW [VX]
synonym: "AUC(0-t) (BAY 43-9695 (M1))" NARROW [VX]
synonym: "AUC(0-t) (SB235365)" NARROW [VX]
synonym: "AUC(0-t) (model independent analysis)" NARROW [VX]
synonym: "AUC(0-tau)" NARROW [VX]
synonym: "AUC(0-tlast)" NARROW [VX]
synonym: "AUC(0-tlast) plasma" RELATED [VX]
synonym: "AUC(0-tlast) pool plasma" RELATED [VX]
synonym: "AUC(0-tn)" NARROW [VX]
synonym: "AUC(0-x)" RELATED [VX]
synonym: "AUC(024)" NARROW [VX]
synonym: "AUC(024h)" NARROW [VX]
synonym: "AUC(0¿24h)" NARROW [VX]
synonym: "AUC(0¿6h)" NARROW [VX]
synonym: "AUC(1-28Days)" RELATED [VX]
synonym: "AUC(1-4)" RELATED [VX]
synonym: "AUC(24)" NARROW [VX]
synonym: "AUC(24- )" RELATED [VX]
synonym: "AUC(24h)" RELATED [VX]
synonym: "AUC(X)" RELATED [VX]
synonym: "AUC(ingal)" RELATED [VX]
synonym: "AUC(inh)" RELATED [VX]
synonym: "AUC(last)" RELATED [VX]
synonym: "AUC(o-24)" NARROW [VX]
synonym: "AUC(o-t)" NARROW [VX]
synonym: "AUC(t)" RELATED [VX]
synonym: "AUC(t0)" RELATED [VX]
synonym: "AUC(to 8h)" NARROW [VX]
synonym: "AUC(tot 24 h)" RELATED [VX]
synonym: "AUC(tot24)" RELATED [VX]
synonym: "AUC(tot24h)" RELATED [VX]
synonym: "AUC(tot4h)" RELATED [VX]
synonym: "AUC(total)" EXACT [VX]
synonym: "AUC-24h" NARROW [VX]
synonym: "AUC0" RELATED [VX]
synonym: "AUC0-" RELATED [VX]
synonym: "AUC0-" RELATED [VX]
synonym: "AUC0-10" RELATED [VX]
synonym: "AUC0-12" NARROW [VX]
synonym: "AUC0-12h" NARROW [VX]
synonym: "AUC0-16" RELATED [VX]
synonym: "AUC0-168" RELATED [VX]
synonym: "AUC0-168 blood" RELATED [VX]
synonym: "AUC0-168 plasma" RELATED [VX]
synonym: "AUC0-168h" RELATED [VX]
synonym: "AUC0-168h blood" RELATED [VX]
synonym: "AUC0-2" NARROW [VX]
synonym: "AUC0-24" NARROW [VX]
synonym: "AUC0-24 (metabolite X1)" NARROW [VX]
synonym: "AUC0-24 (metabolite X2)" NARROW [VX]
synonym: "AUC0-24 blood" RELATED [VX]
synonym: "AUC0-24 h" NARROW [VX]
synonym: "AUC0-24 h (Testes)" RELATED [VX]
synonym: "AUC0-24 h (Whole Blood)" RELATED [VX]
synonym: "AUC0-24 hr" NARROW [VX]
synonym: "AUC0-24 plasma" RELATED [VX]
synonym: "AUC0-24(Steady state- Days 14 & 22,combined)" RELATED [VX]
synonym: "AUC0-24h" NARROW [VX]
synonym: "AUC0-24h (BIIF 1148)" NARROW [VX]
synonym: "AUC0-24h (Rat #6 12hr point)" RELATED [VX]
synonym: "AUC0-24h blood" RELATED [VX]
synonym: "AUC0-24h in pigmented skin" RELATED [VX]
synonym: "AUC0-24hr" NARROW [VX]
synonym: "AUC0-25" RELATED [VX]
synonym: "AUC0-26.2" NARROW [VX]
synonym: "AUC0-26.4" NARROW [VX]
synonym: "AUC0-26.6" NARROW [VX]
synonym: "AUC0-26.7" NARROW [VX]
synonym: "AUC0-27" NARROW [VX]
synonym: "AUC0-28h" NARROW [VX]
synonym: "AUC0-2hpd" NARROW [VX]
synonym: "AUC0-4" RELATED [VX]
synonym: "AUC0-48" NARROW [VX]
synonym: "AUC0-48h" RELATED [VX]
synonym: "AUC0-5" RELATED [VX]
synonym: "AUC0-6" NARROW [VX]
synonym: "AUC0-6h" NARROW [VX]
synonym: "AUC0-7" NARROW [VX]
synonym: "AUC0-72" RELATED [VX]
synonym: "AUC0-72 blood" RELATED [VX]
synonym: "AUC0-72 plasma" RELATED [VX]
synonym: "AUC0-8" NARROW [VX]
synonym: "AUC0-8 h" RELATED [VX]
synonym: "AUC0-8h" NARROW [VX]
synonym: "AUC0-96" RELATED [VX]
synonym: "AUC0-96h" RELATED [VX]
synonym: "AUC0-96h blood" RELATED [VX]
synonym: "AUC0-96h plasma" RELATED [VX]
synonym: "AUC0-?" RELATED [VX]
synonym: "AUC0-inf blood" RELATED [VX]
synonym: "AUC0-inf plasma" RELATED [VX]
synonym: "AUC0-last" RELATED [VX]
synonym: "AUC0-t" RELATED [VX]
synonym: "AUC0-t last blood" RELATED [VX]
synonym: "AUC0-t last plasma" RELATED [VX]
synonym: "AUC0-t plasma" RELATED [VX]
synonym: "AUC0-tlast" RELATED [VX]
synonym: "AUC0.24" NARROW [VX]
synonym: "AUC024" RELATED [VX]
synonym: "AUC1" RELATED [VX]
synonym: "AUC2" RELATED [VX]
synonym: "AUC24" NARROW [VX]
synonym: "AUC24 (Cyanide exposure without endogenous cyanide determined on the two untreated animals/sex)" RELATED [VX]
synonym: "AUC24, ss" RELATED [VX]
synonym: "AUC24,ss" RELATED [VX]
synonym: "AUC24h" RELATED [VX]
synonym: "AUC4" RELATED [VX]
synonym: "AUC4h" RELATED [VX]
synonym: "AUC6" RELATED [VX]
synonym: "AUC7" RELATED [VX]
synonym: "AUC72" RELATED [VX]
synonym: "AUC8" RELATED [VX]
synonym: "AUC96" RELATED [VX]
synonym: "AUCALL" EXACT [SEND]
synonym: "AUC_0_INF" RELATED [VX]
synonym: "AUCall" EXACT [VX]
synonym: "AUCinf blood" RELATED [VX]
synonym: "AUCinf plasma" RELATED [VX]
synonym: "AUCinhal" RELATED [VX]
synonym: "AUClast" RELATED [VX]
synonym: "AUClast blood" RELATED [VX]
synonym: "AUClast plasma" RELATED [VX]
synonym: "AUCo-24" RELATED [VX]
synonym: "AUCss" RELATED [VX]
synonym: "AUCss (Lu 33-108)" RELATED [VX]
synonym: "AUCss24" RELATED [VX]
synonym: "AUCt" RELATED [VX]
synonym: "AUCtot" RELATED [VX]
synonym: "AUCtotal" RELATED [VX]
synonym: "AUCtrap" RELATED [VX]
synonym: "AUCu(0-24)" NARROW [VX]
synonym: "AUD" RELATED [VX]
synonym: "AUD (1-20h)" RELATED [VX]
synonym: "AUDC (0.5-inf)" RELATED [VX]
synonym: "AUMC0-inf" RELATED [VX]
synonym: "AUQ 0-24" RELATED [VX]
synonym: "AUX(0-24h)" RELATED [VX]
synonym: "AUX(0-6h)" RELATED [VX]
synonym: "Area under blood concentration-time curve from 0h (pre-dose) to 24h (AUC(0-24h))" RELATED [VX]
synonym: "Area under concentration time curve from time 0 to 24h post-dose (AUC(0-24))" RELATED [VX]
synonym: "Area under concentration-time curve (AUC(0-24))" RELATED [VX]
synonym: "Area under concentration-time curve from 0 to 24h (AUC(0-24))" RELATED [VX]
synonym: "Area under concentration-time curve from time zero to the last time point of measurable concentration (AUC(0-t))" RELATED [VX]
synonym: "Area under concentration-time profile (AUC(0-t))" RELATED [VX]
synonym: "Area under curve (AUC(0-24h))" RELATED [VX]
synonym: "Area under curve (AUC(0-3))" RELATED [VX]
synonym: "Area under curve AUC(0-24h)" RELATED [VX]
synonym: "Area under curve from 0 to 24 hours post-dose (AUC(0-24))" RELATED [VX]
synonym: "Area under mandibular lymph nodes concentration-time curve from 0h (pre-dose) to 24h (AUC(0-24h))" RELATED [VX]
synonym: "Area under observed plasma concentration versus curve over the dose interval (24 h) (AUC(24))" RELATED [VX]
synonym: "Area under plasma concentration curve (AUC(0-24))" RELATED [VX]
synonym: "Area under plasma concentration curve (AUC(0-24h))" RELATED [VX]
synonym: "Area under plasma concentration curve from 0-24 h post-dose (AUC(0-24h))" RELATED [VX]
synonym: "Area under plasma concentration curve in dosage interval (AUC(0-24))" RELATED [VX]
synonym: "Area under plasma concentration time curve (AUC all)" RELATED [VX]
synonym: "Area under plasma concentration time curve (AUC(0-24))" NARROW [VX]
synonym: "Area under plasma concentration time curve calculated by linear trapezoidal method from time 0 to 24 h post-dose (AUC(0-24))" RELATED [VX]
synonym: "Area under plasma concentration time curve calculated by linear trapezoidal method from time 0 to 24h post-dose (AUC(0-24))" RELATED [VX]
synonym: "Area under plasma concentration time curve from 0 to 24h post-dose (AUC(0-24))" RELATED [VX]
synonym: "Area under plasma concentration time curve from time 0 to 24 h post-dose (AUC(0-24))" RELATED [VX]
synonym: "Area under plasma concentration time curve from time 0 to 24 h postdose (AUC(0-24h))" RELATED [VX]
synonym: "Area under plasma concentration time curve from time 0 to 24 hours (AUC(0-24h))" RELATED [VX]
synonym: "Area under plasma concentration time curve from time 0 to 24h (AUC(0-24))" RELATED [VX]
synonym: "Area under plasma concentration time curve from time 0 to 24h post-dose (AUC(0-24))" RELATED [VX]
synonym: "Area under plasma concentration time curve from time 0 to 24h post-dose (AUC(0-24h))" RELATED [VX]
synonym: "Area under plasma concentration time curve from time 0 to time 24 hours (AUC(0-24))" RELATED [VX]
synonym: "Area under plasma concentration versus time curve time 0 to the last measurable concentration (AUC(t))" RELATED [VX]
synonym: "Area under plasma concentration versus time curve to 24 h (AUC(24))" RELATED [VX]
synonym: "Area under plasma concentration versus time extrapolated to infinity (AUC)" RELATED [VX]
synonym: "Area under plasma concentration-time curve (AUC(0-24))" NARROW [VX]
synonym: "Area under plasma concentration-time curve calculated by linear trapezoidal method from time 0 to 24 h post-dose (AUC(0-24))" RELATED [VX]
synonym: "Area under plasma concentration-time curve from start of inhalation to 24 hours (AUC(tot24h))" RELATED [VX]
synonym: "Area under plasma concentration-time curve from zero (end ofinhalation) to 24 hours (AUC(0-24h))" RELATED [VX]
synonym: "Area under plasma concentration-time curve from zero to 24 hours (AUC(0-24h))" NARROW [VX]
synonym: "Area under plasma concentration-time curve from zero to t hours (AUC(0-t))" RELATED [VX]
synonym: "Area under plasma concentration-time curve observed from time 0 to time 24 h (AUC(24))" RELATED [VX]
synonym: "Area under plasma concentration-time curves from 0 to 24h (AUC(0-24))" RELATED [VX]
synonym: "Area under platinum plasma concentration-time curve 0 to 24 hours (AUC(0-24))" RELATED [VX]
synonym: "Area under spleen concentration-time curve from 0h (pre-dose) to 24h (AUC(0-24h))" RELATED [VX]
synonym: "Area under the curve (AUC(0-12h))" RELATED [VX]
synonym: "Area under the curve (AUC(0-24))" RELATED [VX]
synonym: "Area under the curve (AUC(0-24h))" RELATED [VX]
synonym: "Area under the curve (AUC(0-24hr))" RELATED [VX]
synonym: "Area under the curve (AUC(0-6h))" RELATED [VX]
synonym: "Area under the curve (AUC)" RELATED [VX]
synonym: "Area under the observed plasma concentration versus time curve extrapolated to infinity (AUC)" RELATED [VX]
synonym: "Area under the plasma concentration time curve (AUC(0-24h))" RELATED [VX]
synonym: "Area under the plasma concentration time curve between 0 and 24 hours (AUC(0-24))" RELATED [VX]
synonym: "Area under the plasma concentration time curve from 0 to 24 (AUC(0-24))" RELATED [VX]
synonym: "Area under the plasma concentration time curve from 0 to 9 (AUC(0-9))" RELATED [VX]
synonym: "Area under the plasma concentration time curve from time 0 to 24 h post-dose (AUC(0-24h))" RELATED [VX]
synonym: "Area under the plasma concentration time curve up to 24 hours (AUC(0-24))" RELATED [VX]
synonym: "Area under the plasma concentration-time curve (AUC(0-24))" RELATED [VX]
synonym: "Area under the plasma concentration-time curve (AUC(0-6))" RELATED [VX]
synonym: "Area under the plasma concentration-time curve during dosing (AUC(inhal))" RELATED [VX]
synonym: "Area under the plasma concentration-time curve from 0 to 24 hours post dose (AUC(0-24))" RELATED [VX]
synonym: "Area under the plasma concentration-time curve from time 0 to time 24h (AUC(24))" RELATED [VX]
synonym: "Area under the plasma concentration-time curve from time 0 to time 24h at steady-state (AUC(24,ss))" RELATED [VX]
synonym: "Area under the plasma concentration-time curve from zero to 24 hours (AUC(0-24))" NARROW [VX]
synonym: "Area under the plasma concentration-time curve from zero to 24 hours (AUC(0-24h))" RELATED [VX]
synonym: "Area under the plasma concentration-time curve from zero to t hours (AUC(0-t))" RELATED [VX]
synonym: "Areas under plasma concentration-time curves (AUC(0-24))" RELATED [VX]
synonym: "Areas under plasma concentration-time curves (AUC(0-24h))" RELATED [VX]
synonym: "Auc" RELATED [VX]
synonym: "Auc 0-24" NARROW [VX]
synonym: "Auc(0-24)" NARROW [VX]
synonym: "Auc(0-24h)" NARROW [VX]
synonym: "Auc0-24" NARROW [VX]
synonym: "Blood AUC(0-168h)" RELATED [VX]
synonym: "Blood AUC(0-Tlast)" RELATED [VX]
synonym: "Blood AUCs (0-24)" RELATED [VX]
synonym: "Composite AUC(0-24) (NJH)" RELATED [VX]
synonym: "DNAUC (0-t)" RELATED [VX]
synonym: "DPF (0-24h)" RELATED [VX]
synonym: "DPF (0-48h)" RELATED [VX]
synonym: "Exposure AUC" RELATED [VX]
synonym: "Ganciclovir - AUC" RELATED [VX]
synonym: "Mean AUC" RELATED [VX]
synonym: "Mean AUC (0-24h)" RELATED [VX]
synonym: "Mean AUC (0-26h)" RELATED [VX]
synonym: "Mean AUC (0-6h)" NARROW [VX]
synonym: "Mean AUC (0-72h)" RELATED [VX]
synonym: "Mean AUC (0-t)" RELATED [VX]
synonym: "Mean AUC(0-12h)" RELATED [VX]
synonym: "Mean AUC(0-24)" RELATED [VX]
synonym: "Mean AUC(0-24h)" NARROW [VX]
synonym: "Mean AUC(0-24h) from Day 1,14,28" RELATED [VX]
synonym: "Mean AUC(0-24h)/Dose from Day 1,14,28" RELATED [VX]
synonym: "Mean AUC(0-28 days)" RELATED [VX]
synonym: "Mean AUC(0-t)" RELATED [VX]
synonym: "Mean AUC(t)" RELATED [VX]
synonym: "Mean AUC(total)" RELATED [VX]
synonym: "Mean area under concentration-time curve from t zero to last quantifiable plasma concentration (AUC(0-t))" RELATED [VX]
synonym: "Plasma AUC 0-24" NARROW [VX]
synonym: "Plasma AUC 0-96" NARROW [VX]
synonym: "Plasma AUC(0-Tlast)" RELATED [VX]
synonym: "Plasma AUC(0-t)" NARROW [VX]
synonym: "Plasma AUC0-t" NARROW [VX]
synonym: "Plasma exposure" RELATED [VX]
synonym: "Plasma ultrafiltrate AUC 0-24" RELATED [VX]
synonym: "Plasma ultrafiltrate AUC 0-96" NARROW [VX]
synonym: "Plasma ultrafiltrate AUC(0-t)" RELATED [VX]
synonym: "Plasma ultrafiltrate AUC0-t" NARROW [VX]
synonym: "Rac  AUC 0-24" RELATED [VX]
synonym: "Rac(AUC 0-24)" RELATED [VX]
synonym: "Rac(AUC(0-24)" RELATED [VX]
synonym: "The area under the plasma concentration versus time curve from time 0 to 24 h (AUC(24))" RELATED [VX]
synonym: "Total AUC" RELATED [VX]
synonym: "Total area under plasma concentration-time profile at day 1 (AUC)" RELATED [VX]
synonym: "mean AUC (0-t)" RELATED [VX]
is_a: terms:085493 ! terms_C85493

[Term]
id: terms:085565
name: AUC to Last Nonzero Conc
def: "The area under the curve (AUC) from the time of dosing to the last measurable concentration."[]
synonym: "AUCLST" EXACT [SEND]
synonym: "Area under plasma concentration-time curve from zero to last detectable concentration (AUC(0-t ))" RELATED [VX]
is_a: terms:085493 ! terms_C85493

[Term]
id: terms:085566
name: AUC from T1 to T2
def: "The area under the curve (AUC) over the interval from T1 to T2."[]
synonym: "AUC (0-10)" NARROW [VX]
synonym: "AUC (0-24 )" NARROW [VX]
synonym: "AUC (0-24) plasma" NARROW [VX]
synonym: "AUC (0-6h)" NARROW [VX]
synonym: "AUC (0-7)" NARROW [VX]
synonym: "AUC (0-8 )" NARROW [VX]
synonym: "AUC (0.5-24h)" RELATED [VX]
synonym: "AUC (1-24)" NARROW [VX]
synonym: "AUC (1-24h)" RELATED [VX]
synonym: "AUC (1-6h) (brain)" RELATED [VX]
synonym: "AUC (1-6h) (liver)" RELATED [VX]
synonym: "AUC (1-6h) (plasma)" RELATED [VX]
synonym: "AUC (12)" NARROW [VX]
synonym: "AUC (24)" NARROW [VX]
synonym: "AUC 0-12" NARROW [VX]
synonym: "AUC 0-12h" NARROW [VX]
synonym: "AUC 0-5h" NARROW [VX]
synonym: "AUC 0-96 (plasma-ultrafiltrate)" RELATED [VX]
synonym: "AUC 0.1-3h" NARROW [VX]
synonym: "AUC 0.5-1hr" RELATED [VX]
synonym: "AUC 1-24" NARROW [VX]
synonym: "AUC 1-2hr" NARROW [VX]
synonym: "AUC 10-240 min" RELATED [VX]
synonym: "AUC 10-240min lung" RELATED [VX]
synonym: "AUC 2-4hr" NARROW [VX]
synonym: "AUC 4-8hr" NARROW [VX]
synonym: "AUC 8-24h" RELATED [VX]
synonym: "AUC 8-24h after 2d dose" RELATED [VX]
synonym: "AUC 8-24hr" NARROW [VX]
synonym: "AUC alpha" RELATED [VX]
synonym: "AUC beta" RELATED [VX]
synonym: "AUC during period of inhalation (AUCinhal)" RELATED [VX]
synonym: "AUC t1-tn" RELATED [VX]
synonym: "AUC(0-(t+24)h)" RELATED [VX]
synonym: "AUC(0-0.1.25)" RELATED [VX]
synonym: "AUC(0-12-25h)" RELATED [VX]
synonym: "AUC(0-18)" NARROW [VX]
synonym: "AUC(0-24" NARROW [VX]
synonym: "AUC(0-24 )" NARROW [VX]
synonym: "AUC(0-4h)" NARROW [VX]
synonym: "AUC(0-6h)" NARROW [VX]
synonym: "AUC(0-72)" NARROW [VX]
synonym: "AUC(0-eoi)" RELATED [VX]
synonym: "AUC(0.08-48h)" RELATED [VX]
synonym: "AUC(0.08-72h)" RELATED [VX]
synonym: "AUC(0.08-tlast)" RELATED [VX]
synonym: "AUC(0.08-tlast) whole blood" RELATED [VX]
synonym: "AUC(0.083-168h)" RELATED [VX]
synonym: "AUC(0.083-168h) blood" RELATED [VX]
synonym: "AUC(0.083-24h)" RELATED [VX]
synonym: "AUC(0.083-72h)" RELATED [VX]
synonym: "AUC(0.0833-24h)" NARROW [VX]
synonym: "AUC(0.0833-24h) (Male/Female)" NARROW [VX]
synonym: "AUC(0.1-3h)" NARROW [VX]
synonym: "AUC(0.17-t) (model independent analysis)" NARROW [VX]
synonym: "AUC(0.5-24)" RELATED [VX]
synonym: "AUC(0.5-24h)" RELATED [VX]
synonym: "AUC(0.667-24)" RELATED [VX]
synonym: "AUC(1-24)" NARROW [VX]
synonym: "AUC(12-36h)" RELATED [VX]
synonym: "AUC(14-28)" RELATED [VX]
synonym: "AUC(141-168d)" RELATED [VX]
synonym: "AUC(15-28)" RELATED [VX]
synonym: "AUC(169-239d)" RELATED [VX]
synonym: "AUC(2-12)" NARROW [VX]
synonym: "AUC(2-24)" NARROW [VX]
synonym: "AUC(3h-inf)" RELATED [VX]
synonym: "AUC(8-24 h)" NARROW [VX]
synonym: "AUC(eoi-24)" RELATED [VX]
synonym: "AUC(eoi-24h)" NARROW [VX]
synonym: "AUC(eoi-inf)" RELATED [VX]
synonym: "AUC(eoi-t)" RELATED [VX]
synonym: "AUC)0-24)" NARROW [VX]
synonym: "AUC0.5-24" NARROW [VX]
synonym: "AUC1-24" NARROW [VX]
synonym: "AUC2-24" NARROW [VX]
synonym: "AUC2-7" NARROW [VX]
synonym: "AUC500.01/AUC225" RELATED [VX]
synonym: "AUC90-24h)" RELATED [VX]
synonym: "AUCINT" EXACT [SEND]
synonym: "AUCinfusion" RELATED [VX]
synonym: "AUD (0.5-4(7)h)" RELATED [VX]
synonym: "Accumulation ratio (Rac (AUC) D33/D1)" RELATED [VX]
synonym: "Accumulation ratio for AUC(0-24) (R AUC(0-24))" RELATED [VX]
synonym: "Area under the curve (AUC(6-12h))" RELATED [VX]
synonym: "Areas under plasma concentration-time curves (AUC(24-336))" RELATED [VX]
synonym: "Rac (AUC) Day5/Day1" RELATED [VX]
is_a: terms:085493 ! terms_C85493

[Term]
id: terms:085567
name: AUC Over Dosing Interval
def: "The area under the curve (AUC) for the defined interval between doses (TAU)."[]
synonym: "AUC last (2nd treatment)" RELATED [VX]
synonym: "AUC last (3rd treatment)" RELATED [VX]
synonym: "AUCTAU" EXACT [SEND]
synonym: "AUCtau" EXACT [VX]
is_a: terms:085493 ! terms_C85493

[Term]
id: terms:085569
name: AUMC to Last Nonzero Conc
def: "The area under the moment curve (AUMC) from the time of dosing to the last measurable concentration."[]
is_a: terms:085493 ! terms_C85493

[Term]
id: terms:085570
name: AUMC Over Dosing Interval
def: "The area under the first moment curve (AUMC) for the defined interval between doses (TAU)."[]
is_a: terms:085493 ! terms_C85493

[Term]
id: terms:085571
name: AURC to Last Nonzero Rate
def: "The area under the urinary excretion rate curve (AURC) from time zero to the time of the last measurable concentration."[]
is_a: terms:085493 ! terms_C85493

[Term]
id: terms:085572
name: AURC from T1 to T2
def: "The area under the urinary excretion rate curve (AURC) over the interval from T1 to T2."[]
is_a: terms:085493 ! terms_C85493

[Term]
id: terms:085575
name: Average Concentration
def: "AUCTAU divided by TAU."[]
synonym: "Average plasma concentration calculated in dosage interval (Cmean)" RELATED [VX]
synonym: "Average steady-state plaasma concentration (Css,avg(24-336))" RELATED [VX]
synonym: "Average total plasma concentration" RELATED [VX]
synonym: "C(0-8h)" RELATED [VX]
synonym: "C(2-28days)" RELATED [VX]
synonym: "C(average)" RELATED [VX]
synonym: "C24-C48" RELATED [VX]
synonym: "CAVG" EXACT [SEND]
synonym: "Cav" RELATED [VX]
synonym: "Cav(0-24h)" RELATED [VX]
synonym: "Cav(Steady state- Days 14 & 22,combined)" RELATED [VX]
synonym: "Caverage" RELATED [VX]
synonym: "Cavg" EXACT [VX]
synonym: "Cmean" RELATED [VX]
synonym: "Css^a" RELATED [VX]
synonym: "Cssav" RELATED [VX]
synonym: "Mean C (5-10 min)" RELATED [VX]
synonym: "Mean C(120h) from Day 1,14,28" RELATED [VX]
synonym: "Mean Css" RELATED [VX]
synonym: "Mean HTF919 concentration" RELATED [VX]
synonym: "Mean blood concentration (day 1 of oestrous cycle)" RELATED [VX]
synonym: "Mean blood concentration (day 2 of oestrous cycle)" RELATED [VX]
synonym: "Mean blood concentration (day 3 of oestrous cycle)" RELATED [VX]
synonym: "Mean blood concentration (day 4 of oestrous cycle)" RELATED [VX]
synonym: "Mean blood concetration" RELATED [VX]
synonym: "Mean brain concentration" RELATED [VX]
synonym: "Mean concentration of MPA" RELATED [VX]
synonym: "Mean concentrations of AZD9935" RELATED [VX]
synonym: "Mean hair concentration" RELATED [VX]
synonym: "Mean kidneys concentration" RELATED [VX]
synonym: "Mean liver concentration" RELATED [VX]
synonym: "Mean lungs concentration" RELATED [VX]
synonym: "Mean normalized plasma concentrations" RELATED [VX]
synonym: "Mean plasma concentration (days 1- 5)" RELATED [VX]
synonym: "Mean plasma concentration (days 1-39)" RELATED [VX]
synonym: "Mean plasma concentration (days 15-39)" RELATED [VX]
synonym: "Mean plasma concentration (days 8-12)" RELATED [VX]
synonym: "Mean plasma concentration C4 hours" RELATED [VX]
synonym: "Mean plasma concentration C6 hours" RELATED [VX]
synonym: "Mean plasma level" RELATED [VX]
synonym: "Mean serum concentration" RELATED [VX]
synonym: "Mean skin concentration" RELATED [VX]
synonym: "Mean testicles concentration" RELATED [VX]
synonym: "Plasma average" RELATED [VX]
synonym: "Plasma concentration (mean arithm.)" RELATED [VX]
synonym: "Plasma concentration (mean geom.)" RELATED [VX]
synonym: "Serum concentration Cav(0-6h)" RELATED [VX]
synonym: "Steady state plasma concentraton" RELATED [VX]
is_a: terms:085493 ! terms_C85493

[Term]
id: terms:085579
name: Min Conc
def: "The minimum concentration between dose time and dose time plus Tau (at Tmin)."[]
synonym: "CMIN" EXACT [SEND]
synonym: "Cmin" EXACT [VX]
synonym: "Cmin (SSR-epimer)" NARROW [VX]
synonym: "Cmin (pre-dose concentration)" RELATED [VX]
synonym: "Cmin after the 1st dosing" RELATED [VX]
synonym: "Cmin after the 2nd dosing" RELATED [VX]
synonym: "Cmin1" RELATED [VX]
synonym: "Cmin2" RELATED [VX]
synonym: "Cmix" RELATED [VX]
synonym: "Mean minimum plasma concentration (Cmin)" RELATED [VX]
synonym: "Minimum plasma concentration (Cmin)" RELATED [VX]
is_a: terms:085493 ! terms_C85493

[Term]
id: terms:085580
name: Midpoint of Interval of Last Nonzero ER
def: "The midpoint of collection interval associated with last measurable excretion rate."[]
is_a: terms:085493 ! terms_C85493

[Term]
id: terms:085581
name: Fluctuation%
def: "The difference between Cmin and Cmax standardized to Cavg, between dose time and Tau."[]
is_a: terms:085493 ! terms_C85493

[Term]
id: terms:085644
name: Initial Conc
def: "Initial concentration. Given only for bolus IV models."[]
synonym: "C0" EXACT [VX]
synonym: "Concentration 5 minutes after end of infusion (C5min)" RELATED [VX]
synonym: "Ct=0 (extrapolated)" RELATED [VX]
is_a: terms:085493 ! terms_C85493

[Term]
id: terms:085652
name: Lambda z
def: "The first order rate constant associated with the terminal (log-linear) portion of the curve."[]
synonym: "Lambda z" EXACT [VX]
synonym: "lambda z" EXACT [VX]
is_a: terms:085493 ! terms_C85493

[Term]
id: terms:085653
name: Lambda z Lower Limit
def: "The lower limit on time for values to be included in the calculation of Lambda z."[]
is_a: terms:085493 ! terms_C85493

[Term]
id: terms:085654
name: Lambda z Upper Limit
def: "The upper limit on time for values to be included in the calculation of Lambda z."[]
is_a: terms:085493 ! terms_C85493

[Term]
id: terms:085655
name: Last Nonzero Conc
def: "The concentration corresponding to Tlast."[]
synonym: "C last (2nd treatment)" RELATED [VX]
synonym: "C last (3rd treatment)" RELATED [VX]
synonym: "C(last)" RELATED [VX]
synonym: "CLST" EXACT [SEND]
synonym: "Clast" RELATED [VX]
synonym: "Last measurable concentration (C last)" RELATED [VX]
synonym: "Mean last quantifiable plasma concentration (Ct)" RELATED [VX]
is_a: terms:085493 ! terms_C85493

[Term]
id: terms:085656
name: Last Meas Excretion Rate
def: "The last measurable (positive) excretion rate determined for the specimen type specified in PPSPEC."[]
is_a: terms:085493 ! terms_C85493

[Term]
id: terms:085698
name: Max Conc Norm by Dose
def: "The maximum concentration occurring at Tmax, divided by the dose."[]
synonym: "C max,norm" RELATED [VX]
synonym: "C max/D" RELATED [VX]
synonym: "C max/Dose" RELATED [VX]
synonym: "C max/dose" RELATED [VX]
synonym: "CMAXD" EXACT [SEND]
synonym: "Cmax (dose normalised)" RELATED [VX]
synonym: "Cmax (dose normalized)" RELATED [VX]
synonym: "Cmax (normalised to dose 100 mg/kg)" RELATED [VX]
synonym: "Cmax (normalized to dose 1 mg/kg)" RELATED [VX]
synonym: "Cmax / dose" EXACT [VX]
synonym: "Cmax dose normalized" RELATED [VX]
synonym: "Cmax normalised to a dose of 100 mg/kg" RELATED [VX]
synonym: "Cmax,norm" RELATED [VX]
synonym: "Cmax.norm" RELATED [VX]
synonym: "Cmax/D" EXACT [VX]
synonym: "Cmax/Dose" EXACT [VX]
synonym: "Cmax/Dose (Testes)" RELATED [VX]
synonym: "Cmax/Dose (Whole Blood)" RELATED [VX]
synonym: "Cmax/Dose (recovery animals)" RELATED [VX]
synonym: "Cmax/d" EXACT [VX]
synonym: "Cmax/dOSe" EXACT [VX]
synonym: "Cmax/dose" EXACT [VX]
synonym: "Css.av" RELATED [VX]
synonym: "Dose normalised Cmax" RELATED [VX]
synonym: "Dose-normalized Cmax (Cmax/dose)" RELATED [VX]
synonym: "Maximum plasma concentration (Cmax)  (dose-normalized)" RELATED [VX]
synonym: "Norm.Cmax" RELATED [VX]
is_a: terms:085493 ! terms_C85493

[Term]
id: terms:085699
name: Max Excretion Rate
def: "The maximum excretion rate determined for the specimen type specified in PPSPEC."[]
is_a: terms:085493 ! terms_C85493

[Term]
id: terms:085761
name: AUC Infinity Obs
def: "The area under the curve (AUC) extrapolated to infinity, calculated using the observed value of the last non-zero concentration."[]
synonym: "AUC (0- )" EXACT [VX]
synonym: "AUC (0-)" EXACT [VX]
synonym: "AUC (0-?)" EXACT [VX]
synonym: "AUC (0-INF)" EXACT [VX]
synonym: "AUC (0-inf)" EXACT [VX]
synonym: "AUC 0-" EXACT [VX]
synonym: "AUC 0-inf" EXACT [VX]
synonym: "AUC 0-inf (Lu 33-108)" RELATED [VX]
synonym: "AUC 0-~" EXACT [VX]
synonym: "AUC Extrap" RELATED [VX]
synonym: "AUC INF (24h)" RELATED [VX]
synonym: "AUC Inf" EXACT [VX]
synonym: "AUC extrap." RELATED [VX]
synonym: "AUC inf" EXACT [VX]
synonym: "AUC(0)" EXACT [VX]
synonym: "AUC(0- )" EXACT [VX]
synonym: "AUC(0-inf )" EXACT [VX]
synonym: "AUC(0-inf)" EXACT [VX]
synonym: "AUC(inf)" EXACT [VX]
synonym: "AUC0-INF" EXACT [VX]
synonym: "AUC0-i" EXACT [VX]
synonym: "AUC0-inf" EXACT [VX]
synonym: "AUCIFO" EXACT [SEND]
synonym: "AUCINF" EXACT [VX]
synonym: "AUCextr" RELATED [VX]
synonym: "AUCextra" RELATED [VX]
synonym: "AUCinf" EXACT [VX]
synonym: "AUCinfinity" RELATED [VX]
synonym: "Area under plasma concentration-time curve from zero to infinity (AUC)" RELATED [VX]
synonym: "Area under the plasma concentration time curve to infinity (AUC)" RELATED [VX]
synonym: "Area under the plasma concentration-time curve from zero to infinity (AUC)" RELATED [VX]
synonym: "Mean AUC inf" EXACT [VX]
is_a: terms:085493 ! terms_C85493

[Term]
id: terms:085763
name: AUC %Back Extrapolation Obs
def: "Applies only for intravascular bolus dosing. The area under the curve (AUC) from the first measured concentration value back extrapolated to the concentration value at time zero as a percentage of the area under the curve extrapolated to infinity using the observed value of the last non-zero concentration."[]
is_a: terms:085493 ! terms_C85493

[Term]
id: terms:085764
name: AUC %Extrapolation Obs
def: "The area under the curve (AUC) from the last observed non-zero concentration value to infinity as a percentage of the area under the curve extrapolated to infinity."[]
synonym: "Percent AUC extrapolated (model independent analysis)" RELATED [VX]
is_a: terms:085493 ! terms_C85493

[Term]
id: terms:085765
name: AUMC Infinity Obs
def: "The area under the moment curve (AUMC) extrapolated to infinity, calculated using the observed value of the last non-zero concentration."[]
is_a: terms:085493 ! terms_C85493

[Term]
id: terms:085766
name: AUMC % Extrapolation Obs
def: "The area under the moment curve (AUMC) from the last observed non-zero concentration value to infinity as a percentage of the area under the moment curve extrapolated to infinity."[]
is_a: terms:085493 ! terms_C85493

[Term]
id: terms:085767
name: AURC Infinity Obs
def: "The area under the urinary excretion rate curve (AURC) extrapolated to infinity, calculated using the observed value of the last excretion rate."[]
is_a: terms:085493 ! terms_C85493

[Term]
id: terms:085768
name: AURC % Extrapolation Obs
def: "The area under the urinary excretion rate curve (AURC) from the last observed non-zero rate value to infinity as a percentage of the area under the urinary excretion rate curve extrapolated to infinity."[]
is_a: terms:085493 ! terms_C85493

[Term]
id: terms:085770
name: Vol Dist Steady State Obs
def: "The volume of distribution at steady state based on the observed CLST for a substance administered by intravascular dosing."[]
synonym: "V dss" RELATED [VX]
synonym: "VSS" RELATED [VX]
synonym: "VSSO" EXACT [SEND]
synonym: "Vdss" RELATED [VX]
synonym: "Vss" RELATED [VX]
synonym: "Vss1" RELATED [VX]
synonym: "Vss_Obs" RELATED [VX]
is_a: terms:085493 ! terms_C85493

[Term]
id: terms:085772
name: Total CL Obs by F
def: "The total body clearance for extravascular administration divided by the fraction of dose absorbed, calculated using the observed value of the last non-zero concentration."[]
synonym: "CL/F (multiple dose)" RELATED [VX]
synonym: "CL/F (single dose)" RELATED [VX]
synonym: "CL/F after 2d dose" RELATED [VX]
synonym: "CLFO" EXACT [SEND]
synonym: "Cl (observed)/F" RELATED [VX]
synonym: "Cl/f" RELATED [VX]
synonym: "Clearance/F" RELATED [VX]
is_a: terms:085493 ! terms_C85493

[Term]
id: terms:085773
name: Total CL Obs
def: "The total body clearance for intravascular administration, calculated using the observed value of the last non-zero concentration."[]
synonym: "CL blood" RELATED [VX]
synonym: "CLO" EXACT [SEND]
synonym: "CL_TOTAL" RELATED [VX]
synonym: "CLa" RELATED [VX]
synonym: "CLoral" RELATED [VX]
synonym: "CLplasma" RELATED [VX]
synonym: "CLs" RELATED [VX]
synonym: "CLtot" RELATED [VX]
synonym: "Cl" RELATED [VX]
synonym: "Cl (blood clearance)" RELATED [VX]
synonym: "Cl total plasma" RELATED [VX]
synonym: "Cl_Obs" RELATED [VX]
synonym: "Cl_obs(mean Day1/Day5)" RELATED [VX]
synonym: "Clearance" RELATED [VX]
synonym: "Clearance (CL(0-24))" RELATED [VX]
synonym: "Clearance (CL(24-336))" RELATED [VX]
synonym: "Clearance (CL)" RELATED [VX]
synonym: "Clearance (CL) (model dependent analysis)" RELATED [VX]
synonym: "Clearance (CL) (model independent analysis)" RELATED [VX]
synonym: "Clearance (CL) plasma" RELATED [VX]
synonym: "Clnf" RELATED [VX]
synonym: "Mean total body clearance (CL)" RELATED [VX]
synonym: "Plasma clearance" RELATED [VX]
synonym: "Plasma clearance (CL)" RELATED [VX]
synonym: "Total plasma clearance" RELATED [VX]
is_a: terms:085493 ! terms_C85493

[Term]
id: terms:085774
name: Vz Obs
def: "The volume of distribution associated with the terminal slope following intravascular administration, calculated using the observed value of the last non-zero concentration."[]
synonym: "V" RELATED [VX]
synonym: "V 1" RELATED [VX]
synonym: "VZ" RELATED [VX]
synonym: "VZO" EXACT [SEND]
synonym: "Volume of distribution" RELATED [VX]
synonym: "Volume of distribution (Vz)" RELATED [VX]
synonym: "Vz" RELATED [VX]
synonym: "Vz obs(mean Day1/Day5)" RELATED [VX]
synonym: "Vz-obs" EXACT [VX]
is_a: terms:085493 ! terms_C85493

[Term]
id: terms:085775
name: Vz Obs by F
def: "The volume of distribution associated with the terminal slope following extravascular administration divided by the fraction of dose absorbed, calculated using the observed value of the last non-zero concentration."[]
synonym: "Vz (observed)/F" RELATED [VX]
synonym: "Vz/F" RELATED [VX]
is_a: terms:085493 ! terms_C85493

[Term]
id: terms:085785
name: AUC Infinity Pred
def: "The area under the curve (AUC) extrapolated to infinity, calculated using the predicted value of the last non-zero concentration."[]
synonym: "AUC predicted to infinity" RELATED [VX]
synonym: "AUCIFP" EXACT [SEND]
is_a: terms:085493 ! terms_C85493

[Term]
id: terms:085786
name: AUC Infinity Pred Norm by Dose
def: "The area under the curve (AUC) extrapolated to infinity, calculated using the predicted value of the last non-zero concentration, divided by the dose."[]
is_a: terms:085493 ! terms_C85493

[Term]
id: terms:085787
name: AUC %Back Extrapolation Pred
def: "Applies only for intravascular bolus dosing. The area under the curve (AUC) from the first measured concentration value back extrapolated to the concentration value at time zero as a percentage of the area under the curve extrapolated to infinity using the predicted value of the last non-zero concentration."[]
is_a: terms:085493 ! terms_C85493

[Term]
id: terms:085788
name: AUC %Extrapolation Pred
def: "The area under the curve (AUC) from the last predicted non-zero concentration value to infinity as a percentage of the area under the curve extrapolated to infinity."[]
synonym: "AUCPEP" EXACT [SEND]
is_a: terms:085493 ! terms_C85493

[Term]
id: terms:085789
name: AUMC Infinity Pred
def: "The area under the moment curve (AUMC) extrapolated to infinity, calculated using the predicted value of the last non-zero concentration."[]
is_a: terms:085493 ! terms_C85493

[Term]
id: terms:085790
name: AUMC % Extrapolation Pred
def: "The area under the moment curve (AUMC) from the last predicted non-zero concentration value to infinity as a percentage of the area under the moment curve extrapolated to infinity."[]
is_a: terms:085493 ! terms_C85493

[Term]
id: terms:085791
name: AURC Infinity Pred
def: "The area under the urinary excretion rate curve (AURC) extrapolated to infinity, calculated using the predicted value of the last non-zero excretion rate."[]
is_a: terms:085493 ! terms_C85493

[Term]
id: terms:085792
name: AURC % Extrapolation Pred
def: "The area under the urinary excretion rate curve (AURC) from the last predicted non-zero rate value to infinity as a percentage of the area under the urinary excretion rate curve extrapolated to infinity."[]
is_a: terms:085493 ! terms_C85493

[Term]
id: terms:085794
name: Vol Dist Steady State Pred
def: "The volume of distribution at steady state based on the predicted CLST for a substance administered by intravascular dosing."[]
is_a: terms:085493 ! terms_C85493

[Term]
id: terms:085796
name: Total CL Pred by F
def: "The total body clearance for extravascular administration divided by the fraction of dose absorbed, calculated using the predicted value of the last non-zero concentration."[]
is_a: terms:085493 ! terms_C85493

[Term]
id: terms:085797
name: Total CL Pred
def: "The total body clearance for intravascular administration, calculated using the predicted value of the last non-zero concentration."[]
is_a: terms:085493 ! terms_C85493

[Term]
id: terms:085798
name: Vz Pred
def: "The volume of distribution associated with the terminal slope following intravascular administration, calculated using the predicted value of the last non-zero concentration."[]
is_a: terms:085493 ! terms_C85493

[Term]
id: terms:085799
name: Vz Pred by F
def: "The volume of distribution associated with the terminal slope following extravascular administration divided by the fraction of dose absorbed, calculated using the predicted value of the last non-zero concentration."[]
is_a: terms:085493 ! terms_C85493

[Term]
id: terms:085816
name: Number of Points for Lambda z
def: "The number of time points used in computing Lambda z."[]
is_a: terms:085493 ! terms_C85493

[Term]
id: terms:085817
name: Sum of Urine Vol
def: "The sum of urine volumes that are used for PK parameters."[]
is_a: terms:085493 ! terms_C85493

[Term]
id: terms:085818
name: Half-Life Lambda z
def: "Terminal half-life."[]
synonym: "Elimination half-life (t1/2)" RELATED [VX]
synonym: "HALFLIFE_Z" RELATED [VX]
synonym: "Half-life (model independent analysis)" RELATED [VX]
synonym: "Half-life (t1/2_lambda_z)" RELATED [VX]
synonym: "Half-life alpha" RELATED [VX]
synonym: "LAMZHL" EXACT [SEND]
synonym: "Lz" RELATED [VX]
synonym: "Seminal ves. (contour) t1/2 lambda z" RELATED [VX]
synonym: "T 1/2z" NARROW [VX]
synonym: "T1/2 lambda z" RELATED [VX]
synonym: "T1/2,z" RELATED [VX]
synonym: "T1/2yz" RELATED [VX]
synonym: "T1/2z" NARROW [VX]
synonym: "Terminal T1/2" EXACT [VX]
synonym: "Terminal haif-life (t1/2z)" RELATED [VX]
synonym: "Terminal half-life" RELATED [VX]
synonym: "Terminal half-life (T1/2z)" RELATED [VX]
synonym: "Terminal half-life (t1/2)" RELATED [VX]
synonym: "Terminal half-life (t1/2z)" RELATED [VX]
synonym: "Terminal half-life in blood (t1/2)" RELATED [VX]
synonym: "The apparent terminal half-life" RELATED [VX]
synonym: "The apparent terminal half-life t 1/2" RELATED [VX]
synonym: "The terminal time half-life" RELATED [VX]
synonym: "k lambda 1" RELATED [VX]
synonym: "k lambda 1 blood" RELATED [VX]
synonym: "k lambda 2" RELATED [VX]
synonym: "k lambda 2  blood" RELATED [VX]
synonym: "k lambda 2 blood" RELATED [VX]
synonym: "k lambda z" RELATED [VX]
synonym: "k lambda z  blood" RELATED [VX]
synonym: "k lambda z blood" RELATED [VX]
synonym: "k lambda1" RELATED [VX]
synonym: "k lambda2" RELATED [VX]
synonym: "k lambda3" RELATED [VX]
synonym: "lambda 1" RELATED [VX]
synonym: "lambda 2" RELATED [VX]
synonym: "lambda 3" RELATED [VX]
synonym: "t 1/2 Z" NARROW [VX]
synonym: "t 1/2 z" NARROW [VX]
synonym: "t 1/2z" NARROW [VX]
synonym: "t(1/2)_lambda_z" NARROW [VX]
synonym: "t(1/2)z" NARROW [VX]
synonym: "t1/2 lambda 1" RELATED [VX]
synonym: "t1/2 lambda 1 blood" RELATED [VX]
synonym: "t1/2 lambda 2" RELATED [VX]
synonym: "t1/2 lambda 2  blood" RELATED [VX]
synonym: "t1/2 lambda 2 blood" RELATED [VX]
synonym: "t1/2 lambda 3" RELATED [VX]
synonym: "t1/2 lambda z" RELATED [VX]
synonym: "t1/2 lambda z  blood" RELATED [VX]
synonym: "t1/2 lambda z blood" RELATED [VX]
synonym: "t1/2 lambda1" RELATED [VX]
synonym: "t1/2 lambda2" RELATED [VX]
synonym: "t1/2 lambda3" RELATED [VX]
synonym: "t1/2 terminal" RELATED [VX]
synonym: "t1/2/z" RELATED [VX]
synonym: "t1/2/z" RELATED [VX]
synonym: "t1/2lambdaz" RELATED [VX]
synonym: "t1/2z" NARROW [VX]
is_a: terms:085493 ! terms_C85493

[Term]
id: terms:085821
name: Correlation Between TimeX and Log ConcY
def: "The correlation between time (X) and log concentration (Y) for the points used in the estimation of lambda z."[]
is_a: terms:085493 ! terms_C85493

[Term]
id: terms:085822
name: Time of Last Nonzero Conc
def: "The time of the last measurable (positive) concentration."[]
synonym: "T last" RELATED [VX]
synonym: "T last (1st treatment)" RELATED [VX]
synonym: "T last (3rd treatment)" RELATED [VX]
synonym: "T lsat (2nd treatment)" RELATED [VX]
synonym: "T(last)" RELATED [VX]
synonym: "TLST" EXACT [SEND]
synonym: "Time corresponding to C inf (t inf)" RELATED [VX]
synonym: "Time corresponding to C last (t last)" RELATED [VX]
synonym: "Time to reach last quantifiable plasma concentration (t)" RELATED [VX]
synonym: "Tlast" RELATED [VX]
synonym: "t last" RELATED [VX]
synonym: "tlast" RELATED [VX]
is_a: terms:085493 ! terms_C85493

[Term]
id: terms:085823
name: Midpoint of Interval of Maximum ER
def: "The midpoint of collection interval associated with the maximum excretion rate."[]
is_a: terms:085493 ! terms_C85493

[Term]
id: terms:085824
name: Time Until First Nonzero Conc
def: "The time prior to the first measurable (non-zero) concentration."[]
synonym: "tlag" EXACT [VX]
is_a: terms:085493 ! terms_C85493

[Term]
id: terms:085825
name: Time of CMIN Observation
def: "The time of minimum concentration sampled during a dosing interval."[]
synonym: "TMIN" EXACT [VX]
synonym: "Tmin" EXACT [VX]
is_a: terms:085493 ! terms_C85493

[Term]
id: terms:085841
name: AURC All
def: "The area under the urinary excretion rate curve (AURC) from time zero to the time of the last observation, regardless of whether the last observation is a measurable concentration or not."[]
is_a: terms:085493 ! terms_C85493

[Term]
id: terms:092305
name: AUC to Last Nonzero Conc Norm by WT
def: "The area under the curve (AUC) from the time of dosing to the last measurable concentration divided by the weight."[]
is_a: terms:085493 ! terms_C85493

[Term]
id: terms:092306
name: AUC All Norm by Dose
def: "The area under the curve (AUC) from the time of dosing to the time of the last observation divided by the dose, regardless of whether the last concentration is measurable or not."[]
synonym: "AUC (0-12)/dose" RELATED [VX]
synonym: "AUC (0-24) norm" RELATED [VX]
synonym: "AUC (0-24h)/Dose (recovery animals)" RELATED [VX]
synonym: "AUC (0-t)/Dose" RELATED [VX]
synonym: "AUC (dose corrected)" NARROW [VX]
synonym: "AUC (mean)" RELATED [VX]
synonym: "AUC (t)" RELATED [VX]
synonym: "AUC 0-24/Dose" RELATED [VX]
synonym: "AUC 0-24/dose" RELATED [VX]
synonym: "AUC 0-5h/dose" RELATED [VX]
synonym: "AUC last (0-24h)/dose" RELATED [VX]
synonym: "AUC norm." RELATED [VX]
synonym: "AUC(0-24 h) norm." RELATED [VX]
synonym: "AUC(0-24 h)/dose" RELATED [VX]
synonym: "AUC(0-24 mg" RELATED [VX]
synonym: "AUC(0-24) (NJH)/Dose" RELATED [VX]
synonym: "AUC(0-24) (dose-normalized)" RELATED [VX]
synonym: "AUC(0-24) (normalised to dose 100 mg/kg)" RELATED [VX]
synonym: "AUC(0-24) / dose" RELATED [VX]
synonym: "AUC(0-24) /dose" RELATED [VX]
synonym: "AUC(0-24) dose normalized" RELATED [VX]
synonym: "AUC(0-24) norm" RELATED [VX]
synonym: "AUC(0-24)h ratio" RELATED [VX]
synonym: "AUC(0-24)norm" RELATED [VX]
synonym: "AUC(0-24/dose" RELATED [VX]
synonym: "AUC(0-24h) /Dose" RELATED [VX]
synonym: "AUC(0-24h)/ dose" RELATED [VX]
synonym: "AUC(0-24h)/Dose" RELATED [VX]
synonym: "AUC(0-24h)/dose" RELATED [VX]
synonym: "AUC(0-24h)/dose ratio" RELATED [VX]
synonym: "AUC(0-24hr)/dose" RELATED [VX]
synonym: "AUC(0-3)/dose" RELATED [VX]
synonym: "AUC(0-48)/Dose" RELATED [VX]
synonym: "AUC(0-48h)/Dose" RELATED [VX]
synonym: "AUC(0-7)norm" RELATED [VX]
synonym: "AUC(0-8h)/dose" RELATED [VX]
synonym: "AUC(0-Tlast)/dose" NARROW [VX]
synonym: "AUC(0-tlast)/D plasma" RELATED [VX]
synonym: "AUC(0-tn)norm" RELATED [VX]
synonym: "AUC/D" RELATED [VX]
synonym: "AUC/DOSE" NARROW [VX]
synonym: "AUC/Dose" NARROW [VX]
synonym: "AUC/Dose (Testes)" RELATED [VX]
synonym: "AUC/Dose (Whole Blood)" RELATED [VX]
synonym: "AUC/d" RELATED [VX]
synonym: "AUC/dose" NARROW [VX]
synonym: "AUC/dose as free base" RELATED [VX]
synonym: "AUC/dose as salt form" RELATED [VX]
synonym: "AUC/mg/kg" RELATED [VX]
synonym: "AUC0-24 h vs. lower dose" RELATED [VX]
synonym: "AUC0-24 h/Dose" RELATED [VX]
synonym: "AUC0-24 hr /Dose" RELATED [VX]
synonym: "AUC0-24/Dose" RELATED [VX]
synonym: "AUC0-24/dose" RELATED [VX]
synonym: "AUC0-INF vs. lower dose" RELATED [VX]
synonym: "AUC0-inf/Dose" RELATED [VX]
synonym: "AUC0-t/dose" RELATED [VX]
synonym: "AUCALLD" EXACT [SEND]
synonym: "AUCnorm" RELATED [VX]
synonym: "AUCu(0-24)norm" RELATED [VX]
synonym: "AUD/dose" RELATED [VX]
synonym: "Area under curve normalized by dose (AUC/dose)" RELATED [VX]
synonym: "Area under the curve normalized by the dose (AUC(0-9)/dose)" RELATED [VX]
synonym: "Dose normalised AUC" RELATED [VX]
synonym: "Dose normalised AUC(0-24)" RELATED [VX]
synonym: "Dose normalised AUC(0-24) (AUC(0-24)/dose)" RELATED [VX]
synonym: "Dose normalised AUC0-24 (AUC(0-24)/dose)" RELATED [VX]
synonym: "Dose normalized AUC(0-24)" RELATED [VX]
synonym: "Dose-normalized AUC(0-24h) (AUC(0-24h)/dose)" RELATED [VX]
synonym: "Mean AUC (0-24h)/dose" RELATED [VX]
synonym: "Norm AUC" RELATED [VX]
synonym: "Norm. AUC" RELATED [VX]
synonym: "Normalised AUC" RELATED [VX]
synonym: "Plasma  radioactivity" RELATED [VX]
synonym: "Plasma radioactivity" RELATED [VX]
is_a: terms:085493 ! terms_C85493

[Term]
id: terms:092307
name: AUC All Norm by SA
def: "The area under the curve (AUC) from the time of dosing to the time of the last observation divided by the surface area, regardless of whether the last concentration is measurable or not."[]
is_a: terms:085493 ! terms_C85493

[Term]
id: terms:092308
name: AUC All Norm by WT
def: "The area under the curve (AUC) from the time of dosing to the time of the last observation divided by the weight, regardless of whether the last concentration is measurable or not."[]
is_a: terms:085493 ! terms_C85493

[Term]
id: terms:092309
name: AUC to Last Nonzero Conc Norm by BMI
def: "The area under the curve (AUC) from the time of dosing to the last measurable concentration divided by the body mass index."[]
is_a: terms:085493 ! terms_C85493

[Term]
id: terms:092310
name: AUC to Last Nonzero Conc Norm by Dose
def: "The area under the curve (AUC) from the time of dosing to the last measurable concentration divided by the dose."[]
synonym: "AUClast/Dose" RELATED [VX]
is_a: terms:085493 ! terms_C85493

[Term]
id: terms:092311
name: AUC to Last Nonzero Conc Norm by SA
def: "The area under the curve (AUC) from the time of dosing to the last measurable concentration divided by the surface area."[]
is_a: terms:085493 ! terms_C85493

[Term]
id: terms:092312
name: AUC from T1 to T2 Norm by BMI
def: "The area under the curve (AUC) over the interval from T1 to T2 divided by the body mass index."[]
is_a: terms:085493 ! terms_C85493

[Term]
id: terms:092313
name: AUC from T1 to T2 Norm by Dose
def: "The area under the curve (AUC) over the interval from T1 to T2 divided by the dose."[]
synonym: "AUC (0-24)/D" NARROW [VX]
synonym: "AUC (0-24)/Dose" RELATED [VX]
synonym: "AUC (0-24)/dose" NARROW [VX]
synonym: "AUC (0-24h)/Dose" NARROW [VX]
synonym: "AUC (0-24h)/dose" NARROW [VX]
synonym: "AUC 0-24/D" NARROW [VX]
synonym: "AUC 0-24h/Dose" NARROW [VX]
synonym: "AUC 0-24h/dose" NARROW [VX]
synonym: "AUC(0-24)/D" RELATED [VX]
synonym: "AUC(0-24)/Dose" NARROW [VX]
synonym: "AUC(0-24)/d" NARROW [VX]
synonym: "AUC(0-24)/dose" NARROW [VX]
synonym: "AUC(0.0833-24h)/dose" NARROW [VX]
synonym: "AUC90-24h) (dose normalized)" RELATED [VX]
synonym: "AUCINTD" EXACT [SEND]
synonym: "Dose-normalized AUC(0.17-t)" RELATED [VX]
is_a: terms:085493 ! terms_C85493

[Term]
id: terms:092314
name: AUC from T1 to T2 Norm by SA
def: "The area under the curve (AUC) over the interval from T1 to T2 divided by the surface area."[]
is_a: terms:085493 ! terms_C85493

[Term]
id: terms:092315
name: AUC from T1 to T2 Norm by WT
def: "The area under the curve (AUC) over the interval from T1 to T2 divided by the weight."[]
is_a: terms:085493 ! terms_C85493

[Term]
id: terms:092316
name: AUC Infinity Obs Norm by BMI
def: "The area under the curve (AUC) extrapolated to infinity, calculated using the observed value of the last non-zero concentration, divided by the body mass index."[]
is_a: terms:085493 ! terms_C85493

[Term]
id: terms:092317
name: AUC Infinity Obs Norm by SA
def: "The area under the curve (AUC) extrapolated to infinity, calculated using the observed value of the last non-zero concentration, divided by the surface area."[]
is_a: terms:085493 ! terms_C85493

[Term]
id: terms:092318
name: AUC Infinity Obs Norm by WT
def: "The area under the curve (AUC) extrapolated to infinity, calculated using the observed value of the last non-zero concentration, divided by the weight."[]
is_a: terms:085493 ! terms_C85493

[Term]
id: terms:092319
name: AUC Infinity Pred Norm by BMI
def: "The area under the curve (AUC) extrapolated to infinity, calculated using the predicted value of the last non-zero concentration, divided by the body mass index."[]
is_a: terms:085493 ! terms_C85493

[Term]
id: terms:092320
name: AUC Infinity Pred Norm by SA
def: "The area under the curve (AUC) extrapolated to infinity, calculated using the predicted value of the last non-zero concentration, divided by the surface area."[]
is_a: terms:085493 ! terms_C85493

[Term]
id: terms:092321
name: AUC Infinity Pred Norm by WT
def: "The area under the curve (AUC) extrapolated to infinity, calculated using the predicted value of the last non-zero concentration, divided by the weight."[]
is_a: terms:085493 ! terms_C85493

[Term]
id: terms:092322
name: AUC Over Dosing Interval Norm by BMI
def: "The area under the curve (AUC) for the defined interval between doses (TAU) divided by the body mass index."[]
is_a: terms:085493 ! terms_C85493

[Term]
id: terms:092323
name: AUC Over Dosing Interval Norm by Dose
def: "The area under the curve (AUC) for the defined interval between doses (TAU) divided by the dose."[]
is_a: terms:085493 ! terms_C85493

[Term]
id: terms:092324
name: AUC Over Dosing Interval Norm by SA
def: "The area under the curve (AUC) for the defined interval between doses (TAU) divided by the surface area."[]
is_a: terms:085493 ! terms_C85493

[Term]
id: terms:092325
name: AUC Over Dosing Interval Norm by WT
def: "The area under the curve (AUC) for the defined interval between doses (TAU) divided by the weight."[]
is_a: terms:085493 ! terms_C85493

[Term]
id: terms:092326
name: AUMC to Last Nonzero Conc Norm by BMI
def: "The area under the moment curve (AUMC) from the time of dosing to the last measurable concentration divided by the body mass index."[]
is_a: terms:085493 ! terms_C85493

[Term]
id: terms:092327
name: AUMC to Last Nonzero Conc Norm by Dose
def: "The area under the moment curve (AUMC) from the time of dosing to the last measurable concentration divided by the dose."[]
is_a: terms:085493 ! terms_C85493

[Term]
id: terms:092328
name: AUMC to Last Nonzero Conc Norm by SA
def: "The area under the moment curve (AUMC) from the time of dosing to the last measurable concentration divided by the surface area."[]
is_a: terms:085493 ! terms_C85493

[Term]
id: terms:092329
name: AUMC to Last Nonzero Conc Norm by WT
def: "The area under the moment curve (AUMC) from the time of dosing to the last measurable concentration divided by the weight."[]
is_a: terms:085493 ! terms_C85493

[Term]
id: terms:092330
name: AUMC Infinity Obs Norm by BMI
def: "The area under the moment curve (AUMC) extrapolated to infinity, calculated using the observed value of the last non-zero concentration, divided by the body mass index."[]
is_a: terms:085493 ! terms_C85493

[Term]
id: terms:092331
name: AUMC Infinity Obs Norm by Dose
def: "The area under the moment curve (AUMC) extrapolated to infinity, calculated using the observed value of the last non-zero concentration, divided by the dose."[]
is_a: terms:085493 ! terms_C85493

[Term]
id: terms:092332
name: AUMC Infinity Obs Norm by SA
def: "The area under the moment curve (AUMC) extrapolated to infinity, calculated using the observed value of the last non-zero concentration, divided by the surface area."[]
is_a: terms:085493 ! terms_C85493

[Term]
id: terms:092333
name: AUMC Infinity Obs Norm by WT
def: "The area under the moment curve (AUMC) extrapolated to infinity, calculated using the observed value of the last non-zero concentration, divided by the weight."[]
is_a: terms:085493 ! terms_C85493

[Term]
id: terms:092334
name: AUMC Infinity Pred Norm by BMI
def: "The area under the moment curve (AUMC) extrapolated to infinity, calculated using the predicted value of the last non-zero concentration, divided by the body mass index."[]
is_a: terms:085493 ! terms_C85493

[Term]
id: terms:092335
name: AUMC Infinity Pred Norm by Dose
def: "The area under the moment curve (AUMC) extrapolated to infinity, calculated using the predicted value of the last non-zero concentration, divided by the dose."[]
is_a: terms:085493 ! terms_C85493

[Term]
id: terms:092336
name: AUMC Infinity Pred Norm by SA
def: "The area under the moment curve (AUMC) extrapolated to infinity, calculated using the predicted value of the last non-zero concentration, divided by the surface area."[]
is_a: terms:085493 ! terms_C85493

[Term]
id: terms:092337
name: AUMC Infinity Pred Norm by WT
def: "The area under the moment curve (AUMC) extrapolated to infinity, calculated using the predicted value of the last non-zero concentration, divided by the weight."[]
is_a: terms:085493 ! terms_C85493

[Term]
id: terms:092338
name: AUMC Over Dosing Interval Norm by BMI
def: "The area under the first moment curve (AUMC) for the defined interval between doses (TAU) divided by the body mass index."[]
is_a: terms:085493 ! terms_C85493

[Term]
id: terms:092339
name: AUMC Over Dosing Interval Norm by Dose
def: "The area under the first moment curve (AUMC) for the defined interval between doses (TAU) divided by the dose."[]
is_a: terms:085493 ! terms_C85493

[Term]
id: terms:092340
name: AUMC Over Dosing Interval Norm by SA
def: "The area under the first moment curve (AUMC) for the defined interval between doses (TAU) divided by the surface area."[]
is_a: terms:085493 ! terms_C85493

[Term]
id: terms:092341
name: AUMC Over Dosing Interval Norm by WT
def: "The area under the first moment curve (AUMC) for the defined interval between doses (TAU) divided by the weight."[]
is_a: terms:085493 ! terms_C85493

[Term]
id: terms:092342
name: AURC All Norm by BMI
def: "The area under the urinary excretion rate curve (AURC) from time zero to the last measurable rate divided by the body mass index."[]
is_a: terms:085493 ! terms_C85493

[Term]
id: terms:092343
name: AURC All Norm by Dose
def: "The area under the urinary excretion rate curve (AURC) from time zero to the last measurable rate divided by the dose."[]
is_a: terms:085493 ! terms_C85493

[Term]
id: terms:092344
name: AURC All Norm by SA
def: "The area under the urinary excretion rate curve (AURC) from time zero to the last measurable rate divided by the surface area."[]
is_a: terms:085493 ! terms_C85493

[Term]
id: terms:092345
name: AURC All Norm by WT
def: "The area under the urinary excretion rate curve (AURC) from time zero to the last measurable rate divided by the weight."[]
is_a: terms:085493 ! terms_C85493

[Term]
id: terms:092346
name: AURC Dosing to Last Conc Norm by BMI
def: "The area under the urinary excretion rate curve (AURC) from time zero to the last measurable rate, divided by the body mass index."[]
is_a: terms:085493 ! terms_C85493

[Term]
id: terms:092347
name: AURC Dosing to Last Conc Norm by Dose
def: "The area under the urinary excretion rate curve (AURC) from time zero to the last measurable rate, divided by the dose."[]
is_a: terms:085493 ! terms_C85493

[Term]
id: terms:092348
name: AURC Dosing to Last Conc Norm by SA
def: "The area under the urinary excretion rate curve (AURC) from time zero to the last measurable rate, divided by the surface area."[]
is_a: terms:085493 ! terms_C85493

[Term]
id: terms:092349
name: AURC Dosing to Last Conc Norm by WT
def: "The area under the urinary excretion rate curve (AURC) from time zero to the last measurable rate, divided by the weight."[]
is_a: terms:085493 ! terms_C85493

[Term]
id: terms:092350
name: AURC from T1 to T2 Norm by BMI
def: "The area under the urinary excretion rate curve (AURC) over the interval from T1 to T2 divided by the body mass index."[]
is_a: terms:085493 ! terms_C85493

[Term]
id: terms:092351
name: AURC from T1 to T2 Norm by Dose
def: "The area under the urinary excretion rate curve (AURC) over the interval from T1 to T2 divided by the dose."[]
is_a: terms:085493 ! terms_C85493

[Term]
id: terms:092352
name: AURC from T1 to T2 Norm by SA
def: "The area under the urinary excretion rate curve (AURC) over the interval from T1 to T2 divided by the surface area."[]
is_a: terms:085493 ! terms_C85493

[Term]
id: terms:092353
name: AURC from T1 to T2 Norm by WT
def: "The area under the urinary excretion rate curve (AURC) over the interval from T1 to T2 divided by the weight."[]
is_a: terms:085493 ! terms_C85493

[Term]
id: terms:092354
name: AURC Infinity Obs Norm by BMI
def: "The area under the urinary excretion rate curve (AURC) extrapolated to infinity, calculated using the observed value of the last excretion rate, divided by the body mass index."[]
is_a: terms:085493 ! terms_C85493

[Term]
id: terms:092355
name: AURC Infinity Obs Norm by Dose
def: "The area under the urinary excretion rate curve (AURC) extrapolated to infinity, calculated using the observed value of the last excretion rate, divided by the dose."[]
is_a: terms:085493 ! terms_C85493

[Term]
id: terms:092356
name: AURC Infinity Obs Norm by SA
def: "The area under the urinary excretion rate curve (AURC) extrapolated to infinity, calculated using the observed value of the last excretion rate, divided by the surface area."[]
is_a: terms:085493 ! terms_C85493

[Term]
id: terms:092357
name: AURC Infinity Obs Norm by WT
def: "The area under the urinary excretion rate curve (AURC) extrapolated to infinity, calculated using the observed value of the last excretion rate, divided by the weight."[]
is_a: terms:085493 ! terms_C85493

[Term]
id: terms:092358
name: AURC Infinity Pred Norm by BMI
def: "The area under the urinary excretion rate curve (AURC) extrapolated to infinity, calculated using the predicted value of the last non-zero excretion rate, divded by the body mass index."[]
is_a: terms:085493 ! terms_C85493

[Term]
id: terms:092359
name: AURC Infinity Pred Norm by Dose
def: "The area under the urinary excretion rate curve (AURC) extrapolated to infinity, calculated using the predicted value of the last non-zero excretion rate, divded by the dose."[]
is_a: terms:085493 ! terms_C85493

[Term]
id: terms:092360
name: AURC Infinity Pred Norm by SA
def: "The area under the urinary excretion rate curve (AURC) extrapolated to infinity, calculated using the predicted value of the last non-zero excretion rate, divded by the surface area."[]
is_a: terms:085493 ! terms_C85493

[Term]
id: terms:092361
name: AURC Infinity Pred Norm by WT
def: "The area under the urinary excretion rate curve (AURC) extrapolated to infinity, calculated using the predicted value of the last non-zero excretion rate, divded by the weight."[]
is_a: terms:085493 ! terms_C85493

[Term]
id: terms:092362
name: AUC All Norm by BMI
def: "The area under the curve (AUC) from the time of dosing to the time of the last observation divided by the body mass index, regardless of whether the last concentration is measurable or not."[]
is_a: terms:085493 ! terms_C85493

[Term]
id: terms:092367
name: Average Conc Norm by BMI
def: "AUCTAU divided by TAU and then divided by the body mass index."[]
is_a: terms:085493 ! terms_C85493

[Term]
id: terms:092368
name: Average Conc Norm by Dose
def: "AUCTAU divided by TAU and then divided by the dose."[]
is_a: terms:085493 ! terms_C85493

[Term]
id: terms:092369
name: Average Conc Norm by SA
def: "AUCTAU divided by TAU and then divided by the surface area."[]
is_a: terms:085493 ! terms_C85493

[Term]
id: terms:092370
name: Average Conc Norm by WT
def: "AUCTAU divided by TAU and then divided by the weight."[]
is_a: terms:085493 ! terms_C85493

[Term]
id: terms:092371
name: Max Conc Norm by BMI
def: "The maximum concentration occurring at Tmax, divided by the body mass index."[]
is_a: terms:085493 ! terms_C85493

[Term]
id: terms:092372
name: Max Conc Norm by SA
def: "The maximum concentration occurring at Tmax, divided by the surface area."[]
is_a: terms:085493 ! terms_C85493

[Term]
id: terms:092373
name: Max Conc Norm by WT
def: "The maximum concentration occurring at Tmax, divided by the weight."[]
is_a: terms:085493 ! terms_C85493

[Term]
id: terms:092374
name: Min Conc Norm by BMI
def: "The minimum concentration between dose time and dose time plus Tau (at Tmin) divided by the body mass index."[]
is_a: terms:085493 ! terms_C85493

[Term]
id: terms:092375
name: Min Conc Norm by Dose
def: "The minimum concentration between dose time and dose time plus Tau (at Tmin) divided by the dose."[]
is_a: terms:085493 ! terms_C85493

[Term]
id: terms:092376
name: Min Conc Norm by SA
def: "The minimum concentration between dose time and dose time plus Tau (at Tmin) divided by the surface area."[]
is_a: terms:085493 ! terms_C85493

[Term]
id: terms:092377
name: Min Conc Norm by WT
def: "The minimum concentration between dose time and dose time plus Tau (at Tmin) divided by the weight."[]
is_a: terms:085493 ! terms_C85493

[Term]
id: terms:092383
name: Initial Conc Norm by BMI
def: "Initial concentration divided by the body mass index. Given only for bolus IV models."[]
is_a: terms:085493 ! terms_C85493

[Term]
id: terms:092384
name: Initial Conc Norm by Dose
def: "Initial concentration divided by the dose. Given only for bolus IV models."[]
is_a: terms:085493 ! terms_C85493

[Term]
id: terms:092385
name: Initial Conc Norm by SA
def: "Initial concentration divided by the surface area. Given only for bolus IV models."[]
is_a: terms:085493 ! terms_C85493

[Term]
id: terms:092386
name: Initial Conc Norm by WT
def: "Initial concentration divided by the weight. Given only for bolus IV models."[]
is_a: terms:085493 ! terms_C85493

[Term]
id: terms:092387
name: Last Nonzero Conc Norm by BMI
def: "The concentration corresponding to Tlast divided by the body mass index."[]
is_a: terms:085493 ! terms_C85493

[Term]
id: terms:092388
name: Last Nonzero Conc Norm by Dose
def: "The concentration corresponding to Tlast divided by the dose."[]
is_a: terms:085493 ! terms_C85493

[Term]
id: terms:092389
name: Last Nonzero Conc Norm by SA
def: "The concentration corresponding to Tlast divided by the surface area."[]
is_a: terms:085493 ! terms_C85493

[Term]
id: terms:092390
name: Last Nonzero Conc Norm by WT
def: "The concentration corresponding to Tlast divided by the weight."[]
is_a: terms:085493 ! terms_C85493

[Term]
id: terms:092391
name: Last Meas Excretion Rate Norm by BMI
def: "The last measurable (positive) excretion rate divided by the body mass index."[]
is_a: terms:085493 ! terms_C85493

[Term]
id: terms:092392
name: Last Meas Excretion Rate Norm by Dose
def: "The last measurable (positive) excretion rate divided by the dose."[]
is_a: terms:085493 ! terms_C85493

[Term]
id: terms:092393
name: Last Meas Excretion Rate Norm by SA
def: "The last measurable (positive) excretion rate divided by the surface area."[]
is_a: terms:085493 ! terms_C85493

[Term]
id: terms:092394
name: Last Meas Excretion Rate Norm by WT
def: "The last measurable (positive) excretion rate divided by the weight."[]
is_a: terms:085493 ! terms_C85493

[Term]
id: terms:092395
name: Max Excretion Rate Norm by BMI
def: "The maximum excretion rate divided by the body mass index."[]
is_a: terms:085493 ! terms_C85493

[Term]
id: terms:092396
name: Max Excretion Rate Norm by Dose
def: "The maximum excretion rate divided by the dose."[]
is_a: terms:085493 ! terms_C85493

[Term]
id: terms:092397
name: Max Excretion Rate Norm by SA
def: "The maximum excretion rate divided by the surface area."[]
is_a: terms:085493 ! terms_C85493

[Term]
id: terms:092398
name: Max Excretion Rate Norm by WT
def: "The maximum excretion rate divided by the weight."[]
is_a: terms:085493 ! terms_C85493

[Term]
id: terms:092399
name: Total CL Obs by F Norm by BMI
def: "The total body clearance for extravascular administration divided by the fraction of dose absorbed, calculated using the observed value of the last non-zero concentration, divided by the body mass index."[]
is_a: terms:085493 ! terms_C85493

[Term]
id: terms:092400
name: Total CL Obs by F Norm by Dose
def: "The total body clearance for extravascular administration divided by the fraction of dose absorbed, calculated using the observed value of the last non-zero concentration, divided by the dose."[]
is_a: terms:085493 ! terms_C85493

[Term]
id: terms:092401
name: Total CL Obs by F Norm by SA
def: "The total body clearance for extravascular administration divided by the fraction of dose absorbed, calculated using the observed value of the last non-zero concentration, divided by the surface area."[]
is_a: terms:085493 ! terms_C85493

[Term]
id: terms:092402
name: Total CL Obs by F Norm by WT
def: "The total body clearance for extravascular administration divided by the fraction of dose absorbed, calculated using the observed value of the last non-zero concentration, divided by the weight."[]
is_a: terms:085493 ! terms_C85493

[Term]
id: terms:092403
name: Total CL Obs Norm by BMI
def: "The total body clearance for intravascular administration, calculated using the observed value of the last non-zero concentration, divided by the body mass index."[]
is_a: terms:085493 ! terms_C85493

[Term]
id: terms:092404
name: Total CL Obs Norm by Dose
def: "The total body clearance for intravascular administration, calculated using the observed value of the last non-zero concentration, divided by the dose."[]
is_a: terms:085493 ! terms_C85493

[Term]
id: terms:092405
name: Total CL Obs Norm by SA
def: "The total body clearance for intravascular administration, calculated using the observed value of the last non-zero concentration, divided by the surface area."[]
is_a: terms:085493 ! terms_C85493

[Term]
id: terms:092406
name: Total CL Obs Norm by WT
def: "The total body clearance for intravascular administration, calculated using the observed value of the last non-zero concentration, divided by the weight."[]
is_a: terms:085493 ! terms_C85493

[Term]
id: terms:092407
name: Vz Obs Norm by BMI
def: "The volume of distribution associated with the terminal slope following intravascular administration, calculated using the observed value of the last non-zero concentration, divided by the body mass index."[]
is_a: terms:085493 ! terms_C85493

[Term]
id: terms:092408
name: Vz Obs Norm by SA
def: "The volume of distribution associated with the terminal slope following intravascular administration, calculated using the observed value of the last non-zero concentration, divided by the surface area."[]
is_a: terms:085493 ! terms_C85493

[Term]
id: terms:092409
name: Vz Obs Norm by WT
def: "The volume of distribution associated with the terminal slope following intravascular administration, calculated using the observed value of the last non-zero concentration, divided by the weight."[]
is_a: terms:085493 ! terms_C85493

[Term]
id: terms:092410
name: Vz Obs by F Norm by BMI
def: "The volume of distribution associated with the terminal slope following extravascular administration divided by the fraction of dose absorbed, calculated using the observed value of the last non-zero concentration, divided by the body mass index."[]
is_a: terms:085493 ! terms_C85493

[Term]
id: terms:092411
name: Vz Obs by F Norm by SA
def: "The volume of distribution associated with the terminal slope following extravascular administration divided by the fraction of dose absorbed, calculated using the observed value of the last non-zero concentration, divided by the surface area."[]
is_a: terms:085493 ! terms_C85493

[Term]
id: terms:092412
name: Vz Obs by F Norm by WT
def: "The volume of distribution associated with the terminal slope following extravascular administration divided by the fraction of dose absorbed, calculated using the observed value of the last non-zero concentration, divided by the weight."[]
is_a: terms:085493 ! terms_C85493

[Term]
id: terms:092417
name: Total CL Pred by F Norm by BMI
def: "The total body clearance for extravascular administration divided by the fraction of dose absorbed, calculated using the predicted value of the last non-zero concentration, divided by body mass index."[]
is_a: terms:085493 ! terms_C85493

[Term]
id: terms:092418
name: Total CL Pred by F Norm by Dose
def: "The total body clearance for extravascular administration divided by the fraction of dose absorbed, calculated using the predicted value of the last non-zero concentration, divided by the dose."[]
is_a: terms:085493 ! terms_C85493

[Term]
id: terms:092419
name: Total CL Pred by F Norm by SA
def: "The total body clearance for extravascular administration divided by the fraction of dose absorbed, calculated using the predicted value of the last non-zero concentration, divided by the surface area."[]
is_a: terms:085493 ! terms_C85493

[Term]
id: terms:092420
name: Total CL Pred by F Norm by WT
def: "The total body clearance for extravascular administration divided by the fraction of dose absorbed, calculated using the predicted value of the last non-zero concentration, divided by the weight."[]
is_a: terms:085493 ! terms_C85493

[Term]
id: terms:092421
name: Total CL Pred Norm by BMI
def: "The total body clearance for intravascular administration, calculated using the predicted value of the last non-zero concentration, divided by the body mass index."[]
is_a: terms:085493 ! terms_C85493

[Term]
id: terms:092422
name: Total CL Pred Norm by Dose
def: "The total body clearance for intravascular administration, calculated using the predicted value of the last non-zero concentration, divided by the dose."[]
is_a: terms:085493 ! terms_C85493

[Term]
id: terms:092423
name: Total CL Pred Norm by SA
def: "The total body clearance for intravascular administration, calculated using the predicted value of the last non-zero concentration, divided by the surface area."[]
is_a: terms:085493 ! terms_C85493

[Term]
id: terms:092424
name: Total CL Pred Norm by WT
def: "The total body clearance for intravascular administration, calculated using the predicted value of the last non-zero concentration, divided by the weight."[]
is_a: terms:085493 ! terms_C85493

[Term]
id: terms:092425
name: Vz Pred Norm by BMI
def: "The volume of distribution associated with the terminal slope following intravascular administration, calculated using the predicted value of the last non-zero concentration, divided by the body mass index."[]
is_a: terms:085493 ! terms_C85493

[Term]
id: terms:092426
name: Vz Pred Norm by SA
def: "The volume of distribution associated with the terminal slope following intravascular administration, calculated using the predicted value of the last non-zero concentration, divided by the surface area."[]
is_a: terms:085493 ! terms_C85493

[Term]
id: terms:092427
name: Vz Pred Norm by WT
def: "The volume of distribution associated with the terminal slope following intravascular administration, calculated using the predicted value of the last non-zero concentration, divided by the weight."[]
is_a: terms:085493 ! terms_C85493

[Term]
id: terms:092428
name: Vz Pred by F Norm by BMI
def: "The volume of distribution associated with the terminal slope following extravascular administration divided by the fraction of dose absorbed, calculated using the predicted value of the last non-zero concentration, divided by the body mass index."[]
is_a: terms:085493 ! terms_C85493

[Term]
id: terms:092429
name: Vz Pred by F Norm by SA
def: "The volume of distribution associated with the terminal slope following extravascular administration divided by the fraction of dose absorbed, calculated using the predicted value of the last non-zero concentration, divided by the surface area."[]
is_a: terms:085493 ! terms_C85493

[Term]
id: terms:092430
name: Vz Pred by F Norm by WT
def: "The volume of distribution associated with the terminal slope following extravascular administration divided by the fraction of dose absorbed, calculated using the predicted value of the last non-zero concentration, divided by the weight."[]
is_a: terms:085493 ! terms_C85493

[Term]
id: terms:095007
name: Effective Half-Life
def: "The drug half-life that quantifies the accumulation ratio of a drug following multiple dosing."[]
synonym: "Beta half-life (model dependent analysis)" RELATED [VX]
synonym: "Distribution half-life" RELATED [VX]
synonym: "Distribution half-life (t)" RELATED [VX]
synonym: "E t1/2" NARROW [VX]
synonym: "E t1/2 a" NARROW [VX]
synonym: "E t1/2 alpha" NARROW [VX]
synonym: "E t1/2 b" NARROW [VX]
synonym: "E t1/2 beta" NARROW [VX]
synonym: "EFFHL" EXACT [SEND]
synonym: "Effective t1/2" RELATED [VX]
synonym: "Et1/2 beta" RELATED [VX]
synonym: "Haf-life (t1/2)" RELATED [VX]
synonym: "Half life" EXACT [VX]
synonym: "Half llife" EXACT [VX]
synonym: "Half-life" EXACT [VX]
synonym: "Half-life (t(1/2))" RELATED [VX]
synonym: "Half-life (t1/2)" RELATED [VX]
synonym: "Half-life beta" RELATED [VX]
synonym: "Half-life, alfa" RELATED [VX]
synonym: "Half-life, beta" RELATED [VX]
synonym: "Hlaf-life" RELATED [VX]
synonym: "Mean T 1/2" RELATED [VX]
synonym: "Plasma half-life" NARROW [VX]
synonym: "Plasma ultrafiltrate half-life" NARROW [VX]
synonym: "Plasma ultrafiltrate half-life (Terminal phase)" NARROW [VX]
synonym: "T 1/2" EXACT [VX]
synonym: "T 1/2 (multiple dose)" RELATED [VX]
synonym: "T 1/2 (multiple dose, after 1st daily dose)" NARROW [VX]
synonym: "T 1/2 (multiple dose, after 2nd daily dose)" NARROW [VX]
synonym: "T 1/2 (single dose)" NARROW [VX]
synonym: "T1/2" EXACT [VX]
synonym: "T1/2 (Lu 33-108)" NARROW [VX]
synonym: "T1/2 a (ICS 205-930)" NARROW [VX]
synonym: "T1/2 a (metabolite x)" NARROW [VX]
synonym: "T1/2 alpha" NARROW [VX]
synonym: "T1/2 alpha  (metabolite X)" NARROW [VX]
synonym: "T1/2 b (ICS 205-930)" NARROW [VX]
synonym: "T1/2 b (metabolite x)" NARROW [VX]
synonym: "T1/2 beta" NARROW [VX]
synonym: "T1/2 beta (metabolite X)" NARROW [VX]
synonym: "T1/2 blood" RELATED [VX]
synonym: "T1/2 repeated dose (2nd dose)" RELATED [VX]
synonym: "T1/2a" RELATED [VX]
synonym: "T1/2b" RELATED [VX]
synonym: "T1/2elim" NARROW [VX]
synonym: "Terminal half life" RELATED [VX]
synonym: "t  1/2" EXACT [VX]
synonym: "t 1/2" EXACT [VX]
synonym: "t 1/2 (1)" NARROW [VX]
synonym: "t 1/2 (2)" NARROW [VX]
synonym: "t 1/2 1" NARROW [VX]
synonym: "t 1/2 after 1st dose" RELATED [VX]
synonym: "t 1/2 alpha" NARROW [VX]
synonym: "t 1/2 beta" NARROW [VX]
synonym: "t 1/2 plasma" RELATED [VX]
synonym: "t 1/2(mean Day1/Day5)" RELATED [VX]
synonym: "t max 2" RELATED [VX]
synonym: "t max.2" RELATED [VX]
synonym: "t(1/2)" EXACT [VX]
synonym: "t(1/2)alpha" NARROW [VX]
synonym: "t(1/2)beta" NARROW [VX]
synonym: "t1/2" EXACT [VX]
synonym: "t1/2 (1)" RELATED [VX]
synonym: "t1/2 (2)" RELATED [VX]
synonym: "t1/2 (SSR-epimer)" NARROW [VX]
synonym: "t1/2 (beta)" NARROW [VX]
synonym: "t1/2 (gamma)" RELATED [VX]
synonym: "t1/2 (h)" RELATED [VX]
synonym: "t1/2 a" NARROW [VX]
synonym: "t1/2 abs" RELATED [VX]
synonym: "t1/2 alpha" NARROW [VX]
synonym: "t1/2 b" NARROW [VX]
synonym: "t1/2 beta" NARROW [VX]
synonym: "t1/2 blood" RELATED [VX]
synonym: "t1/2 plasma" RELATED [VX]
synonym: "t1/2(144-192) plasma" RELATED [VX]
synonym: "t1/2(24-168h) blood" RELATED [VX]
synonym: "t1/2(5-30 min) blood" RELATED [VX]
synonym: "t1/2(6 or 8-240h) plasma" RELATED [VX]
synonym: "t1/2(6-12 or10h) blood" RELATED [VX]
synonym: "t1/2(Steady state- Days 14 & 22,combined)" RELATED [VX]
synonym: "t1/2(single dose)" RELATED [VX]
synonym: "t1/2(tmax-120h) plasma" RELATED [VX]
synonym: "t1/2(tmax-168 or 192h) blood" RELATED [VX]
synonym: "t1/2, 8-24 h" RELATED [VX]
synonym: "t1/2, abs" RELATED [VX]
synonym: "t1/2, alpha" NARROW [VX]
synonym: "t1/2, beta" NARROW [VX]
synonym: "t1/2, delta" RELATED [VX]
synonym: "t1/2, gamma" RELATED [VX]
synonym: "t1/2a" RELATED [VX]
synonym: "t1/2alpha" RELATED [VX]
synonym: "t1/2b" RELATED [VX]
synonym: "t1/2beta" RELATED [VX]
synonym: "tl/2" RELATED [VX]
is_a: terms:085493 ! terms_C85493

[Term]
id: terms:096695
name: AUC Infinity Obs Norm by Dose
def: "The area under the curve (AUC) extrapolated to infinity, calculated using the observed value of the last non-zero concentration, divided by the dose."[]
is_a: terms:085493 ! terms_C85493

